@prefix rdf: <http://www.w3.org/1999/02/22-rdf-syntax-ns#> .
@prefix rdfs: <http://www.w3.org/2000/01/rdf-schema#> .
@prefix owl: <http://www.w3.org/2002/07/owl#> .
@prefix xsd: <http://www.w3.org/2001/XMLSchema#> .
@prefix xml: <http://www.w3.org/XML/1998/namespace/> .
@prefix mms-ontology: <https://opencae.jpl.nasa.gov/mms/rdf/ontology/> .
@prefix mms-graph: <https://opencae.jpl.nasa.gov/mms/rdf/graph/> .
@prefix mms-property: <https://opencae.jpl.nasa.gov/mms/rdf/property/> .
@prefix mms-derived-property: <https://opencae.jpl.nasa.gov/mms/rdf/derived-property/> .
@prefix mms-class: <https://opencae.jpl.nasa.gov/mms/rdf/class/> .
@prefix mms-element: <https://opencae.jpl.nasa.gov/mms/rdf/element/> .
@prefix mms-artifact: <https://opencae.jpl.nasa.gov/mms/rdf/artifact/> .
@prefix mms-index: <https://opencae.jpl.nasa.gov/mms/rdf/index/> .
@prefix mms-shape: <https://opencae.jpl.nasa.gov/mms/rdf/shape/> .
@prefix xmi: <http://www.omg.org/spec/XMI/20131001#> .
@prefix uml: <http://www.omg.org/spec/UML/20161101#> .
@prefix uml-model: <https://www.omg.org/spec/UML/20161101/UML.xmi#> .
@prefix uml-model-dt: <https://www.omg.org/spec/UML/20161101/UML.xmi#datatype/> .
@prefix uml-primitives: <https://www.omg.org/spec/UML/20161101/PrimitiveTypes.xmi#> .
@prefix uml-class: <https://opencae.jpl.nasa.gov/mms/rdf/uml-class/> .
@prefix uml-property: <https://opencae.jpl.nasa.gov/mms/rdf/uml-property/> .
@prefix shacl: <http://www.w3.org/ns/shacl#> .

mms-class:Element a owl:Class ;
	rdfs:label "Element" ;
	owl:equivalentClass uml-class:Element ;
	mms-ontology:category mms-class:Element .

mms-class:Commit a owl:Class ;
	rdfs:label "Commit" ;
	mms-ontology:category mms-class:Artifact .

mms-class:Ref a owl:Class ;
	rdfs:label "Ref" ;
	mms-ontology:category mms-class:Artifact .

mms-class:Project a owl:Class ;
	rdfs:label "Project" ;
	mms-ontology:category mms-class:Artifact .

mms-ontology:Property a owl:Class ;
	rdfs:label "Property" .

mms-class:PropertyPath a owl:Class ;
	rdfs:label "Property Path" ;
	mms-ontology:category mms-class:ElementList .

mms-ontology:ObjectProperty a owl:Class ;
	rdfs:label "Object Property" ;
	owl:equivalentClass owl:ObjectProperty ;
	rdfs:subClassOf mms-ontology:Property .

mms-ontology:DatatypeProperty a owl:Class ;
	rdfs:label "Datatype Property" ;
	owl:equivalentClass owl:DatatypeProperty ;
	rdfs:subClassOf mms-ontology:Property .

mms-ontology:UmlObjectProperty a owl:Class ;
	rdfs:label "UML Object Property" ;
	rdfs:subClassOf mms-ontology:ObjectProperty .

mms-ontology:UmlDatatypeProperty a owl:Class ;
	rdfs:label "UML Datatype Property" ;
	rdfs:subClassOf mms-ontology:DatatypeProperty .

mms-ontology:DerivedObjectProperty a owl:Class ;
	rdfs:label "Derived Object Property" ;
	rdfs:subClassOf mms-ontology:ObjectProperty .

mms-ontology:DerivedDatatypeProperty a owl:Class ;
	rdfs:label "Derived Datatype Property" ;
	rdfs:subClassOf mms-ontology:DatatypeProperty .

# a datatype restriction for properties with langString ranges
mms-ontology:Comment_EN owl:equivalentClass [
		rdf:type rdfs:Datatype ;
		owl:onDatatype rdfs:langString ;
		owl:withRestrictions (
			[
				xml:lang "en"^^xsd:language ;
			]
		) ;
	] .

# an enumerated class declaration for types of visibility
mms-class:Visibility a mms-ontology:EnumeratedClass ;
	mms-ontology:category mms-class:Element ;
	owl:oneOf (
		mms-class:Visibility.Public
		mms-class:Visibility.Private
		mms-class:Visibility.None
	) .

mms-class:Visibility.Public a owl:Class ;
	mms-ontology:enumerationValue "public" ;
	mms-ontology:category mms-class:Element .

mms-class:Visibility.Private a owl:Class ;
	mms-ontology:enumerationValue "private" ;
	mms-ontology:category mms-class:Element .

mms-class:Visibility.None a owl:Class ;
	mms-ontology:enumerationValue rdf:nil ;
	mms-ontology:category mms-class:Element .

# special properties that need to be manually added to extend UML specification
mms-property:appliedStereotypeInstance a mms-ontology:UmlObjectProperty ;
	mms-ontology:cardinality "1"^^uml-model-dt:cardinalityRange ;
	mms-ontology:key "appliedStereotypeInstanceId" ;
	rdfs:label "Applied Stereotype Instance" ;
	rdfs:comment "An extension to the UML specification to account stereotype application from the Cameo Systems Modeler."@en ;
	rdfs:domain uml-class:Element ;
	rdfs:range uml-class:InstanceSpecification .

# special properties that need to be manually added to extend UML specification
mms-ontology:elementId a mms-ontology:DatatypeProperty ;
	rdfs:label "Element ID" ;
	rdfs:comment "A custom property to describe the original ID of the model element as a string."@en ;
	rdfs:domain mms-class:Element ;
	rdfs:range xsd:string .

mms-property:owningExpressionStringExpression a mms-ontology:UmlObjectProperty ;
	mms-ontology:cardinality "1"^^uml-model-dt:cardinalityRange ;
	mms-ontology:key "owningExpressionId" ;
	rdfs:label "owningExpressionStringExpression" ;
	rdfs:comment "The StringExpression that is the owningExpression of this StringExpression. Based on the UML property 'StringExpression-owningExpression' which is described as: The StringExpression of which this StringExpression is a subExpression."@en ;
	rdfs:domain uml-class:StringExpression ;
	rdfs:range uml-class:StringExpression ;
	mms-ontology:umlPropertySource uml-property:StringExpression-owningExpression .

mms-property:qualifierQualifierValue a mms-ontology:UmlObjectProperty ;
	mms-ontology:cardinality "*"^^uml-model-dt:cardinalityRange ;
	mms-ontology:key "qualifierIds" ;
	rdfs:label "qualifierQualifierValue" ;
	rdfs:comment "A QualifierValue that is the qualifier of this LinkEndData. Based on the UML property 'LinkEndData-qualifier' which is described as: A set of QualifierValues used to provide values for the qualifiers of the end."@en ;
	rdfs:domain uml-class:LinkEndData ;
	rdfs:range uml-class:QualifierValue ;
	mms-ontology:umlPropertySource uml-property:LinkEndData-qualifier .

mms-property:qualifierPropertyFromProperty a mms-ontology:UmlObjectProperty ;
	mms-ontology:cardinality "*"^^uml-model-dt:cardinalityRange ;
	mms-ontology:key "qualifierIds" ;
	rdfs:label "qualifierPropertyFromProperty" ;
	rdfs:comment "A Property that is the qualifier of this Property. Based on the UML property 'Property-qualifier' which is described as: An optional list of ordered qualifier attributes for the end."@en ;
	rdfs:domain uml-class:Property ;
	rdfs:range uml-class:Property ;
	mms-ontology:umlPropertySource uml-property:Property-qualifier .

mms-property:qualifierPropertyFromQualifierValue a mms-ontology:UmlObjectProperty ;
	mms-ontology:cardinality "1"^^uml-model-dt:cardinalityRange ;
	mms-ontology:key "qualifierId" ;
	rdfs:label "qualifierPropertyFromQualifierValue" ;
	rdfs:comment "The Property that is the qualifier of this QualifierValue. Based on the UML property 'QualifierValue-qualifier' which is described as: The qualifier Property for which the value is to be specified."@en ;
	rdfs:domain uml-class:QualifierValue ;
	rdfs:range uml-class:Property ;
	mms-ontology:umlPropertySource uml-property:QualifierValue-qualifier .

mms-property:qualifierPropertyFromReadLinkObjectEndQualifierAction a mms-ontology:UmlObjectProperty ;
	mms-ontology:cardinality "1"^^uml-model-dt:cardinalityRange ;
	mms-ontology:key "qualifierId" ;
	rdfs:label "qualifierPropertyFromReadLinkObjectEndQualifierAction" ;
	rdfs:comment "The Property that is the qualifier of this ReadLinkObjectEndQualifierAction. Based on the UML property 'ReadLinkObjectEndQualifierAction-qualifier' which is described as: The qualifier Property to be read."@en ;
	rdfs:domain uml-class:ReadLinkObjectEndQualifierAction ;
	rdfs:range uml-class:Property ;
	mms-ontology:umlPropertySource uml-property:ReadLinkObjectEndQualifierAction-qualifier .

mms-property:elementImport a mms-ontology:UmlObjectProperty ;
	mms-ontology:cardinality "*"^^uml-model-dt:cardinalityRange ;
	mms-ontology:key "elementImportIds" ;
	rdfs:label "elementImport" ;
	rdfs:comment "A ElementImport that belongs to this Namespace. Based on the UML property 'Namespace-elementImport' which is described as: References the ElementImports owned by the Namespace."@en ;
	rdfs:domain uml-class:Namespace ;
	rdfs:range uml-class:ElementImport ;
	mms-ontology:umlPropertySource uml-property:Namespace-elementImport .

mms-property:maxintValueSpecification a mms-ontology:UmlObjectProperty ;
	mms-ontology:cardinality "1"^^uml-model-dt:cardinalityRange ;
	mms-ontology:key "maxintId" ;
	rdfs:label "maxintValueSpecification" ;
	rdfs:comment "The ValueSpecification that is the maxint of this InteractionConstraint. Based on the UML property 'InteractionConstraint-maxint' which is described as: The maximum number of iterations of a loop"@en ;
	rdfs:domain uml-class:InteractionConstraint ;
	rdfs:range uml-class:ValueSpecification ;
	mms-ontology:umlPropertySource uml-property:InteractionConstraint-maxint .

mms-property:qualifiedNameString a mms-ontology:UmlDatatypeProperty ;
	mms-ontology:cardinality "1"^^uml-model-dt:cardinalityRange ;
	mms-ontology:key "qualifiedNameId" ;
	rdfs:label "qualifiedNameString" ;
	rdfs:comment "The String that is the qualifiedName of this NamedElement. Based on the UML property 'NamedElement-qualifiedName' which is described as: A name that allows the NamedElement to be identified within a hierarchy of nested Namespaces. It is constructed from the names of the containing Namespaces starting at the root of the hierarchy and ending with the name of the NamedElement itself."@en ;
	rdfs:domain uml-class:NamedElement ;
	rdfs:range xsd:string ;
	mms-ontology:umlPropertySource uml-property:NamedElement-qualifiedName .

mms-property:featuringClassifier a mms-ontology:UmlObjectProperty ;
	mms-ontology:cardinality "1"^^uml-model-dt:cardinalityRange ;
	mms-ontology:key "featuringClassifierId" ;
	rdfs:label "featuringClassifier" ;
	rdfs:comment "The Classifier that belongs to this Feature. Based on the UML property 'Feature-featuringClassifier' which is described as: The Classifiers that have this Feature as a feature."@en ;
	rdfs:domain uml-class:Feature ;
	rdfs:range uml-class:Classifier ;
	mms-ontology:umlPropertySource uml-property:Feature-featuringClassifier .

mms-property:receivingPackage a mms-ontology:UmlObjectProperty ;
	mms-ontology:cardinality "1"^^uml-model-dt:cardinalityRange ;
	mms-ontology:key "receivingPackageId" ;
	rdfs:label "receivingPackage" ;
	rdfs:comment "The Package that belongs to this PackageMerge. Based on the UML property 'PackageMerge-receivingPackage' which is described as: References the Package that is being extended with the contents of the merged package of the PackageMerge."@en ;
	rdfs:domain uml-class:PackageMerge ;
	rdfs:range uml-class:Package ;
	mms-ontology:umlPropertySource uml-property:PackageMerge-receivingPackage .

mms-property:isControlType a mms-ontology:UmlDatatypeProperty ;
	mms-ontology:key "isControlType" ;
	rdfs:label "isControlType" ;
	rdfs:comment "Indicates whether the type of the ObjectNode is to be treated as representing control values that may traverse ControlFlows."@en ;
	rdfs:domain uml-class:ObjectNode ;
	rdfs:range xsd:boolean ;
	mms-ontology:umlPropertySource uml-property:ObjectNode-isControlType .

mms-property:isControlTypeObjectNode a mms-ontology:UmlDatatypeProperty ;
	owl:equivalentProperty mms-property:isControlType .

mms-property:submachineStateMachine a mms-ontology:UmlObjectProperty ;
	mms-ontology:cardinality "1"^^uml-model-dt:cardinalityRange ;
	mms-ontology:key "submachineId" ;
	rdfs:label "submachineStateMachine" ;
	rdfs:comment "The StateMachine that is the submachine of this State. Based on the UML property 'State-submachine' which is described as: The StateMachine that is to be inserted in place of the (submachine) State."@en ;
	rdfs:domain uml-class:State ;
	rdfs:range uml-class:StateMachine ;
	mms-ontology:umlPropertySource uml-property:State-submachine .

mms-property:objectInputPinFromClearAssociationAction a mms-ontology:UmlObjectProperty ;
	mms-ontology:cardinality "1"^^uml-model-dt:cardinalityRange ;
	mms-ontology:key "objectId" ;
	rdfs:label "objectInputPinFromClearAssociationAction" ;
	rdfs:comment "The InputPin that is the object of this ClearAssociationAction. Based on the UML property 'ClearAssociationAction-object' which is described as: The InputPin that gives the object whose participation in the Association is to be cleared."@en ;
	rdfs:domain uml-class:ClearAssociationAction ;
	rdfs:range uml-class:InputPin ;
	mms-ontology:umlPropertySource uml-property:ClearAssociationAction-object .

mms-property:objectInputPinFromReadIsClassifiedObjectAction a mms-ontology:UmlObjectProperty ;
	mms-ontology:cardinality "1"^^uml-model-dt:cardinalityRange ;
	mms-ontology:key "objectId" ;
	rdfs:label "objectInputPinFromReadIsClassifiedObjectAction" ;
	rdfs:comment "The InputPin that is the object of this ReadIsClassifiedObjectAction. Based on the UML property 'ReadIsClassifiedObjectAction-object' which is described as: The InputPin that holds the object whose classification is to be tested."@en ;
	rdfs:domain uml-class:ReadIsClassifiedObjectAction ;
	rdfs:range uml-class:InputPin ;
	mms-ontology:umlPropertySource uml-property:ReadIsClassifiedObjectAction-object .

mms-property:objectInputPinFromReclassifyObjectAction a mms-ontology:UmlObjectProperty ;
	mms-ontology:cardinality "1"^^uml-model-dt:cardinalityRange ;
	mms-ontology:key "objectId" ;
	rdfs:label "objectInputPinFromReclassifyObjectAction" ;
	rdfs:comment "The InputPin that is the object of this ReclassifyObjectAction. Based on the UML property 'ReclassifyObjectAction-object' which is described as: The InputPin that holds the object to be reclassified."@en ;
	rdfs:domain uml-class:ReclassifyObjectAction ;
	rdfs:range uml-class:InputPin ;
	mms-ontology:umlPropertySource uml-property:ReclassifyObjectAction-object .

mms-property:objectInputPinFromReadLinkObjectEndAction a mms-ontology:UmlObjectProperty ;
	mms-ontology:cardinality "1"^^uml-model-dt:cardinalityRange ;
	mms-ontology:key "objectId" ;
	rdfs:label "objectInputPinFromReadLinkObjectEndAction" ;
	rdfs:comment "The InputPin that is the object of this ReadLinkObjectEndAction. Based on the UML property 'ReadLinkObjectEndAction-object' which is described as: The input pin from which the link object is obtained."@en ;
	rdfs:domain uml-class:ReadLinkObjectEndAction ;
	rdfs:range uml-class:InputPin ;
	mms-ontology:umlPropertySource uml-property:ReadLinkObjectEndAction-object .

mms-property:objectInputPinFromUnmarshallAction a mms-ontology:UmlObjectProperty ;
	mms-ontology:cardinality "1"^^uml-model-dt:cardinalityRange ;
	mms-ontology:key "objectId" ;
	rdfs:label "objectInputPinFromUnmarshallAction" ;
	rdfs:comment "The InputPin that is the object of this UnmarshallAction. Based on the UML property 'UnmarshallAction-object' which is described as: The InputPin that gives the object to be unmarshalled."@en ;
	rdfs:domain uml-class:UnmarshallAction ;
	rdfs:range uml-class:InputPin ;
	mms-ontology:umlPropertySource uml-property:UnmarshallAction-object .

mms-property:objectInputPinFromStartClassifierBehaviorAction a mms-ontology:UmlObjectProperty ;
	mms-ontology:cardinality "1"^^uml-model-dt:cardinalityRange ;
	mms-ontology:key "objectId" ;
	rdfs:label "objectInputPinFromStartClassifierBehaviorAction" ;
	rdfs:comment "The InputPin that is the object of this StartClassifierBehaviorAction. Based on the UML property 'StartClassifierBehaviorAction-object' which is described as: The InputPin that holds the object whose classifierBehavior is to be started."@en ;
	rdfs:domain uml-class:StartClassifierBehaviorAction ;
	rdfs:range uml-class:InputPin ;
	mms-ontology:umlPropertySource uml-property:StartClassifierBehaviorAction-object .

mms-property:objectInputPinFromStructuralFeatureAction a mms-ontology:UmlObjectProperty ;
	mms-ontology:cardinality "1"^^uml-model-dt:cardinalityRange ;
	mms-ontology:key "objectId" ;
	rdfs:label "objectInputPinFromStructuralFeatureAction" ;
	rdfs:comment "The InputPin that is the object of this StructuralFeatureAction. Based on the UML property 'StructuralFeatureAction-object' which is described as: The InputPin from which the object whose StructuralFeature is to be read or written is obtained."@en ;
	rdfs:domain uml-class:StructuralFeatureAction ;
	rdfs:range uml-class:InputPin ;
	mms-ontology:umlPropertySource uml-property:StructuralFeatureAction-object .

mms-property:objectInputPinFromStartObjectBehaviorAction a mms-ontology:UmlObjectProperty ;
	mms-ontology:cardinality "1"^^uml-model-dt:cardinalityRange ;
	mms-ontology:key "objectId" ;
	rdfs:label "objectInputPinFromStartObjectBehaviorAction" ;
	rdfs:comment "The InputPin that is the object of this StartObjectBehaviorAction. Based on the UML property 'StartObjectBehaviorAction-object' which is described as: An InputPin that holds the object that is either a Behavior to be started or has a classifierBehavior to be started."@en ;
	rdfs:domain uml-class:StartObjectBehaviorAction ;
	rdfs:range uml-class:InputPin ;
	mms-ontology:umlPropertySource uml-property:StartObjectBehaviorAction-object .

mms-property:objectInputPinFromReadLinkObjectEndQualifierAction a mms-ontology:UmlObjectProperty ;
	mms-ontology:cardinality "1"^^uml-model-dt:cardinalityRange ;
	mms-ontology:key "objectId" ;
	rdfs:label "objectInputPinFromReadLinkObjectEndQualifierAction" ;
	rdfs:comment "The InputPin that is the object of this ReadLinkObjectEndQualifierAction. Based on the UML property 'ReadLinkObjectEndQualifierAction-object' which is described as: The InputPin from which the link object is obtained."@en ;
	rdfs:domain uml-class:ReadLinkObjectEndQualifierAction ;
	rdfs:range uml-class:InputPin ;
	mms-ontology:umlPropertySource uml-property:ReadLinkObjectEndQualifierAction-object .

mms-property:namespace a mms-ontology:UmlObjectProperty ;
	mms-ontology:cardinality "1"^^uml-model-dt:cardinalityRange ;
	mms-ontology:key "namespaceId" ;
	rdfs:label "namespace" ;
	rdfs:comment "The Namespace that belongs to this NamedElement. Based on the UML property 'NamedElement-namespace' which is described as: Specifies the Namespace that owns the NamedElement."@en ;
	rdfs:domain uml-class:NamedElement ;
	rdfs:range uml-class:Namespace ;
	mms-ontology:umlPropertySource uml-property:NamedElement-namespace .

mms-property:isUnmarshall a mms-ontology:UmlDatatypeProperty ;
	mms-ontology:key "isUnmarshall" ;
	rdfs:label "isUnmarshall" ;
	rdfs:comment "Indicates whether there is a single OutputPin for a SignalEvent occurrence, or multiple OutputPins for attribute values of the instance of the Signal associated with a SignalEvent occurrence."@en ;
	rdfs:domain uml-class:AcceptEventAction ;
	rdfs:range xsd:boolean ;
	mms-ontology:umlPropertySource uml-property:AcceptEventAction-isUnmarshall .

mms-property:isUnmarshallAcceptEventAction a mms-ontology:UmlDatatypeProperty ;
	owl:equivalentProperty mms-property:isUnmarshall .

mms-property:URIString a mms-ontology:UmlDatatypeProperty ;
	mms-ontology:cardinality "1"^^uml-model-dt:cardinalityRange ;
	mms-ontology:key "URIId" ;
	rdfs:label "URIString" ;
	rdfs:comment "The String that is the URI of this Package. Based on the UML property 'Package-URI' which is described as: Provides an identifier for the package that can be used for many purposes. A URI is the universally unique identification of the package following the IETF URI specification, RFC 2396 http://www.ietf.org/rfc/rfc2396.txt and it must comply with those syntax rules."@en ;
	rdfs:domain uml-class:Package ;
	rdfs:range xsd:string ;
	mms-ontology:umlPropertySource uml-property:Package-URI .

mms-property:typeAssociation a mms-ontology:UmlObjectProperty ;
	mms-ontology:cardinality "1"^^uml-model-dt:cardinalityRange ;
	mms-ontology:key "typeId" ;
	rdfs:label "typeAssociation" ;
	rdfs:comment "The Association that is the type of this Connector. Based on the UML property 'Connector-type' which is described as: An optional Association that classifies links corresponding to this Connector."@en ;
	rdfs:domain uml-class:Connector ;
	rdfs:range uml-class:Association ;
	mms-ontology:umlPropertySource uml-property:Connector-type .

mms-property:typeFromTypedElement a mms-ontology:UmlObjectProperty ;
	mms-ontology:cardinality "1"^^uml-model-dt:cardinalityRange ;
	mms-ontology:key "typeId" ;
	rdfs:label "typeFromTypedElement" ;
	rdfs:comment "The Type that belongs to this TypedElement. Based on the UML property 'TypedElement-type' which is described as: The type of the TypedElement."@en ;
	rdfs:domain uml-class:TypedElement ;
	rdfs:range uml-class:Type ;
	mms-ontology:umlPropertySource uml-property:TypedElement-type .

mms-property:typeFromOperation a mms-ontology:UmlObjectProperty ;
	mms-ontology:cardinality "1"^^uml-model-dt:cardinalityRange ;
	mms-ontology:key "typeId" ;
	rdfs:label "typeFromOperation" ;
	rdfs:comment "The Type that belongs to this Operation. Based on the UML property 'Operation-type' which is described as: The return type of the operation, if present. This information is derived from the return result for this Operation."@en ;
	rdfs:domain uml-class:Operation ;
	rdfs:range uml-class:Type ;
	mms-ontology:umlPropertySource uml-property:Operation-type .

mms-property:typeCollaboration a mms-ontology:UmlObjectProperty ;
	mms-ontology:cardinality "1"^^uml-model-dt:cardinalityRange ;
	mms-ontology:key "typeId" ;
	rdfs:label "typeCollaboration" ;
	rdfs:comment "The Collaboration that is the type of this CollaborationUse. Based on the UML property 'CollaborationUse-type' which is described as: The Collaboration which is used in this CollaborationUse. The Collaboration defines the cooperation between its roles which are mapped to ConnectableElements relating to the Classifier owning the CollaborationUse."@en ;
	rdfs:domain uml-class:CollaborationUse ;
	rdfs:range uml-class:Collaboration ;
	mms-ontology:umlPropertySource uml-property:CollaborationUse-type .

mms-property:typeStereotype a mms-ontology:UmlObjectProperty ;
	mms-ontology:cardinality "1"^^uml-model-dt:cardinalityRange ;
	mms-ontology:key "typeId" ;
	rdfs:label "typeStereotype" ;
	rdfs:comment "The Stereotype that is the type of this ExtensionEnd. Based on the UML property 'ExtensionEnd-type' which is described as: References the type of the ExtensionEnd. Note that this association restricts the possible types of an ExtensionEnd to only be Stereotypes."@en ;
	rdfs:domain uml-class:ExtensionEnd ;
	rdfs:range uml-class:Stereotype ;
	mms-ontology:umlPropertySource uml-property:ExtensionEnd-type .

mms-property:signatureNamedElement a mms-ontology:UmlObjectProperty ;
	mms-ontology:cardinality "1"^^uml-model-dt:cardinalityRange ;
	mms-ontology:key "signatureId" ;
	rdfs:label "signatureNamedElement" ;
	rdfs:comment "The NamedElement that is the signature of this Message. Based on the UML property 'Message-signature' which is described as: The signature of the Message is the specification of its content. It refers either an Operation or a Signal."@en ;
	rdfs:domain uml-class:Message ;
	rdfs:range uml-class:NamedElement ;
	mms-ontology:umlPropertySource uml-property:Message-signature .

mms-property:signatureTemplateSignatureFromTemplateParameter a mms-ontology:UmlObjectProperty ;
	mms-ontology:cardinality "1"^^uml-model-dt:cardinalityRange ;
	mms-ontology:key "signatureId" ;
	rdfs:label "signatureTemplateSignatureFromTemplateParameter" ;
	rdfs:comment "The TemplateSignature that is the signature of this TemplateParameter. Based on the UML property 'TemplateParameter-signature' which is described as: The TemplateSignature that owns this TemplateParameter."@en ;
	rdfs:domain uml-class:TemplateParameter ;
	rdfs:range uml-class:TemplateSignature ;
	mms-ontology:umlPropertySource uml-property:TemplateParameter-signature .

mms-property:signatureTemplateSignatureFromTemplateBinding a mms-ontology:UmlObjectProperty ;
	mms-ontology:cardinality "1"^^uml-model-dt:cardinalityRange ;
	mms-ontology:key "signatureId" ;
	rdfs:label "signatureTemplateSignatureFromTemplateBinding" ;
	rdfs:comment "The TemplateSignature that is the signature of this TemplateBinding. Based on the UML property 'TemplateBinding-signature' which is described as: The TemplateSignature for the template that is the target of this TemplateBinding."@en ;
	rdfs:domain uml-class:TemplateBinding ;
	rdfs:range uml-class:TemplateSignature ;
	mms-ontology:umlPropertySource uml-property:TemplateBinding-signature .

mms-property:inputValueFromLinkAction a mms-ontology:UmlObjectProperty ;
	mms-ontology:cardinality "*"^^uml-model-dt:cardinalityRange ;
	mms-ontology:key "inputValueIds" ;
	rdfs:label "inputValueFromLinkAction" ;
	rdfs:comment "A InputPin that is the inputValue of this LinkAction. Based on the UML property 'LinkAction-inputValue' which is described as: InputPins used by the LinkEndData of the LinkAction."@en ;
	rdfs:domain uml-class:LinkAction ;
	rdfs:range uml-class:InputPin ;
	mms-ontology:umlPropertySource uml-property:LinkAction-inputValue .

mms-property:inputValueFromOpaqueAction a mms-ontology:UmlObjectProperty ;
	mms-ontology:cardinality "*"^^uml-model-dt:cardinalityRange ;
	mms-ontology:key "inputValueIds" ;
	rdfs:label "inputValueFromOpaqueAction" ;
	rdfs:comment "A InputPin that is the inputValue of this OpaqueAction. Based on the UML property 'OpaqueAction-inputValue' which is described as: The InputPins providing inputs to the OpaqueAction."@en ;
	rdfs:domain uml-class:OpaqueAction ;
	rdfs:range uml-class:InputPin ;
	mms-ontology:umlPropertySource uml-property:OpaqueAction-inputValue .

mms-property:importingNamespaceFromPackageImport a mms-ontology:UmlObjectProperty ;
	mms-ontology:cardinality "1"^^uml-model-dt:cardinalityRange ;
	mms-ontology:key "importingNamespaceId" ;
	rdfs:label "importingNamespaceFromPackageImport" ;
	rdfs:comment "The Namespace that belongs to this PackageImport. Based on the UML property 'PackageImport-importingNamespace' which is described as: Specifies the Namespace that imports the members from a Package."@en ;
	rdfs:domain uml-class:PackageImport ;
	rdfs:range uml-class:Namespace ;
	mms-ontology:umlPropertySource uml-property:PackageImport-importingNamespace .

mms-property:importingNamespaceFromElementImport a mms-ontology:UmlObjectProperty ;
	mms-ontology:cardinality "1"^^uml-model-dt:cardinalityRange ;
	mms-ontology:key "importingNamespaceId" ;
	rdfs:label "importingNamespaceFromElementImport" ;
	rdfs:comment "The Namespace that belongs to this ElementImport. Based on the UML property 'ElementImport-importingNamespace' which is described as: Specifies the Namespace that imports a PackageableElement from another Namespace."@en ;
	rdfs:domain uml-class:ElementImport ;
	rdfs:range uml-class:Namespace ;
	mms-ontology:umlPropertySource uml-property:ElementImport-importingNamespace .

mms-property:reducerBehavior a mms-ontology:UmlObjectProperty ;
	mms-ontology:cardinality "1"^^uml-model-dt:cardinalityRange ;
	mms-ontology:key "reducerId" ;
	rdfs:label "reducerBehavior" ;
	rdfs:comment "The Behavior that is the reducer of this ReduceAction. Based on the UML property 'ReduceAction-reducer' which is described as: A Behavior that is repreatedly applied to two elements of the input collection to produce a value that is of the same type as elements of the collection."@en ;
	rdfs:domain uml-class:ReduceAction ;
	rdfs:range uml-class:Behavior ;
	mms-ontology:umlPropertySource uml-property:ReduceAction-reducer .

mms-property:inGroupFromActivityNode a mms-ontology:UmlObjectProperty ;
	mms-ontology:cardinality "*"^^uml-model-dt:cardinalityRange ;
	mms-ontology:key "inGroupIds" ;
	rdfs:label "inGroupFromActivityNode" ;
	rdfs:comment "A ActivityGroup that is the inGroup of this ActivityNode. Based on the UML property 'ActivityNode-inGroup' which is described as: ActivityGroups containing the ActivityNode."@en ;
	rdfs:domain uml-class:ActivityNode ;
	rdfs:range uml-class:ActivityGroup ;
	mms-ontology:umlPropertySource uml-property:ActivityNode-inGroup .

mms-property:inGroupFromActivityEdge a mms-ontology:UmlObjectProperty ;
	mms-ontology:cardinality "*"^^uml-model-dt:cardinalityRange ;
	mms-ontology:key "inGroupIds" ;
	rdfs:label "inGroupFromActivityEdge" ;
	rdfs:comment "A ActivityGroup that is the inGroup of this ActivityEdge. Based on the UML property 'ActivityEdge-inGroup' which is described as: ActivityGroups containing the ActivityEdge."@en ;
	rdfs:domain uml-class:ActivityEdge ;
	rdfs:range uml-class:ActivityGroup ;
	mms-ontology:umlPropertySource uml-property:ActivityEdge-inGroup .

mms-property:structuredNodeInput a mms-ontology:UmlObjectProperty ;
	mms-ontology:cardinality "*"^^uml-model-dt:cardinalityRange ;
	mms-ontology:key "structuredNodeInputIds" ;
	rdfs:label "structuredNodeInput" ;
	rdfs:comment "A InputPin that is the structuredNodeInput of this StructuredActivityNode. Based on the UML property 'StructuredActivityNode-structuredNodeInput' which is described as: The InputPins owned by the StructuredActivityNode."@en ;
	rdfs:domain uml-class:StructuredActivityNode ;
	rdfs:range uml-class:InputPin ;
	mms-ontology:umlPropertySource uml-property:StructuredActivityNode-structuredNodeInput .

mms-property:executionExecutionSpecification a mms-ontology:UmlObjectProperty ;
	mms-ontology:cardinality "1"^^uml-model-dt:cardinalityRange ;
	mms-ontology:key "executionId" ;
	rdfs:label "executionExecutionSpecification" ;
	rdfs:comment "The ExecutionSpecification that is the execution of this ExecutionOccurrenceSpecification. Based on the UML property 'ExecutionOccurrenceSpecification-execution' which is described as: References the execution specification describing the execution that is started or finished at this execution event."@en ;
	rdfs:domain uml-class:ExecutionOccurrenceSpecification ;
	rdfs:range uml-class:ExecutionSpecification ;
	mms-ontology:umlPropertySource uml-property:ExecutionOccurrenceSpecification-execution .

mms-property:member a mms-ontology:UmlObjectProperty ;
	mms-ontology:cardinality "*"^^uml-model-dt:cardinalityRange ;
	mms-ontology:key "memberIds" ;
	rdfs:label "member" ;
	rdfs:comment "A NamedElement that is the member of this Namespace. Based on the UML property 'Namespace-member' which is described as: A collection of NamedElements identifiable within the Namespace, either by being owned or by being introduced by importing or inheritance."@en ;
	rdfs:domain uml-class:Namespace ;
	rdfs:range uml-class:NamedElement ;
	mms-ontology:umlPropertySource uml-property:Namespace-member .

mms-property:collaborationUse a mms-ontology:UmlObjectProperty ;
	mms-ontology:cardinality "*"^^uml-model-dt:cardinalityRange ;
	mms-ontology:key "collaborationUseIds" ;
	rdfs:label "collaborationUse" ;
	rdfs:comment "A CollaborationUse that belongs to this Classifier. Based on the UML property 'Classifier-collaborationUse' which is described as: The CollaborationUses owned by the Classifier."@en ;
	rdfs:domain uml-class:Classifier ;
	rdfs:range uml-class:CollaborationUse ;
	mms-ontology:umlPropertySource uml-property:Classifier-collaborationUse .

mms-property:endPropertyFromLinkEndData a mms-ontology:UmlObjectProperty ;
	mms-ontology:cardinality "1"^^uml-model-dt:cardinalityRange ;
	mms-ontology:key "endId" ;
	rdfs:label "endPropertyFromLinkEndData" ;
	rdfs:comment "The Property that is the end of this LinkEndData. Based on the UML property 'LinkEndData-end' which is described as: The Association end for which this LinkEndData specifies values."@en ;
	rdfs:domain uml-class:LinkEndData ;
	rdfs:range uml-class:Property ;
	mms-ontology:umlPropertySource uml-property:LinkEndData-end .

mms-property:endPropertyFromReadLinkObjectEndAction a mms-ontology:UmlObjectProperty ;
	mms-ontology:cardinality "1"^^uml-model-dt:cardinalityRange ;
	mms-ontology:key "endId" ;
	rdfs:label "endPropertyFromReadLinkObjectEndAction" ;
	rdfs:comment "The Property that is the end of this ReadLinkObjectEndAction. Based on the UML property 'ReadLinkObjectEndAction-end' which is described as: The Association end to be read."@en ;
	rdfs:domain uml-class:ReadLinkObjectEndAction ;
	rdfs:range uml-class:Property ;
	mms-ontology:umlPropertySource uml-property:ReadLinkObjectEndAction-end .

mms-property:endConnectorEndFromConnectableElement a mms-ontology:UmlObjectProperty ;
	mms-ontology:cardinality "*"^^uml-model-dt:cardinalityRange ;
	mms-ontology:key "endIds" ;
	rdfs:label "endConnectorEndFromConnectableElement" ;
	rdfs:comment "A ConnectorEnd that is the end of this ConnectableElement. Based on the UML property 'ConnectableElement-end' which is described as: A set of ConnectorEnds that attach to this ConnectableElement."@en ;
	rdfs:domain uml-class:ConnectableElement ;
	rdfs:range uml-class:ConnectorEnd ;
	mms-ontology:umlPropertySource uml-property:ConnectableElement-end .

mms-property:endConnectorEndFromConnector a mms-ontology:UmlObjectProperty ;
	mms-ontology:cardinality "*"^^uml-model-dt:cardinalityRange ;
	mms-ontology:key "endIds" ;
	rdfs:label "endConnectorEndFromConnector" ;
	rdfs:comment "A ConnectorEnd that is the end of this Connector. Based on the UML property 'Connector-end' which is described as: A Connector has at least two ConnectorEnds, each representing the participation of instances of the Classifiers typing the ConnectableElements attached to the end. The set of ConnectorEnds is ordered."@en ;
	rdfs:domain uml-class:Connector ;
	rdfs:range uml-class:ConnectorEnd ;
	mms-ontology:umlPropertySource uml-property:Connector-end .

mms-property:handlerBodyExecutableNode a mms-ontology:UmlObjectProperty ;
	mms-ontology:cardinality "1"^^uml-model-dt:cardinalityRange ;
	mms-ontology:key "handlerBodyId" ;
	rdfs:label "handlerBodyExecutableNode" ;
	rdfs:comment "The ExecutableNode that is the handlerBody of this ExceptionHandler. Based on the UML property 'ExceptionHandler-handlerBody' which is described as: An ExecutableNode that is executed if the ExceptionHandler catches an exception."@en ;
	rdfs:domain uml-class:ExceptionHandler ;
	rdfs:range uml-class:ExecutableNode ;
	mms-ontology:umlPropertySource uml-property:ExceptionHandler-handlerBody .

mms-property:ownedAttributeFromClass a mms-ontology:UmlObjectProperty ;
	mms-ontology:cardinality "*"^^uml-model-dt:cardinalityRange ;
	mms-ontology:key "ownedAttributeIds" ;
	rdfs:label "ownedAttributeFromClass" ;
	rdfs:comment "A Property that is the ownedAttribute of this Class. Based on the UML property 'Class-ownedAttribute' which is described as: The attributes (i.e., the Properties) owned by the Class."@en ;
	rdfs:domain uml-class:Class ;
	rdfs:range uml-class:Property ;
	mms-ontology:umlPropertySource uml-property:Class-ownedAttribute .

mms-property:ownedAttributeFromSignal a mms-ontology:UmlObjectProperty ;
	mms-ontology:cardinality "*"^^uml-model-dt:cardinalityRange ;
	mms-ontology:key "ownedAttributeIds" ;
	rdfs:label "ownedAttributeFromSignal" ;
	rdfs:comment "A Property that is the ownedAttribute of this Signal. Based on the UML property 'Signal-ownedAttribute' which is described as: The attributes owned by the Signal."@en ;
	rdfs:domain uml-class:Signal ;
	rdfs:range uml-class:Property ;
	mms-ontology:umlPropertySource uml-property:Signal-ownedAttribute .

mms-property:ownedAttributeFromDataType a mms-ontology:UmlObjectProperty ;
	mms-ontology:cardinality "*"^^uml-model-dt:cardinalityRange ;
	mms-ontology:key "ownedAttributeIds" ;
	rdfs:label "ownedAttributeFromDataType" ;
	rdfs:comment "A Property that is the ownedAttribute of this DataType. Based on the UML property 'DataType-ownedAttribute' which is described as: The attributes owned by the DataType."@en ;
	rdfs:domain uml-class:DataType ;
	rdfs:range uml-class:Property ;
	mms-ontology:umlPropertySource uml-property:DataType-ownedAttribute .

mms-property:ownedAttributeFromArtifact a mms-ontology:UmlObjectProperty ;
	mms-ontology:cardinality "*"^^uml-model-dt:cardinalityRange ;
	mms-ontology:key "ownedAttributeIds" ;
	rdfs:label "ownedAttributeFromArtifact" ;
	rdfs:comment "A Property that is the ownedAttribute of this Artifact. Based on the UML property 'Artifact-ownedAttribute' which is described as: The attributes or association ends defined for the Artifact. The association is a specialization of the ownedMember association."@en ;
	rdfs:domain uml-class:Artifact ;
	rdfs:range uml-class:Property ;
	mms-ontology:umlPropertySource uml-property:Artifact-ownedAttribute .

mms-property:ownedAttributeFromInterface a mms-ontology:UmlObjectProperty ;
	mms-ontology:cardinality "*"^^uml-model-dt:cardinalityRange ;
	mms-ontology:key "ownedAttributeIds" ;
	rdfs:label "ownedAttributeFromInterface" ;
	rdfs:comment "A Property that is the ownedAttribute of this Interface. Based on the UML property 'Interface-ownedAttribute' which is described as: The attributes (i.e., the Properties) owned by the Interface."@en ;
	rdfs:domain uml-class:Interface ;
	rdfs:range uml-class:Property ;
	mms-ontology:umlPropertySource uml-property:Interface-ownedAttribute .

mms-property:ownedAttributeFromStructuredClassifier a mms-ontology:UmlObjectProperty ;
	mms-ontology:cardinality "*"^^uml-model-dt:cardinalityRange ;
	mms-ontology:key "ownedAttributeIds" ;
	rdfs:label "ownedAttributeFromStructuredClassifier" ;
	rdfs:comment "A Property that is the ownedAttribute of this StructuredClassifier. Based on the UML property 'StructuredClassifier-ownedAttribute' which is described as: The Properties owned by the StructuredClassifier."@en ;
	rdfs:domain uml-class:StructuredClassifier ;
	rdfs:range uml-class:Property ;
	mms-ontology:umlPropertySource uml-property:StructuredClassifier-ownedAttribute .

mms-property:inputElement a mms-ontology:UmlObjectProperty ;
	mms-ontology:cardinality "*"^^uml-model-dt:cardinalityRange ;
	mms-ontology:key "inputElementIds" ;
	rdfs:label "inputElement" ;
	rdfs:comment "A ExpansionNode that is the inputElement of this ExpansionRegion. Based on the UML property 'ExpansionRegion-inputElement' which is described as: The ExpansionNodes that hold the input collections for the ExpansionRegion."@en ;
	rdfs:domain uml-class:ExpansionRegion ;
	rdfs:range uml-class:ExpansionNode ;
	mms-ontology:umlPropertySource uml-property:ExpansionRegion-inputElement .

mms-property:minintValueSpecification a mms-ontology:UmlObjectProperty ;
	mms-ontology:cardinality "1"^^uml-model-dt:cardinalityRange ;
	mms-ontology:key "minintId" ;
	rdfs:label "minintValueSpecification" ;
	rdfs:comment "The ValueSpecification that is the minint of this InteractionConstraint. Based on the UML property 'InteractionConstraint-minint' which is described as: The minimum number of iterations of a loop"@en ;
	rdfs:domain uml-class:InteractionConstraint ;
	rdfs:range uml-class:ValueSpecification ;
	mms-ontology:umlPropertySource uml-property:InteractionConstraint-minint .

mms-property:parameterFromParameterSet a mms-ontology:UmlObjectProperty ;
	mms-ontology:cardinality "*"^^uml-model-dt:cardinalityRange ;
	mms-ontology:key "parameterIds" ;
	rdfs:label "parameterFromParameterSet" ;
	rdfs:comment "A Parameter that belongs to this ParameterSet. Based on the UML property 'ParameterSet-parameter' which is described as: Parameters in the ParameterSet."@en ;
	rdfs:domain uml-class:ParameterSet ;
	rdfs:range uml-class:Parameter ;
	mms-ontology:umlPropertySource uml-property:ParameterSet-parameter .

mms-property:parameterFromActivityParameterNode a mms-ontology:UmlObjectProperty ;
	mms-ontology:cardinality "1"^^uml-model-dt:cardinalityRange ;
	mms-ontology:key "parameterId" ;
	rdfs:label "parameterFromActivityParameterNode" ;
	rdfs:comment "The Parameter that belongs to this ActivityParameterNode. Based on the UML property 'ActivityParameterNode-parameter' which is described as: The Parameter for which the ActivityParameterNode will be accepting or providing values."@en ;
	rdfs:domain uml-class:ActivityParameterNode ;
	rdfs:range uml-class:Parameter ;
	mms-ontology:umlPropertySource uml-property:ActivityParameterNode-parameter .

mms-property:parameterTemplateParameter a mms-ontology:UmlObjectProperty ;
	mms-ontology:cardinality "*"^^uml-model-dt:cardinalityRange ;
	mms-ontology:key "parameterIds" ;
	rdfs:label "parameterTemplateParameter" ;
	rdfs:comment "A TemplateParameter that is the parameter of this TemplateSignature. Based on the UML property 'TemplateSignature-parameter' which is described as: The ordered set of all formal TemplateParameters for this TemplateSignature."@en ;
	rdfs:domain uml-class:TemplateSignature ;
	rdfs:range uml-class:TemplateParameter ;
	mms-ontology:umlPropertySource uml-property:TemplateSignature-parameter .

mms-property:lowerIntegerFromOperation a mms-ontology:UmlDatatypeProperty ;
	mms-ontology:cardinality "1"^^uml-model-dt:cardinalityRange ;
	mms-ontology:key "lowerId" ;
	rdfs:label "lowerIntegerFromOperation" ;
	rdfs:comment "The Integer that is the lower of this Operation. Based on the UML property 'Operation-lower' which is described as: Specifies the lower multiplicity of the return parameter, if present. This information is derived from the return result for this Operation."@en ;
	rdfs:domain uml-class:Operation ;
	rdfs:range xsd:integer ;
	mms-ontology:umlPropertySource uml-property:Operation-lower .

mms-property:lowerIntegerFromExtensionEnd a mms-ontology:UmlDatatypeProperty ;
	mms-ontology:cardinality "1"^^uml-model-dt:cardinalityRange ;
	mms-ontology:key "lowerId" ;
	rdfs:label "lowerIntegerFromExtensionEnd" ;
	rdfs:comment "The Integer that is the lower of this ExtensionEnd. Based on the UML property 'ExtensionEnd-lower' which is described as: This redefinition changes the default multiplicity of association ends, since model elements are usually extended by 0 or 1 instance of the extension stereotype."@en ;
	rdfs:domain uml-class:ExtensionEnd ;
	rdfs:range xsd:integer ;
	mms-ontology:umlPropertySource uml-property:ExtensionEnd-lower .

mms-property:lowerIntegerFromMultiplicityElement a mms-ontology:UmlDatatypeProperty ;
	mms-ontology:cardinality "1"^^uml-model-dt:cardinalityRange ;
	mms-ontology:key "lowerId" ;
	rdfs:label "lowerIntegerFromMultiplicityElement" ;
	rdfs:comment "The Integer that is the lower of this MultiplicityElement. Based on the UML property 'MultiplicityElement-lower' which is described as: The lower bound of the multiplicity interval."@en ;
	rdfs:domain uml-class:MultiplicityElement ;
	rdfs:range xsd:integer ;
	mms-ontology:umlPropertySource uml-property:MultiplicityElement-lower .

mms-property:ownedLiteral a mms-ontology:UmlObjectProperty ;
	mms-ontology:cardinality "*"^^uml-model-dt:cardinalityRange ;
	mms-ontology:key "ownedLiteralIds" ;
	rdfs:label "ownedLiteral" ;
	rdfs:comment "A EnumerationLiteral that is the ownedLiteral of this Enumeration. Based on the UML property 'Enumeration-ownedLiteral' which is described as: The ordered set of literals owned by this Enumeration."@en ;
	rdfs:domain uml-class:Enumeration ;
	rdfs:range uml-class:EnumerationLiteral ;
	mms-ontology:umlPropertySource uml-property:Enumeration-ownedLiteral .

mms-property:behaviorFromCallBehaviorAction a mms-ontology:UmlObjectProperty ;
	mms-ontology:cardinality "1"^^uml-model-dt:cardinalityRange ;
	mms-ontology:key "behaviorId" ;
	rdfs:label "behaviorFromCallBehaviorAction" ;
	rdfs:comment "The Behavior that belongs to this CallBehaviorAction. Based on the UML property 'CallBehaviorAction-behavior' which is described as: The Behavior being invoked."@en ;
	rdfs:domain uml-class:CallBehaviorAction ;
	rdfs:range uml-class:Behavior ;
	mms-ontology:umlPropertySource uml-property:CallBehaviorAction-behavior .

mms-property:behaviorFromBehaviorExecutionSpecification a mms-ontology:UmlObjectProperty ;
	mms-ontology:cardinality "1"^^uml-model-dt:cardinalityRange ;
	mms-ontology:key "behaviorId" ;
	rdfs:label "behaviorFromBehaviorExecutionSpecification" ;
	rdfs:comment "The Behavior that belongs to this BehaviorExecutionSpecification. Based on the UML property 'BehaviorExecutionSpecification-behavior' which is described as: Behavior whose execution is occurring."@en ;
	rdfs:domain uml-class:BehaviorExecutionSpecification ;
	rdfs:range uml-class:Behavior ;
	mms-ontology:umlPropertySource uml-property:BehaviorExecutionSpecification-behavior .

mms-property:behaviorFromOpaqueExpression a mms-ontology:UmlObjectProperty ;
	mms-ontology:cardinality "1"^^uml-model-dt:cardinalityRange ;
	mms-ontology:key "behaviorId" ;
	rdfs:label "behaviorFromOpaqueExpression" ;
	rdfs:comment "The Behavior that belongs to this OpaqueExpression. Based on the UML property 'OpaqueExpression-behavior' which is described as: Specifies the behavior of the OpaqueExpression as a UML Behavior."@en ;
	rdfs:domain uml-class:OpaqueExpression ;
	rdfs:range uml-class:Behavior ;
	mms-ontology:umlPropertySource uml-property:OpaqueExpression-behavior .

mms-property:coveredLifelineFromOccurrenceSpecification a mms-ontology:UmlObjectProperty ;
	mms-ontology:cardinality "1"^^uml-model-dt:cardinalityRange ;
	mms-ontology:key "coveredId" ;
	rdfs:label "coveredLifelineFromOccurrenceSpecification" ;
	rdfs:comment "The Lifeline that is the covered of this OccurrenceSpecification. Based on the UML property 'OccurrenceSpecification-covered' which is described as: References the Lifeline on which the OccurrenceSpecification appears."@en ;
	rdfs:domain uml-class:OccurrenceSpecification ;
	rdfs:range uml-class:Lifeline ;
	mms-ontology:umlPropertySource uml-property:OccurrenceSpecification-covered .

mms-property:coveredFromInteractionFragment a mms-ontology:UmlObjectProperty ;
	mms-ontology:cardinality "*"^^uml-model-dt:cardinalityRange ;
	mms-ontology:key "coveredIds" ;
	rdfs:label "coveredFromInteractionFragment" ;
	rdfs:comment "A Lifeline that is the covered of this InteractionFragment. Based on the UML property 'InteractionFragment-covered' which is described as: References the Lifelines that the InteractionFragment involves."@en ;
	rdfs:domain uml-class:InteractionFragment ;
	rdfs:range uml-class:Lifeline ;
	mms-ontology:umlPropertySource uml-property:InteractionFragment-covered .

mms-property:coveredLifelineFromStateInvariant a mms-ontology:UmlObjectProperty ;
	mms-ontology:cardinality "1"^^uml-model-dt:cardinalityRange ;
	mms-ontology:key "coveredId" ;
	rdfs:label "coveredLifelineFromStateInvariant" ;
	rdfs:comment "The Lifeline that is the covered of this StateInvariant. Based on the UML property 'StateInvariant-covered' which is described as: References the Lifeline on which the StateInvariant appears."@en ;
	rdfs:domain uml-class:StateInvariant ;
	rdfs:range uml-class:Lifeline ;
	mms-ontology:umlPropertySource uml-property:StateInvariant-covered .

mms-property:associationFromClearAssociationAction a mms-ontology:UmlObjectProperty ;
	mms-ontology:cardinality "1"^^uml-model-dt:cardinalityRange ;
	mms-ontology:key "associationId" ;
	rdfs:label "associationFromClearAssociationAction" ;
	rdfs:comment "The Association that belongs to this ClearAssociationAction. Based on the UML property 'ClearAssociationAction-association' which is described as: The Association to be cleared."@en ;
	rdfs:domain uml-class:ClearAssociationAction ;
	rdfs:range uml-class:Association ;
	mms-ontology:umlPropertySource uml-property:ClearAssociationAction-association .

mms-property:associationFromProperty a mms-ontology:UmlObjectProperty ;
	mms-ontology:cardinality "1"^^uml-model-dt:cardinalityRange ;
	mms-ontology:key "associationId" ;
	rdfs:label "associationFromProperty" ;
	rdfs:comment "The Association that belongs to this Property. Based on the UML property 'Property-association' which is described as: The Association of which this Property is a member, if any."@en ;
	rdfs:domain uml-class:Property ;
	rdfs:range uml-class:Association ;
	mms-ontology:umlPropertySource uml-property:Property-association .

mms-property:feature a mms-ontology:UmlObjectProperty ;
	mms-ontology:cardinality "*"^^uml-model-dt:cardinalityRange ;
	mms-ontology:key "featureIds" ;
	rdfs:label "feature" ;
	rdfs:comment "A Feature that belongs to this Classifier. Based on the UML property 'Classifier-feature' which is described as: Specifies each Feature directly defined in the classifier. Note that there may be members of the Classifier that are of the type Feature but are not included, e.g., inherited features."@en ;
	rdfs:domain uml-class:Classifier ;
	rdfs:range uml-class:Feature ;
	mms-ontology:umlPropertySource uml-property:Classifier-feature .

mms-property:predecessorClause a mms-ontology:UmlObjectProperty ;
	mms-ontology:cardinality "*"^^uml-model-dt:cardinalityRange ;
	mms-ontology:key "predecessorClauseIds" ;
	rdfs:label "predecessorClause" ;
	rdfs:comment "A Clause that belongs to this Clause. Based on the UML property 'Clause-predecessorClause' which is described as: A set of Clauses whose tests must all evaluate to false before this Clause can evaluate its test."@en ;
	rdfs:domain uml-class:Clause ;
	rdfs:range uml-class:Clause ;
	mms-ontology:umlPropertySource uml-property:Clause-predecessorClause .

mms-property:edgeFromStructuredActivityNode a mms-ontology:UmlObjectProperty ;
	mms-ontology:cardinality "*"^^uml-model-dt:cardinalityRange ;
	mms-ontology:key "edgeIds" ;
	rdfs:label "edgeFromStructuredActivityNode" ;
	rdfs:comment "A ActivityEdge that is the edge of this StructuredActivityNode. Based on the UML property 'StructuredActivityNode-edge' which is described as: The ActivityEdges immediately contained in the StructuredActivityNode."@en ;
	rdfs:domain uml-class:StructuredActivityNode ;
	rdfs:range uml-class:ActivityEdge ;
	mms-ontology:umlPropertySource uml-property:StructuredActivityNode-edge .

mms-property:edgeFromActivity a mms-ontology:UmlObjectProperty ;
	mms-ontology:cardinality "*"^^uml-model-dt:cardinalityRange ;
	mms-ontology:key "edgeIds" ;
	rdfs:label "edgeFromActivity" ;
	rdfs:comment "A ActivityEdge that is the edge of this Activity. Based on the UML property 'Activity-edge' which is described as: ActivityEdges expressing flow between the nodes of the Activity."@en ;
	rdfs:domain uml-class:Activity ;
	rdfs:range uml-class:ActivityEdge ;
	mms-ontology:umlPropertySource uml-property:Activity-edge .

mms-property:edgeFromActivityPartition a mms-ontology:UmlObjectProperty ;
	mms-ontology:cardinality "*"^^uml-model-dt:cardinalityRange ;
	mms-ontology:key "edgeIds" ;
	rdfs:label "edgeFromActivityPartition" ;
	rdfs:comment "A ActivityEdge that is the edge of this ActivityPartition. Based on the UML property 'ActivityPartition-edge' which is described as: ActivityEdges immediately contained in the ActivityPartition."@en ;
	rdfs:domain uml-class:ActivityPartition ;
	rdfs:range uml-class:ActivityEdge ;
	mms-ontology:umlPropertySource uml-property:ActivityPartition-edge .

mms-property:applyingPackage a mms-ontology:UmlObjectProperty ;
	mms-ontology:cardinality "1"^^uml-model-dt:cardinalityRange ;
	mms-ontology:key "applyingPackageId" ;
	rdfs:label "applyingPackage" ;
	rdfs:comment "The Package that belongs to this ProfileApplication. Based on the UML property 'ProfileApplication-applyingPackage' which is described as: The package that owns the profile application."@en ;
	rdfs:domain uml-class:ProfileApplication ;
	rdfs:range uml-class:Package ;
	mms-ontology:umlPropertySource uml-property:ProfileApplication-applyingPackage .

mms-property:resultOutputPinFromUnmarshallAction a mms-ontology:UmlObjectProperty ;
	mms-ontology:cardinality "*"^^uml-model-dt:cardinalityRange ;
	mms-ontology:key "resultIds" ;
	rdfs:label "resultOutputPinFromUnmarshallAction" ;
	rdfs:comment "A OutputPin that is the result of this UnmarshallAction. Based on the UML property 'UnmarshallAction-result' which is described as: The OutputPins on which are placed the values of the StructuralFeatures of the input object."@en ;
	rdfs:domain uml-class:UnmarshallAction ;
	rdfs:range uml-class:OutputPin ;
	mms-ontology:umlPropertySource uml-property:UnmarshallAction-result .

mms-property:resultOutputPinFromReadStructuralFeatureAction a mms-ontology:UmlObjectProperty ;
	mms-ontology:cardinality "1"^^uml-model-dt:cardinalityRange ;
	mms-ontology:key "resultId" ;
	rdfs:label "resultOutputPinFromReadStructuralFeatureAction" ;
	rdfs:comment "The OutputPin that is the result of this ReadStructuralFeatureAction. Based on the UML property 'ReadStructuralFeatureAction-result' which is described as: The OutputPin on which the result values are placed."@en ;
	rdfs:domain uml-class:ReadStructuralFeatureAction ;
	rdfs:range uml-class:OutputPin ;
	mms-ontology:umlPropertySource uml-property:ReadStructuralFeatureAction-result .

mms-property:resultOutputPinFromReadVariableAction a mms-ontology:UmlObjectProperty ;
	mms-ontology:cardinality "1"^^uml-model-dt:cardinalityRange ;
	mms-ontology:key "resultId" ;
	rdfs:label "resultOutputPinFromReadVariableAction" ;
	rdfs:comment "The OutputPin that is the result of this ReadVariableAction. Based on the UML property 'ReadVariableAction-result' which is described as: The OutputPin on which the result values are placed."@en ;
	rdfs:domain uml-class:ReadVariableAction ;
	rdfs:range uml-class:OutputPin ;
	mms-ontology:umlPropertySource uml-property:ReadVariableAction-result .

mms-property:resultOutputPinFromValueSpecificationAction a mms-ontology:UmlObjectProperty ;
	mms-ontology:cardinality "1"^^uml-model-dt:cardinalityRange ;
	mms-ontology:key "resultId" ;
	rdfs:label "resultOutputPinFromValueSpecificationAction" ;
	rdfs:comment "The OutputPin that is the result of this ValueSpecificationAction. Based on the UML property 'ValueSpecificationAction-result' which is described as: The OutputPin on which the result value is placed."@en ;
	rdfs:domain uml-class:ValueSpecificationAction ;
	rdfs:range uml-class:OutputPin ;
	mms-ontology:umlPropertySource uml-property:ValueSpecificationAction-result .

mms-property:resultOutputPinFromCallAction a mms-ontology:UmlObjectProperty ;
	mms-ontology:cardinality "*"^^uml-model-dt:cardinalityRange ;
	mms-ontology:key "resultIds" ;
	rdfs:label "resultOutputPinFromCallAction" ;
	rdfs:comment "A OutputPin that is the result of this CallAction. Based on the UML property 'CallAction-result' which is described as: The OutputPins on which the reply values from the invocation are placed (if the call is synchronous)."@en ;
	rdfs:domain uml-class:CallAction ;
	rdfs:range uml-class:OutputPin ;
	mms-ontology:umlPropertySource uml-property:CallAction-result .

mms-property:resultOutputPinFromLoopNode a mms-ontology:UmlObjectProperty ;
	mms-ontology:cardinality "*"^^uml-model-dt:cardinalityRange ;
	mms-ontology:key "resultIds" ;
	rdfs:label "resultOutputPinFromLoopNode" ;
	rdfs:comment "A OutputPin that is the result of this LoopNode. Based on the UML property 'LoopNode-result' which is described as: A list of OutputPins that receive the loopVariable values after the last iteration of the loop and constitute the output of the LoopNode."@en ;
	rdfs:domain uml-class:LoopNode ;
	rdfs:range uml-class:OutputPin ;
	mms-ontology:umlPropertySource uml-property:LoopNode-result .

mms-property:resultOutputPinFromAcceptEventAction a mms-ontology:UmlObjectProperty ;
	mms-ontology:cardinality "*"^^uml-model-dt:cardinalityRange ;
	mms-ontology:key "resultIds" ;
	rdfs:label "resultOutputPinFromAcceptEventAction" ;
	rdfs:comment "A OutputPin that is the result of this AcceptEventAction. Based on the UML property 'AcceptEventAction-result' which is described as: OutputPins holding the values received from an Event occurrence."@en ;
	rdfs:domain uml-class:AcceptEventAction ;
	rdfs:range uml-class:OutputPin ;
	mms-ontology:umlPropertySource uml-property:AcceptEventAction-result .

mms-property:resultOutputPinFromCreateObjectAction a mms-ontology:UmlObjectProperty ;
	mms-ontology:cardinality "1"^^uml-model-dt:cardinalityRange ;
	mms-ontology:key "resultId" ;
	rdfs:label "resultOutputPinFromCreateObjectAction" ;
	rdfs:comment "The OutputPin that is the result of this CreateObjectAction. Based on the UML property 'CreateObjectAction-result' which is described as: The OutputPin on which the newly created object is placed."@en ;
	rdfs:domain uml-class:CreateObjectAction ;
	rdfs:range uml-class:OutputPin ;
	mms-ontology:umlPropertySource uml-property:CreateObjectAction-result .

mms-property:resultOutputPinFromConditionalNode a mms-ontology:UmlObjectProperty ;
	mms-ontology:cardinality "*"^^uml-model-dt:cardinalityRange ;
	mms-ontology:key "resultIds" ;
	rdfs:label "resultOutputPinFromConditionalNode" ;
	rdfs:comment "A OutputPin that is the result of this ConditionalNode. Based on the UML property 'ConditionalNode-result' which is described as: The OutputPins that onto which are moved values from the bodyOutputs of the Clause selected for execution."@en ;
	rdfs:domain uml-class:ConditionalNode ;
	rdfs:range uml-class:OutputPin ;
	mms-ontology:umlPropertySource uml-property:ConditionalNode-result .

mms-property:resultOutputPinFromReadSelfAction a mms-ontology:UmlObjectProperty ;
	mms-ontology:cardinality "1"^^uml-model-dt:cardinalityRange ;
	mms-ontology:key "resultId" ;
	rdfs:label "resultOutputPinFromReadSelfAction" ;
	rdfs:comment "The OutputPin that is the result of this ReadSelfAction. Based on the UML property 'ReadSelfAction-result' which is described as: The OutputPin on which the context object is placed."@en ;
	rdfs:domain uml-class:ReadSelfAction ;
	rdfs:range uml-class:OutputPin ;
	mms-ontology:umlPropertySource uml-property:ReadSelfAction-result .

mms-property:resultOutputPinFromWriteStructuralFeatureAction a mms-ontology:UmlObjectProperty ;
	mms-ontology:cardinality "1"^^uml-model-dt:cardinalityRange ;
	mms-ontology:key "resultId" ;
	rdfs:label "resultOutputPinFromWriteStructuralFeatureAction" ;
	rdfs:comment "The OutputPin that is the result of this WriteStructuralFeatureAction. Based on the UML property 'WriteStructuralFeatureAction-result' which is described as: The OutputPin on which is put the input object as modified by the WriteStructuralFeatureAction."@en ;
	rdfs:domain uml-class:WriteStructuralFeatureAction ;
	rdfs:range uml-class:OutputPin ;
	mms-ontology:umlPropertySource uml-property:WriteStructuralFeatureAction-result .

mms-property:resultOutputPinFromReadLinkObjectEndQualifierAction a mms-ontology:UmlObjectProperty ;
	mms-ontology:cardinality "1"^^uml-model-dt:cardinalityRange ;
	mms-ontology:key "resultId" ;
	rdfs:label "resultOutputPinFromReadLinkObjectEndQualifierAction" ;
	rdfs:comment "The OutputPin that is the result of this ReadLinkObjectEndQualifierAction. Based on the UML property 'ReadLinkObjectEndQualifierAction-result' which is described as: The OutputPin where the result value is placed."@en ;
	rdfs:domain uml-class:ReadLinkObjectEndQualifierAction ;
	rdfs:range uml-class:OutputPin ;
	mms-ontology:umlPropertySource uml-property:ReadLinkObjectEndQualifierAction-result .

mms-property:resultOutputPinFromTestIdentityAction a mms-ontology:UmlObjectProperty ;
	mms-ontology:cardinality "1"^^uml-model-dt:cardinalityRange ;
	mms-ontology:key "resultId" ;
	rdfs:label "resultOutputPinFromTestIdentityAction" ;
	rdfs:comment "The OutputPin that is the result of this TestIdentityAction. Based on the UML property 'TestIdentityAction-result' which is described as: The OutputPin whose Boolean value indicates whether the two input objects are identical."@en ;
	rdfs:domain uml-class:TestIdentityAction ;
	rdfs:range uml-class:OutputPin ;
	mms-ontology:umlPropertySource uml-property:TestIdentityAction-result .

mms-property:resultOutputPinFromReadExtentAction a mms-ontology:UmlObjectProperty ;
	mms-ontology:cardinality "1"^^uml-model-dt:cardinalityRange ;
	mms-ontology:key "resultId" ;
	rdfs:label "resultOutputPinFromReadExtentAction" ;
	rdfs:comment "The OutputPin that is the result of this ReadExtentAction. Based on the UML property 'ReadExtentAction-result' which is described as: The OutputPin on which the Classifier instances are placed."@en ;
	rdfs:domain uml-class:ReadExtentAction ;
	rdfs:range uml-class:OutputPin ;
	mms-ontology:umlPropertySource uml-property:ReadExtentAction-result .

mms-property:resultOutputPinFromCreateLinkObjectAction a mms-ontology:UmlObjectProperty ;
	mms-ontology:cardinality "1"^^uml-model-dt:cardinalityRange ;
	mms-ontology:key "resultId" ;
	rdfs:label "resultOutputPinFromCreateLinkObjectAction" ;
	rdfs:comment "The OutputPin that is the result of this CreateLinkObjectAction. Based on the UML property 'CreateLinkObjectAction-result' which is described as: The output pin on which the newly created link object is placed."@en ;
	rdfs:domain uml-class:CreateLinkObjectAction ;
	rdfs:range uml-class:OutputPin ;
	mms-ontology:umlPropertySource uml-property:CreateLinkObjectAction-result .

mms-property:resultOutputPinFromReduceAction a mms-ontology:UmlObjectProperty ;
	mms-ontology:cardinality "1"^^uml-model-dt:cardinalityRange ;
	mms-ontology:key "resultId" ;
	rdfs:label "resultOutputPinFromReduceAction" ;
	rdfs:comment "The OutputPin that is the result of this ReduceAction. Based on the UML property 'ReduceAction-result' which is described as: The output pin on which the result value is placed."@en ;
	rdfs:domain uml-class:ReduceAction ;
	rdfs:range uml-class:OutputPin ;
	mms-ontology:umlPropertySource uml-property:ReduceAction-result .

mms-property:resultOutputPinFromReadLinkObjectEndAction a mms-ontology:UmlObjectProperty ;
	mms-ontology:cardinality "1"^^uml-model-dt:cardinalityRange ;
	mms-ontology:key "resultId" ;
	rdfs:label "resultOutputPinFromReadLinkObjectEndAction" ;
	rdfs:comment "The OutputPin that is the result of this ReadLinkObjectEndAction. Based on the UML property 'ReadLinkObjectEndAction-result' which is described as: The OutputPin where the result value is placed."@en ;
	rdfs:domain uml-class:ReadLinkObjectEndAction ;
	rdfs:range uml-class:OutputPin ;
	mms-ontology:umlPropertySource uml-property:ReadLinkObjectEndAction-result .

mms-property:resultOutputPinFromReadIsClassifiedObjectAction a mms-ontology:UmlObjectProperty ;
	mms-ontology:cardinality "1"^^uml-model-dt:cardinalityRange ;
	mms-ontology:key "resultId" ;
	rdfs:label "resultOutputPinFromReadIsClassifiedObjectAction" ;
	rdfs:comment "The OutputPin that is the result of this ReadIsClassifiedObjectAction. Based on the UML property 'ReadIsClassifiedObjectAction-result' which is described as: The OutputPin that holds the Boolean result of the test."@en ;
	rdfs:domain uml-class:ReadIsClassifiedObjectAction ;
	rdfs:range uml-class:OutputPin ;
	mms-ontology:umlPropertySource uml-property:ReadIsClassifiedObjectAction-result .

mms-property:resultOutputPinFromClearStructuralFeatureAction a mms-ontology:UmlObjectProperty ;
	mms-ontology:cardinality "1"^^uml-model-dt:cardinalityRange ;
	mms-ontology:key "resultId" ;
	rdfs:label "resultOutputPinFromClearStructuralFeatureAction" ;
	rdfs:comment "The OutputPin that is the result of this ClearStructuralFeatureAction. Based on the UML property 'ClearStructuralFeatureAction-result' which is described as: The OutputPin on which is put the input object as modified by the ClearStructuralFeatureAction."@en ;
	rdfs:domain uml-class:ClearStructuralFeatureAction ;
	rdfs:range uml-class:OutputPin ;
	mms-ontology:umlPropertySource uml-property:ClearStructuralFeatureAction-result .

mms-property:resultOutputPinFromReadLinkAction a mms-ontology:UmlObjectProperty ;
	mms-ontology:cardinality "1"^^uml-model-dt:cardinalityRange ;
	mms-ontology:key "resultId" ;
	rdfs:label "resultOutputPinFromReadLinkAction" ;
	rdfs:comment "The OutputPin that is the result of this ReadLinkAction. Based on the UML property 'ReadLinkAction-result' which is described as: The OutputPin on which the objects retrieved from the &#34;open&#34; end of those links whose values on other ends are given by the endData."@en ;
	rdfs:domain uml-class:ReadLinkAction ;
	rdfs:range uml-class:OutputPin ;
	mms-ontology:umlPropertySource uml-property:ReadLinkAction-result .

mms-property:resultParameter a mms-ontology:UmlObjectProperty ;
	mms-ontology:cardinality "1"^^uml-model-dt:cardinalityRange ;
	mms-ontology:key "resultId" ;
	rdfs:label "resultParameter" ;
	rdfs:comment "The Parameter that is the result of this OpaqueExpression. Based on the UML property 'OpaqueExpression-result' which is described as: If an OpaqueExpression is specified using a UML Behavior, then this refers to the single required return Parameter of that Behavior. When the Behavior completes execution, the values on this Parameter give the result of evaluating the OpaqueExpression."@en ;
	rdfs:domain uml-class:OpaqueExpression ;
	rdfs:range uml-class:Parameter ;
	mms-ontology:umlPropertySource uml-property:OpaqueExpression-result .

mms-property:classFromOperation a mms-ontology:UmlObjectProperty ;
	mms-ontology:cardinality "1"^^uml-model-dt:cardinalityRange ;
	mms-ontology:key "classId" ;
	rdfs:label "classFromOperation" ;
	rdfs:comment "The Class that belongs to this Operation. Based on the UML property 'Operation-class' which is described as: The Class that owns this operation, if any."@en ;
	rdfs:domain uml-class:Operation ;
	rdfs:range uml-class:Class ;
	mms-ontology:umlPropertySource uml-property:Operation-class .

mms-property:classFromProperty a mms-ontology:UmlObjectProperty ;
	mms-ontology:cardinality "1"^^uml-model-dt:cardinalityRange ;
	mms-ontology:key "classId" ;
	rdfs:label "classFromProperty" ;
	rdfs:comment "The Class that belongs to this Property. Based on the UML property 'Property-class' which is described as: The Class that owns this Property, if any."@en ;
	rdfs:domain uml-class:Property ;
	rdfs:range uml-class:Class ;
	mms-ontology:umlPropertySource uml-property:Property-class .

mms-property:ownedElement a mms-ontology:UmlObjectProperty ;
	mms-ontology:cardinality "*"^^uml-model-dt:cardinalityRange ;
	mms-ontology:key "ownedElementIds" ;
	rdfs:label "ownedElement" ;
	rdfs:comment "A Element that belongs to this Element. Based on the UML property 'Element-ownedElement' which is described as: The Elements owned by this Element."@en ;
	rdfs:domain uml-class:Element ;
	rdfs:range uml-class:Element ;
	mms-ontology:umlPropertySource uml-property:Element-ownedElement .

mms-property:redefinedProperty a mms-ontology:UmlObjectProperty ;
	mms-ontology:cardinality "*"^^uml-model-dt:cardinalityRange ;
	mms-ontology:key "redefinedPropertyIds" ;
	rdfs:label "redefinedProperty" ;
	rdfs:comment "A Property that belongs to this Property. Based on the UML property 'Property-redefinedProperty' which is described as: The properties that are redefined by this property, if any."@en ;
	rdfs:domain uml-class:Property ;
	rdfs:range uml-class:Property ;
	mms-ontology:umlPropertySource uml-property:Property-redefinedProperty .

mms-property:redefinitionContextClassifierFromVertex a mms-ontology:UmlObjectProperty ;
	mms-ontology:cardinality "1"^^uml-model-dt:cardinalityRange ;
	mms-ontology:key "redefinitionContextId" ;
	rdfs:label "redefinitionContextClassifierFromVertex" ;
	rdfs:comment "The Classifier that is the redefinitionContext of this Vertex. Based on the UML property 'State-redefinitionContext' which is described as: References the Classifier in which context this element may be redefined."@en ;
	rdfs:domain uml-class:Vertex ;
	rdfs:range uml-class:Classifier ;
	mms-ontology:umlPropertySource uml-property:State-redefinitionContext .

mms-property:redefinitionContextClassifierFromRegion a mms-ontology:UmlObjectProperty ;
	mms-ontology:cardinality "1"^^uml-model-dt:cardinalityRange ;
	mms-ontology:key "redefinitionContextId" ;
	rdfs:label "redefinitionContextClassifierFromRegion" ;
	rdfs:comment "The Classifier that is the redefinitionContext of this Region. Based on the UML property 'Region-redefinitionContext' which is described as: References the Classifier in which context this element may be redefined."@en ;
	rdfs:domain uml-class:Region ;
	rdfs:range uml-class:Classifier ;
	mms-ontology:umlPropertySource uml-property:Region-redefinitionContext .

mms-property:redefinitionContextClassifierFromTransition a mms-ontology:UmlObjectProperty ;
	mms-ontology:cardinality "1"^^uml-model-dt:cardinalityRange ;
	mms-ontology:key "redefinitionContextId" ;
	rdfs:label "redefinitionContextClassifierFromTransition" ;
	rdfs:comment "The Classifier that is the redefinitionContext of this Transition. Based on the UML property 'Transition-redefinitionContext' which is described as: References the Classifier in which context this element may be redefined."@en ;
	rdfs:domain uml-class:Transition ;
	rdfs:range uml-class:Classifier ;
	mms-ontology:umlPropertySource uml-property:Transition-redefinitionContext .

mms-property:redefinitionContextFromRedefinableElement a mms-ontology:UmlObjectProperty ;
	mms-ontology:cardinality "*"^^uml-model-dt:cardinalityRange ;
	mms-ontology:key "redefinitionContextIds" ;
	rdfs:label "redefinitionContextFromRedefinableElement" ;
	rdfs:comment "A Classifier that is the redefinitionContext of this RedefinableElement. Based on the UML property 'RedefinableElement-redefinitionContext' which is described as: The contexts that this element may be redefined from."@en ;
	rdfs:domain uml-class:RedefinableElement ;
	rdfs:range uml-class:Classifier ;
	mms-ontology:umlPropertySource uml-property:RedefinableElement-redefinitionContext .

mms-property:roleBinding a mms-ontology:UmlObjectProperty ;
	mms-ontology:cardinality "*"^^uml-model-dt:cardinalityRange ;
	mms-ontology:key "roleBindingIds" ;
	rdfs:label "roleBinding" ;
	rdfs:comment "A Dependency that is the roleBinding of this CollaborationUse. Based on the UML property 'CollaborationUse-roleBinding' which is described as: A mapping between features of the Collaboration and features of the owning Classifier. This mapping indicates which ConnectableElement of the Classifier plays which role(s) in the Collaboration. A ConnectableElement may be bound to multiple roles in the same CollaborationUse (that is, it may play multiple roles)."@en ;
	rdfs:domain uml-class:CollaborationUse ;
	rdfs:range uml-class:Dependency ;
	mms-ontology:umlPropertySource uml-property:CollaborationUse-roleBinding .

mms-property:defaultString a mms-ontology:UmlDatatypeProperty ;
	mms-ontology:cardinality "1"^^uml-model-dt:cardinalityRange ;
	mms-ontology:key "defaultId" ;
	rdfs:label "defaultString" ;
	rdfs:comment "The String that is the default of this Parameter. Based on the UML property 'Parameter-default' which is described as: A String that represents a value to be used when no argument is supplied for the Parameter."@en ;
	rdfs:domain uml-class:Parameter ;
	rdfs:range xsd:string ;
	mms-ontology:umlPropertySource uml-property:Parameter-default .

mms-property:defaultParameterableElement a mms-ontology:UmlObjectProperty ;
	mms-ontology:cardinality "1"^^uml-model-dt:cardinalityRange ;
	mms-ontology:key "defaultId" ;
	rdfs:label "defaultParameterableElement" ;
	rdfs:comment "The ParameterableElement that is the default of this TemplateParameter. Based on the UML property 'TemplateParameter-default' which is described as: The ParameterableElement that is the default for this formal TemplateParameter."@en ;
	rdfs:domain uml-class:TemplateParameter ;
	rdfs:range uml-class:ParameterableElement ;
	mms-ontology:umlPropertySource uml-property:TemplateParameter-default .

mms-property:isSimple a mms-ontology:UmlDatatypeProperty ;
	mms-ontology:key "isSimple" ;
	rdfs:label "isSimple" ;
	rdfs:comment "A State with isSimple=true is said to be a simple State A simple State does not have any Regions and it does not refer to any submachine StateMachine."@en ;
	rdfs:domain uml-class:State ;
	rdfs:range xsd:boolean ;
	mms-ontology:umlPropertySource uml-property:State-isSimple .

mms-property:isSimpleState a mms-ontology:UmlDatatypeProperty ;
	owl:equivalentProperty mms-property:isSimple .

mms-property:redefinedEdge a mms-ontology:UmlObjectProperty ;
	mms-ontology:cardinality "*"^^uml-model-dt:cardinalityRange ;
	mms-ontology:key "redefinedEdgeIds" ;
	rdfs:label "redefinedEdge" ;
	rdfs:comment "A ActivityEdge that is the redefinedEdge of this ActivityEdge. Based on the UML property 'ActivityEdge-redefinedEdge' which is described as: ActivityEdges from a generalization of the Activity containing this ActivityEdge that are redefined by this ActivityEdge."@en ;
	rdfs:domain uml-class:ActivityEdge ;
	rdfs:range uml-class:ActivityEdge ;
	mms-ontology:umlPropertySource uml-property:ActivityEdge-redefinedEdge .

mms-property:afterOccurrenceSpecification a mms-ontology:UmlObjectProperty ;
	mms-ontology:cardinality "1"^^uml-model-dt:cardinalityRange ;
	mms-ontology:key "afterId" ;
	rdfs:label "afterOccurrenceSpecification" ;
	rdfs:comment "The OccurrenceSpecification that is the after of this GeneralOrdering. Based on the UML property 'GeneralOrdering-after' which is described as: The OccurrenceSpecification referenced comes after the OccurrenceSpecification referenced by before."@en ;
	rdfs:domain uml-class:GeneralOrdering ;
	rdfs:range uml-class:OccurrenceSpecification ;
	mms-ontology:umlPropertySource uml-property:GeneralOrdering-after .

mms-property:exceptionInputPin a mms-ontology:UmlObjectProperty ;
	mms-ontology:cardinality "1"^^uml-model-dt:cardinalityRange ;
	mms-ontology:key "exceptionId" ;
	rdfs:label "exceptionInputPin" ;
	rdfs:comment "The InputPin that is the exception of this RaiseExceptionAction. Based on the UML property 'RaiseExceptionAction-exception' which is described as: An InputPin whose value becomes the exception object."@en ;
	rdfs:domain uml-class:RaiseExceptionAction ;
	rdfs:range uml-class:InputPin ;
	mms-ontology:umlPropertySource uml-property:RaiseExceptionAction-exception .

mms-property:upperUnlimitedNaturalFromOperation a mms-ontology:UmlDatatypeProperty ;
	mms-ontology:cardinality "1"^^uml-model-dt:cardinalityRange ;
	mms-ontology:key "upperId" ;
	rdfs:label "upperUnlimitedNaturalFromOperation" ;
	rdfs:comment "The UnlimitedNatural that is the upper of this Operation. Based on the UML property 'Operation-upper' which is described as: The upper multiplicity of the return parameter, if present. This information is derived from the return result for this Operation."@en ;
	rdfs:domain uml-class:Operation ;
	rdfs:range xsd:string ;
	mms-ontology:umlPropertySource uml-property:Operation-upper .

mms-property:upperUnlimitedNaturalFromMultiplicityElement a mms-ontology:UmlDatatypeProperty ;
	mms-ontology:cardinality "1"^^uml-model-dt:cardinalityRange ;
	mms-ontology:key "upperId" ;
	rdfs:label "upperUnlimitedNaturalFromMultiplicityElement" ;
	rdfs:comment "The UnlimitedNatural that is the upper of this MultiplicityElement. Based on the UML property 'MultiplicityElement-upper' which is described as: The upper bound of the multiplicity interval."@en ;
	rdfs:domain uml-class:MultiplicityElement ;
	rdfs:range xsd:string ;
	mms-ontology:umlPropertySource uml-property:MultiplicityElement-upper .

mms-property:observationFromTimeExpression a mms-ontology:UmlObjectProperty ;
	mms-ontology:cardinality "*"^^uml-model-dt:cardinalityRange ;
	mms-ontology:key "observationIds" ;
	rdfs:label "observationFromTimeExpression" ;
	rdfs:comment "A Observation that belongs to this TimeExpression. Based on the UML property 'TimeExpression-observation' which is described as: Refers to the Observations that are involved in the computation of the TimeExpression value."@en ;
	rdfs:domain uml-class:TimeExpression ;
	rdfs:range uml-class:Observation ;
	mms-ontology:umlPropertySource uml-property:TimeExpression-observation .

mms-property:observationFromDuration a mms-ontology:UmlObjectProperty ;
	mms-ontology:cardinality "*"^^uml-model-dt:cardinalityRange ;
	mms-ontology:key "observationIds" ;
	rdfs:label "observationFromDuration" ;
	rdfs:comment "A Observation that belongs to this Duration. Based on the UML property 'Duration-observation' which is described as: Refers to the Observations that are involved in the computation of the Duration value"@en ;
	rdfs:domain uml-class:Duration ;
	rdfs:range uml-class:Observation ;
	mms-ontology:umlPropertySource uml-property:Duration-observation .

mms-property:actualGate a mms-ontology:UmlObjectProperty ;
	mms-ontology:cardinality "*"^^uml-model-dt:cardinalityRange ;
	mms-ontology:key "actualGateIds" ;
	rdfs:label "actualGate" ;
	rdfs:comment "A Gate that belongs to this InteractionUse. Based on the UML property 'InteractionUse-actualGate' which is described as: The actual gates of the InteractionUse."@en ;
	rdfs:domain uml-class:InteractionUse ;
	rdfs:range uml-class:Gate ;
	mms-ontology:umlPropertySource uml-property:InteractionUse-actualGate .

mms-property:signalFromReception a mms-ontology:UmlObjectProperty ;
	mms-ontology:cardinality "1"^^uml-model-dt:cardinalityRange ;
	mms-ontology:key "signalId" ;
	rdfs:label "signalFromReception" ;
	rdfs:comment "The Signal that belongs to this Reception. Based on the UML property 'Reception-signal' which is described as: The Signal that this Reception handles."@en ;
	rdfs:domain uml-class:Reception ;
	rdfs:range uml-class:Signal ;
	mms-ontology:umlPropertySource uml-property:Reception-signal .

mms-property:signalFromBroadcastSignalAction a mms-ontology:UmlObjectProperty ;
	mms-ontology:cardinality "1"^^uml-model-dt:cardinalityRange ;
	mms-ontology:key "signalId" ;
	rdfs:label "signalFromBroadcastSignalAction" ;
	rdfs:comment "The Signal that belongs to this BroadcastSignalAction. Based on the UML property 'BroadcastSignalAction-signal' which is described as: The Signal whose instances are to be sent."@en ;
	rdfs:domain uml-class:BroadcastSignalAction ;
	rdfs:range uml-class:Signal ;
	mms-ontology:umlPropertySource uml-property:BroadcastSignalAction-signal .

mms-property:signalFromSignalEvent a mms-ontology:UmlObjectProperty ;
	mms-ontology:cardinality "1"^^uml-model-dt:cardinalityRange ;
	mms-ontology:key "signalId" ;
	rdfs:label "signalFromSignalEvent" ;
	rdfs:comment "The Signal that belongs to this SignalEvent. Based on the UML property 'SignalEvent-signal' which is described as: The specific Signal that is associated with this SignalEvent."@en ;
	rdfs:domain uml-class:SignalEvent ;
	rdfs:range uml-class:Signal ;
	mms-ontology:umlPropertySource uml-property:SignalEvent-signal .

mms-property:signalFromSendSignalAction a mms-ontology:UmlObjectProperty ;
	mms-ontology:cardinality "1"^^uml-model-dt:cardinalityRange ;
	mms-ontology:key "signalId" ;
	rdfs:label "signalFromSendSignalAction" ;
	rdfs:comment "The Signal that belongs to this SendSignalAction. Based on the UML property 'SendSignalAction-signal' which is described as: The Signal whose instance is transmitted to the target."@en ;
	rdfs:domain uml-class:SendSignalAction ;
	rdfs:range uml-class:Signal ;
	mms-ontology:umlPropertySource uml-property:SendSignalAction-signal .

mms-property:isUniqueOperation a mms-ontology:UmlDatatypeProperty ;
	mms-ontology:key "isUnique" ;
	rdfs:label "isUniqueOperation" ;
	rdfs:comment "Specifies whether the return parameter is unique or not, if present. This information is derived from the return result for this Operation."@en ;
	rdfs:domain uml-class:Operation ;
	rdfs:range xsd:boolean ;
	mms-ontology:umlPropertySource uml-property:Operation-isUnique .

mms-property:isUniqueMultiplicityElement a mms-ontology:UmlDatatypeProperty ;
	mms-ontology:key "isUnique" ;
	rdfs:label "isUniqueMultiplicityElement" ;
	rdfs:comment "For a multivalued multiplicity, this attributes specifies whether the values in an instantiation of this MultiplicityElement are unique."@en ;
	rdfs:domain uml-class:MultiplicityElement ;
	rdfs:range xsd:boolean ;
	mms-ontology:umlPropertySource uml-property:MultiplicityElement-isUnique .

mms-property:ownedParameterFromOperation a mms-ontology:UmlObjectProperty ;
	mms-ontology:cardinality "*"^^uml-model-dt:cardinalityRange ;
	mms-ontology:key "ownedParameterIds" ;
	rdfs:label "ownedParameterFromOperation" ;
	rdfs:comment "A Parameter that belongs to this Operation. Based on the UML property 'Operation-ownedParameter' which is described as: The parameters owned by this Operation."@en ;
	rdfs:domain uml-class:Operation ;
	rdfs:range uml-class:Parameter ;
	mms-ontology:umlPropertySource uml-property:Operation-ownedParameter .

mms-property:ownedParameterFromBehavior a mms-ontology:UmlObjectProperty ;
	mms-ontology:cardinality "*"^^uml-model-dt:cardinalityRange ;
	mms-ontology:key "ownedParameterIds" ;
	rdfs:label "ownedParameterFromBehavior" ;
	rdfs:comment "A Parameter that belongs to this Behavior. Based on the UML property 'Behavior-ownedParameter' which is described as: References a list of Parameters to the Behavior which describes the order and type of arguments that can be given when the Behavior is invoked and of the values which will be returned when the Behavior completes its execution."@en ;
	rdfs:domain uml-class:Behavior ;
	rdfs:range uml-class:Parameter ;
	mms-ontology:umlPropertySource uml-property:Behavior-ownedParameter .

mms-property:ownedParameterFromBehavioralFeature a mms-ontology:UmlObjectProperty ;
	mms-ontology:cardinality "*"^^uml-model-dt:cardinalityRange ;
	mms-ontology:key "ownedParameterIds" ;
	rdfs:label "ownedParameterFromBehavioralFeature" ;
	rdfs:comment "A Parameter that belongs to this BehavioralFeature. Based on the UML property 'BehavioralFeature-ownedParameter' which is described as: The ordered set of formal Parameters of this BehavioralFeature."@en ;
	rdfs:domain uml-class:BehavioralFeature ;
	rdfs:range uml-class:Parameter ;
	mms-ontology:umlPropertySource uml-property:BehavioralFeature-ownedParameter .

mms-property:ownedParameterTemplateParameter a mms-ontology:UmlObjectProperty ;
	mms-ontology:cardinality "*"^^uml-model-dt:cardinalityRange ;
	mms-ontology:key "ownedParameterIds" ;
	rdfs:label "ownedParameterTemplateParameter" ;
	rdfs:comment "A TemplateParameter that is the ownedParameter of this TemplateSignature. Based on the UML property 'TemplateSignature-ownedParameter' which is described as: The formal parameters that are owned by this TemplateSignature."@en ;
	rdfs:domain uml-class:TemplateSignature ;
	rdfs:range uml-class:TemplateParameter ;
	mms-ontology:umlPropertySource uml-property:TemplateSignature-ownedParameter .

mms-property:preconditionFromBehavior a mms-ontology:UmlObjectProperty ;
	mms-ontology:cardinality "*"^^uml-model-dt:cardinalityRange ;
	mms-ontology:key "preconditionIds" ;
	rdfs:label "preconditionFromBehavior" ;
	rdfs:comment "A Constraint that is the precondition of this Behavior. Based on the UML property 'Behavior-precondition' which is described as: An optional set of Constraints specifying what must be fulfilled before the Behavior is invoked."@en ;
	rdfs:domain uml-class:Behavior ;
	rdfs:range uml-class:Constraint ;
	mms-ontology:umlPropertySource uml-property:Behavior-precondition .

mms-property:preconditionFromOperation a mms-ontology:UmlObjectProperty ;
	mms-ontology:cardinality "*"^^uml-model-dt:cardinalityRange ;
	mms-ontology:key "preconditionIds" ;
	rdfs:label "preconditionFromOperation" ;
	rdfs:comment "A Constraint that is the precondition of this Operation. Based on the UML property 'Operation-precondition' which is described as: An optional set of Constraints on the state of the system when the Operation is invoked."@en ;
	rdfs:domain uml-class:Operation ;
	rdfs:range uml-class:Constraint ;
	mms-ontology:umlPropertySource uml-property:Operation-precondition .

mms-property:isOrderedMultiplicityElement a mms-ontology:UmlDatatypeProperty ;
	mms-ontology:key "isOrdered" ;
	rdfs:label "isOrderedMultiplicityElement" ;
	rdfs:comment "For a multivalued multiplicity, this attribute specifies whether the values in an instantiation of this MultiplicityElement are sequentially ordered."@en ;
	rdfs:domain uml-class:MultiplicityElement ;
	rdfs:range xsd:boolean ;
	mms-ontology:umlPropertySource uml-property:MultiplicityElement-isOrdered .

mms-property:isOrderedReduceAction a mms-ontology:UmlDatatypeProperty ;
	mms-ontology:key "isOrdered" ;
	rdfs:label "isOrderedReduceAction" ;
	rdfs:comment "Indicates whether the order of the input collection should determine the order in which the reducer Behavior is applied to its elements."@en ;
	rdfs:domain uml-class:ReduceAction ;
	rdfs:range xsd:boolean ;
	mms-ontology:umlPropertySource uml-property:ReduceAction-isOrdered .

mms-property:isOrderedOperation a mms-ontology:UmlDatatypeProperty ;
	mms-ontology:key "isOrdered" ;
	rdfs:label "isOrderedOperation" ;
	rdfs:comment "Specifies whether the return parameter is ordered or not, if present.  This information is derived from the return result for this Operation."@en ;
	rdfs:domain uml-class:Operation ;
	rdfs:range xsd:boolean ;
	mms-ontology:umlPropertySource uml-property:Operation-isOrdered .

mms-property:languageFromOpaqueAction a mms-ontology:UmlDatatypeProperty ;
	mms-ontology:cardinality "*"^^uml-model-dt:cardinalityRange ;
	mms-ontology:key "languageIds" ;
	rdfs:label "languageFromOpaqueAction" ;
	rdfs:comment "A String that is the language of this OpaqueAction. Based on the UML property 'OpaqueAction-language' which is described as: If provided, a specification of the language used for each of the body Strings."@en ;
	rdfs:domain uml-class:OpaqueAction ;
	rdfs:range xsd:string ;
	mms-ontology:umlPropertySource uml-property:OpaqueAction-language .

mms-property:languageFromOpaqueBehavior a mms-ontology:UmlDatatypeProperty ;
	mms-ontology:cardinality "*"^^uml-model-dt:cardinalityRange ;
	mms-ontology:key "languageIds" ;
	rdfs:label "languageFromOpaqueBehavior" ;
	rdfs:comment "A String that is the language of this OpaqueBehavior. Based on the UML property 'OpaqueBehavior-language' which is described as: Languages the body strings use in the same order as the body strings."@en ;
	rdfs:domain uml-class:OpaqueBehavior ;
	rdfs:range xsd:string ;
	mms-ontology:umlPropertySource uml-property:OpaqueBehavior-language .

mms-property:languageFromOpaqueExpression a mms-ontology:UmlDatatypeProperty ;
	mms-ontology:cardinality "*"^^uml-model-dt:cardinalityRange ;
	mms-ontology:key "languageIds" ;
	rdfs:label "languageFromOpaqueExpression" ;
	rdfs:comment "A String that is the language of this OpaqueExpression. Based on the UML property 'OpaqueExpression-language' which is described as: Specifies the languages used to express the textual bodies of the OpaqueExpression.  Languages are matched to body Strings by order. The interpretation of the body depends on the languages. If the languages are unspecified, they may be implicit from the expression body or the context."@en ;
	rdfs:domain uml-class:OpaqueExpression ;
	rdfs:range xsd:string ;
	mms-ontology:umlPropertySource uml-property:OpaqueExpression-language .

mms-property:isRequired a mms-ontology:UmlDatatypeProperty ;
	mms-ontology:key "isRequired" ;
	rdfs:label "isRequired" ;
	rdfs:comment "Indicates whether an instance of the extending stereotype must be created when an instance of the extended class is created. The attribute value is derived from the value of the lower property of the ExtensionEnd referenced by Extension::ownedEnd; a lower value of 1 means that isRequired is true, but otherwise it is false. Since the default value of ExtensionEnd::lower is 0, the default value of isRequired is false."@en ;
	rdfs:domain uml-class:Extension ;
	rdfs:range xsd:boolean ;
	mms-ontology:umlPropertySource uml-property:Extension-isRequired .

mms-property:isRequiredExtension a mms-ontology:UmlDatatypeProperty ;
	owl:equivalentProperty mms-property:isRequired .

mms-property:executableNode a mms-ontology:UmlObjectProperty ;
	mms-ontology:cardinality "*"^^uml-model-dt:cardinalityRange ;
	mms-ontology:key "executableNodeIds" ;
	rdfs:label "executableNode" ;
	rdfs:comment "A ExecutableNode that belongs to this SequenceNode. Based on the UML property 'SequenceNode-executableNode' which is described as: The ordered set of ExecutableNodes to be sequenced."@en ;
	rdfs:domain uml-class:SequenceNode ;
	rdfs:range uml-class:ExecutableNode ;
	mms-ontology:umlPropertySource uml-property:SequenceNode-executableNode .

mms-property:isIndirectlyInstantiated a mms-ontology:UmlDatatypeProperty ;
	mms-ontology:key "isIndirectlyInstantiated" ;
	rdfs:label "isIndirectlyInstantiated" ;
	rdfs:comment "If true, the Component is defined at design-time, but at run-time (or execution-time) an object specified by the Component does not exist, that is, the Component is instantiated indirectly, through the instantiation of its realizing Classifiers or parts."@en ;
	rdfs:domain uml-class:Component ;
	rdfs:range xsd:boolean ;
	mms-ontology:umlPropertySource uml-property:Component-isIndirectlyInstantiated .

mms-property:isIndirectlyInstantiatedComponent a mms-ontology:UmlDatatypeProperty ;
	owl:equivalentProperty mms-property:isIndirectlyInstantiated .

mms-property:oppositeProperty a mms-ontology:UmlObjectProperty ;
	mms-ontology:cardinality "1"^^uml-model-dt:cardinalityRange ;
	mms-ontology:key "oppositeId" ;
	rdfs:label "oppositeProperty" ;
	rdfs:comment "The Property that is the opposite of this Property. Based on the UML property 'Property-opposite' which is described as: In the case where the Property is one end of a binary association this gives the other end."@en ;
	rdfs:domain uml-class:Property ;
	rdfs:range uml-class:Property ;
	mms-ontology:umlPropertySource uml-property:Property-opposite .

mms-property:deploymentLocationString a mms-ontology:UmlDatatypeProperty ;
	mms-ontology:cardinality "1"^^uml-model-dt:cardinalityRange ;
	mms-ontology:key "deploymentLocationId" ;
	rdfs:label "deploymentLocationString" ;
	rdfs:comment "The String that is the deploymentLocation of this DeploymentSpecification. Based on the UML property 'DeploymentSpecification-deploymentLocation' which is described as: The location where an Artifact is deployed onto a Node. This is typically a 'directory' or 'memory address.'"@en ;
	rdfs:domain uml-class:DeploymentSpecification ;
	rdfs:range xsd:string ;
	mms-ontology:umlPropertySource uml-property:DeploymentSpecification-deploymentLocation .

mms-property:isDimension a mms-ontology:UmlDatatypeProperty ;
	mms-ontology:key "isDimension" ;
	rdfs:label "isDimension" ;
	rdfs:comment "Indicates whether the ActivityPartition groups other ActivityPartitions along a dimension."@en ;
	rdfs:domain uml-class:ActivityPartition ;
	rdfs:range xsd:boolean ;
	mms-ontology:umlPropertySource uml-property:ActivityPartition-isDimension .

mms-property:isDimensionActivityPartition a mms-ontology:UmlDatatypeProperty ;
	owl:equivalentProperty mms-property:isDimension .

mms-property:connectionPointFromStateMachine a mms-ontology:UmlObjectProperty ;
	mms-ontology:cardinality "*"^^uml-model-dt:cardinalityRange ;
	mms-ontology:key "connectionPointIds" ;
	rdfs:label "connectionPointFromStateMachine" ;
	rdfs:comment "A Pseudostate that is the connectionPoint of this StateMachine. Based on the UML property 'StateMachine-connectionPoint' which is described as: The connection points defined for this StateMachine. They represent the interface of the StateMachine when used as part of submachine State"@en ;
	rdfs:domain uml-class:StateMachine ;
	rdfs:range uml-class:Pseudostate ;
	mms-ontology:umlPropertySource uml-property:StateMachine-connectionPoint .

mms-property:connectionPointFromState a mms-ontology:UmlObjectProperty ;
	mms-ontology:cardinality "*"^^uml-model-dt:cardinalityRange ;
	mms-ontology:key "connectionPointIds" ;
	rdfs:label "connectionPointFromState" ;
	rdfs:comment "A Pseudostate that is the connectionPoint of this State. Based on the UML property 'State-connectionPoint' which is described as: The entry and exit Pseudostates of a composite State. These can only be entry or exit Pseudostates, and they must have different names. They can only be defined for composite States."@en ;
	rdfs:domain uml-class:State ;
	rdfs:range uml-class:Pseudostate ;
	mms-ontology:umlPropertySource uml-property:State-connectionPoint .

mms-property:useCaseFromExtensionPoint a mms-ontology:UmlObjectProperty ;
	mms-ontology:cardinality "1"^^uml-model-dt:cardinalityRange ;
	mms-ontology:key "useCaseId" ;
	rdfs:label "useCaseFromExtensionPoint" ;
	rdfs:comment "The UseCase that belongs to this ExtensionPoint. Based on the UML property 'ExtensionPoint-useCase' which is described as: The UseCase that owns this ExtensionPoint."@en ;
	rdfs:domain uml-class:ExtensionPoint ;
	rdfs:range uml-class:UseCase ;
	mms-ontology:umlPropertySource uml-property:ExtensionPoint-useCase .

mms-property:useCaseFromClassifier a mms-ontology:UmlObjectProperty ;
	mms-ontology:cardinality "*"^^uml-model-dt:cardinalityRange ;
	mms-ontology:key "useCaseIds" ;
	rdfs:label "useCaseFromClassifier" ;
	rdfs:comment "A UseCase that belongs to this Classifier. Based on the UML property 'Classifier-useCase' which is described as: The set of UseCases for which this Classifier is the subject."@en ;
	rdfs:domain uml-class:Classifier ;
	rdfs:range uml-class:UseCase ;
	mms-ontology:umlPropertySource uml-property:Classifier-useCase .

mms-property:inheritedParameter a mms-ontology:UmlObjectProperty ;
	mms-ontology:cardinality "*"^^uml-model-dt:cardinalityRange ;
	mms-ontology:key "inheritedParameterIds" ;
	rdfs:label "inheritedParameter" ;
	rdfs:comment "A TemplateParameter that is the inheritedParameter of this RedefinableTemplateSignature. Based on the UML property 'RedefinableTemplateSignature-inheritedParameter' which is described as: The formal template parameters of the extended signatures."@en ;
	rdfs:domain uml-class:RedefinableTemplateSignature ;
	rdfs:range uml-class:TemplateParameter ;
	mms-ontology:umlPropertySource uml-property:RedefinableTemplateSignature-inheritedParameter .

mms-property:nodeFromStructuredActivityNode a mms-ontology:UmlObjectProperty ;
	mms-ontology:cardinality "*"^^uml-model-dt:cardinalityRange ;
	mms-ontology:key "nodeIds" ;
	rdfs:label "nodeFromStructuredActivityNode" ;
	rdfs:comment "A ActivityNode that is the node of this StructuredActivityNode. Based on the UML property 'StructuredActivityNode-node' which is described as: The ActivityNodes immediately contained in the StructuredActivityNode."@en ;
	rdfs:domain uml-class:StructuredActivityNode ;
	rdfs:range uml-class:ActivityNode ;
	mms-ontology:umlPropertySource uml-property:StructuredActivityNode-node .

mms-property:nodeFromActivity a mms-ontology:UmlObjectProperty ;
	mms-ontology:cardinality "*"^^uml-model-dt:cardinalityRange ;
	mms-ontology:key "nodeIds" ;
	rdfs:label "nodeFromActivity" ;
	rdfs:comment "A ActivityNode that is the node of this Activity. Based on the UML property 'Activity-node' which is described as: ActivityNodes coordinated by the Activity."@en ;
	rdfs:domain uml-class:Activity ;
	rdfs:range uml-class:ActivityNode ;
	mms-ontology:umlPropertySource uml-property:Activity-node .

mms-property:nodeFromInterruptibleActivityRegion a mms-ontology:UmlObjectProperty ;
	mms-ontology:cardinality "*"^^uml-model-dt:cardinalityRange ;
	mms-ontology:key "nodeIds" ;
	rdfs:label "nodeFromInterruptibleActivityRegion" ;
	rdfs:comment "A ActivityNode that is the node of this InterruptibleActivityRegion. Based on the UML property 'InterruptibleActivityRegion-node' which is described as: ActivityNodes immediately contained in the InterruptibleActivityRegion."@en ;
	rdfs:domain uml-class:InterruptibleActivityRegion ;
	rdfs:range uml-class:ActivityNode ;
	mms-ontology:umlPropertySource uml-property:InterruptibleActivityRegion-node .

mms-property:nodeFromActivityPartition a mms-ontology:UmlObjectProperty ;
	mms-ontology:cardinality "*"^^uml-model-dt:cardinalityRange ;
	mms-ontology:key "nodeIds" ;
	rdfs:label "nodeFromActivityPartition" ;
	rdfs:comment "A ActivityNode that is the node of this ActivityPartition. Based on the UML property 'ActivityPartition-node' which is described as: ActivityNodes immediately contained in the ActivityPartition."@en ;
	rdfs:domain uml-class:ActivityPartition ;
	rdfs:range uml-class:ActivityNode ;
	mms-ontology:umlPropertySource uml-property:ActivityPartition-node .

mms-property:isLocallyReentrant a mms-ontology:UmlDatatypeProperty ;
	mms-ontology:key "isLocallyReentrant" ;
	rdfs:label "isLocallyReentrant" ;
	rdfs:comment "If true, the Action can begin a new, concurrent execution, even if there is already another execution of the Action ongoing. If false, the Action cannot begin a new execution until any previous execution has completed."@en ;
	rdfs:domain uml-class:Action ;
	rdfs:range xsd:boolean ;
	mms-ontology:umlPropertySource uml-property:Action-isLocallyReentrant .

mms-property:isLocallyReentrantAction a mms-ontology:UmlDatatypeProperty ;
	owl:equivalentProperty mms-property:isLocallyReentrant .

mms-property:clause a mms-ontology:UmlObjectProperty ;
	mms-ontology:cardinality "*"^^uml-model-dt:cardinalityRange ;
	mms-ontology:key "clauseIds" ;
	rdfs:label "clause" ;
	rdfs:comment "A Clause that belongs to this ConditionalNode. Based on the UML property 'ConditionalNode-clause' which is described as: The set of Clauses composing the ConditionalNode."@en ;
	rdfs:domain uml-class:ConditionalNode ;
	rdfs:range uml-class:Clause ;
	mms-ontology:umlPropertySource uml-property:ConditionalNode-clause .

mms-property:annotatedElement a mms-ontology:UmlObjectProperty ;
	mms-ontology:cardinality "*"^^uml-model-dt:cardinalityRange ;
	mms-ontology:key "annotatedElementIds" ;
	rdfs:label "annotatedElement" ;
	rdfs:comment "A Element that belongs to this Comment. Based on the UML property 'Comment-annotatedElement' which is described as: References the Element(s) being commented."@en ;
	rdfs:domain uml-class:Comment ;
	rdfs:range uml-class:Element ;
	mms-ontology:umlPropertySource uml-property:Comment-annotatedElement .

mms-property:valueInputPinFromWriteVariableAction a mms-ontology:UmlObjectProperty ;
	mms-ontology:cardinality "1"^^uml-model-dt:cardinalityRange ;
	mms-ontology:key "valueId" ;
	rdfs:label "valueInputPinFromWriteVariableAction" ;
	rdfs:comment "The InputPin that is the value of this WriteVariableAction. Based on the UML property 'WriteVariableAction-value' which is described as: The InputPin that gives the value to be added or removed from the Variable."@en ;
	rdfs:domain uml-class:WriteVariableAction ;
	rdfs:range uml-class:InputPin ;
	mms-ontology:umlPropertySource uml-property:WriteVariableAction-value .

mms-property:valueInputPinFromLinkEndData a mms-ontology:UmlObjectProperty ;
	mms-ontology:cardinality "1"^^uml-model-dt:cardinalityRange ;
	mms-ontology:key "valueId" ;
	rdfs:label "valueInputPinFromLinkEndData" ;
	rdfs:comment "The InputPin that is the value of this LinkEndData. Based on the UML property 'LinkEndData-value' which is described as: The InputPin that provides the specified value for the given end. This InputPin is omitted if the LinkEndData specifies the &#34;open&#34; end for a ReadLinkAction."@en ;
	rdfs:domain uml-class:LinkEndData ;
	rdfs:range uml-class:InputPin ;
	mms-ontology:umlPropertySource uml-property:LinkEndData-value .

mms-property:valueInputPinFromWriteStructuralFeatureAction a mms-ontology:UmlObjectProperty ;
	mms-ontology:cardinality "1"^^uml-model-dt:cardinalityRange ;
	mms-ontology:key "valueId" ;
	rdfs:label "valueInputPinFromWriteStructuralFeatureAction" ;
	rdfs:comment "The InputPin that is the value of this WriteStructuralFeatureAction. Based on the UML property 'WriteStructuralFeatureAction-value' which is described as: The InputPin that provides the value to be added or removed from the StructuralFeature."@en ;
	rdfs:domain uml-class:WriteStructuralFeatureAction ;
	rdfs:range uml-class:InputPin ;
	mms-ontology:umlPropertySource uml-property:WriteStructuralFeatureAction-value .

mms-property:valueInputPinFromQualifierValue a mms-ontology:UmlObjectProperty ;
	mms-ontology:cardinality "1"^^uml-model-dt:cardinalityRange ;
	mms-ontology:key "valueId" ;
	rdfs:label "valueInputPinFromQualifierValue" ;
	rdfs:comment "The InputPin that is the value of this QualifierValue. Based on the UML property 'QualifierValue-value' which is described as: The InputPin from which the specified value for the qualifier is taken."@en ;
	rdfs:domain uml-class:QualifierValue ;
	rdfs:range uml-class:InputPin ;
	mms-ontology:umlPropertySource uml-property:QualifierValue-value .

mms-property:valueString a mms-ontology:UmlDatatypeProperty ;
	mms-ontology:cardinality "1"^^uml-model-dt:cardinalityRange ;
	mms-ontology:key "valueId" ;
	rdfs:label "valueString" ;
	rdfs:comment "The String that is the value of this LiteralString. Based on the UML property 'LiteralString-value' which is described as: The specified String value."@en ;
	rdfs:domain uml-class:LiteralString ;
	rdfs:range xsd:string ;
	mms-ontology:umlPropertySource uml-property:LiteralString-value .

mms-property:valueValueSpecificationFromValuePin a mms-ontology:UmlObjectProperty ;
	mms-ontology:cardinality "1"^^uml-model-dt:cardinalityRange ;
	mms-ontology:key "valueId" ;
	rdfs:label "valueValueSpecificationFromValuePin" ;
	rdfs:comment "The ValueSpecification that is the value of this ValuePin. Based on the UML property 'ValuePin-value' which is described as: The ValueSpecification that is evaluated to obtain the value that the ValuePin will provide."@en ;
	rdfs:domain uml-class:ValuePin ;
	rdfs:range uml-class:ValueSpecification ;
	mms-ontology:umlPropertySource uml-property:ValuePin-value .

mms-property:valueValueSpecificationFromSlot a mms-ontology:UmlObjectProperty ;
	mms-ontology:cardinality "*"^^uml-model-dt:cardinalityRange ;
	mms-ontology:key "valueIds" ;
	rdfs:label "valueValueSpecificationFromSlot" ;
	rdfs:comment "A ValueSpecification that is the value of this Slot. Based on the UML property 'Slot-value' which is described as: The value or values held by the Slot."@en ;
	rdfs:domain uml-class:Slot ;
	rdfs:range uml-class:ValueSpecification ;
	mms-ontology:umlPropertySource uml-property:Slot-value .

mms-property:valueValueSpecificationFromValueSpecificationAction a mms-ontology:UmlObjectProperty ;
	mms-ontology:cardinality "1"^^uml-model-dt:cardinalityRange ;
	mms-ontology:key "valueId" ;
	rdfs:label "valueValueSpecificationFromValueSpecificationAction" ;
	rdfs:comment "The ValueSpecification that is the value of this ValueSpecificationAction. Based on the UML property 'ValueSpecificationAction-value' which is described as: The ValueSpecification to be evaluated."@en ;
	rdfs:domain uml-class:ValueSpecificationAction ;
	rdfs:range uml-class:ValueSpecification ;
	mms-ontology:umlPropertySource uml-property:ValueSpecificationAction-value .

mms-property:valueUnlimitedNatural a mms-ontology:UmlDatatypeProperty ;
	mms-ontology:cardinality "1"^^uml-model-dt:cardinalityRange ;
	mms-ontology:key "valueId" ;
	rdfs:label "valueUnlimitedNatural" ;
	rdfs:comment "The UnlimitedNatural that is the value of this LiteralUnlimitedNatural. Based on the UML property 'LiteralUnlimitedNatural-value' which is described as: The specified UnlimitedNatural value."@en ;
	rdfs:domain uml-class:LiteralUnlimitedNatural ;
	rdfs:range xsd:string ;
	mms-ontology:umlPropertySource uml-property:LiteralUnlimitedNatural-value .

mms-property:valueInteger a mms-ontology:UmlDatatypeProperty ;
	mms-ontology:cardinality "1"^^uml-model-dt:cardinalityRange ;
	mms-ontology:key "valueId" ;
	rdfs:label "valueInteger" ;
	rdfs:comment "The Integer that is the value of this LiteralInteger. Based on the UML property 'LiteralInteger-value' which is described as: The specified Integer value."@en ;
	rdfs:domain uml-class:LiteralInteger ;
	rdfs:range xsd:integer ;
	mms-ontology:umlPropertySource uml-property:LiteralInteger-value .

mms-property:valueReal a mms-ontology:UmlDatatypeProperty ;
	mms-ontology:cardinality "1"^^uml-model-dt:cardinalityRange ;
	mms-ontology:key "valueId" ;
	rdfs:label "valueReal" ;
	rdfs:comment "The Real that is the value of this LiteralReal. Based on the UML property 'LiteralReal-value' which is described as: The specified Real value."@en ;
	rdfs:domain uml-class:LiteralReal ;
	rdfs:range xsd:double ;
	mms-ontology:umlPropertySource uml-property:LiteralReal-value .

mms-property:valueBoolean a mms-ontology:UmlDatatypeProperty ;
	mms-ontology:cardinality "1"^^uml-model-dt:cardinalityRange ;
	mms-ontology:key "valueId" ;
	rdfs:label "valueBoolean" ;
	rdfs:comment "The Boolean that is the value of this LiteralBoolean. Based on the UML property 'LiteralBoolean-value' which is described as: The specified Boolean value."@en ;
	rdfs:domain uml-class:LiteralBoolean ;
	rdfs:range xsd:boolean ;
	mms-ontology:umlPropertySource uml-property:LiteralBoolean-value .

mms-property:bodyStringFromOpaqueAction a mms-ontology:UmlDatatypeProperty ;
	mms-ontology:cardinality "*"^^uml-model-dt:cardinalityRange ;
	mms-ontology:key "bodyIds" ;
	rdfs:label "bodyStringFromOpaqueAction" ;
	rdfs:comment "A String that is the body of this OpaqueAction. Based on the UML property 'OpaqueAction-body' which is described as: Provides a textual specification of the functionality of the Action, in one or more languages other than UML."@en ;
	rdfs:domain uml-class:OpaqueAction ;
	rdfs:range xsd:string ;
	mms-ontology:umlPropertySource uml-property:OpaqueAction-body .

mms-property:bodyStringFromComment a mms-ontology:UmlDatatypeProperty ;
	mms-ontology:cardinality "1"^^uml-model-dt:cardinalityRange ;
	mms-ontology:key "bodyId" ;
	rdfs:label "bodyStringFromComment" ;
	rdfs:comment "The String that is the body of this Comment. Based on the UML property 'Comment-body' which is described as: Specifies a string that is the comment."@en ;
	rdfs:domain uml-class:Comment ;
	rdfs:range xsd:string ;
	mms-ontology:umlPropertySource uml-property:Comment-body .

mms-property:bodyStringFromOpaqueBehavior a mms-ontology:UmlDatatypeProperty ;
	mms-ontology:cardinality "*"^^uml-model-dt:cardinalityRange ;
	mms-ontology:key "bodyIds" ;
	rdfs:label "bodyStringFromOpaqueBehavior" ;
	rdfs:comment "A String that is the body of this OpaqueBehavior. Based on the UML property 'OpaqueBehavior-body' which is described as: Specifies the behavior in one or more languages."@en ;
	rdfs:domain uml-class:OpaqueBehavior ;
	rdfs:range xsd:string ;
	mms-ontology:umlPropertySource uml-property:OpaqueBehavior-body .

mms-property:bodyStringFromOpaqueExpression a mms-ontology:UmlDatatypeProperty ;
	mms-ontology:cardinality "*"^^uml-model-dt:cardinalityRange ;
	mms-ontology:key "bodyIds" ;
	rdfs:label "bodyStringFromOpaqueExpression" ;
	rdfs:comment "A String that is the body of this OpaqueExpression. Based on the UML property 'OpaqueExpression-body' which is described as: A textual definition of the behavior of the OpaqueExpression, possibly in multiple languages."@en ;
	rdfs:domain uml-class:OpaqueExpression ;
	rdfs:range xsd:string ;
	mms-ontology:umlPropertySource uml-property:OpaqueExpression-body .

mms-property:bodyExecutableNode a mms-ontology:UmlObjectProperty ;
	mms-ontology:cardinality "*"^^uml-model-dt:cardinalityRange ;
	mms-ontology:key "bodyIds" ;
	rdfs:label "bodyExecutableNode" ;
	rdfs:comment "A ExecutableNode that is the body of this Clause. Based on the UML property 'Clause-body' which is described as: The set of ExecutableNodes that are executed if the test evaluates to true and the Clause is chosen over other Clauses within the ConditionalNode that also have tests that evaluate to true."@en ;
	rdfs:domain uml-class:Clause ;
	rdfs:range uml-class:ExecutableNode ;
	mms-ontology:umlPropertySource uml-property:Clause-body .

mms-property:entryPseudostate a mms-ontology:UmlObjectProperty ;
	mms-ontology:cardinality "*"^^uml-model-dt:cardinalityRange ;
	mms-ontology:key "entryIds" ;
	rdfs:label "entryPseudostate" ;
	rdfs:comment "A Pseudostate that is the entry of this ConnectionPointReference. Based on the UML property 'ConnectionPointReference-entry' which is described as: The entryPoint Pseudostates corresponding to this connection point."@en ;
	rdfs:domain uml-class:ConnectionPointReference ;
	rdfs:range uml-class:Pseudostate ;
	mms-ontology:umlPropertySource uml-property:ConnectionPointReference-entry .

mms-property:entryBehavior a mms-ontology:UmlObjectProperty ;
	mms-ontology:cardinality "1"^^uml-model-dt:cardinalityRange ;
	mms-ontology:key "entryId" ;
	rdfs:label "entryBehavior" ;
	rdfs:comment "The Behavior that is the entry of this State. Based on the UML property 'State-entry' which is described as: An optional Behavior that is executed whenever this State is entered regardless of the Transition taken to reach the State. If defined, entry Behaviors are always executed to completion prior to any internal Behavior or Transitions performed within the State."@en ;
	rdfs:domain uml-class:State ;
	rdfs:range uml-class:Behavior ;
	mms-ontology:umlPropertySource uml-property:State-entry .

mms-property:appliedProfile a mms-ontology:UmlObjectProperty ;
	mms-ontology:cardinality "1"^^uml-model-dt:cardinalityRange ;
	mms-ontology:key "appliedProfileId" ;
	rdfs:label "appliedProfile" ;
	rdfs:comment "The Profile that belongs to this ProfileApplication. Based on the UML property 'ProfileApplication-appliedProfile' which is described as: References the Profiles that are applied to a Package through this ProfileApplication."@en ;
	rdfs:domain uml-class:ProfileApplication ;
	rdfs:range uml-class:Profile ;
	mms-ontology:umlPropertySource uml-property:ProfileApplication-appliedProfile .

mms-property:argumentValueSpecificationFromMessage a mms-ontology:UmlObjectProperty ;
	mms-ontology:cardinality "*"^^uml-model-dt:cardinalityRange ;
	mms-ontology:key "argumentIds" ;
	rdfs:label "argumentValueSpecificationFromMessage" ;
	rdfs:comment "A ValueSpecification that is the argument of this Message. Based on the UML property 'Message-argument' which is described as: The arguments of the Message."@en ;
	rdfs:domain uml-class:Message ;
	rdfs:range uml-class:ValueSpecification ;
	mms-ontology:umlPropertySource uml-property:Message-argument .

mms-property:argumentValueSpecificationFromInteractionUse a mms-ontology:UmlObjectProperty ;
	mms-ontology:cardinality "*"^^uml-model-dt:cardinalityRange ;
	mms-ontology:key "argumentIds" ;
	rdfs:label "argumentValueSpecificationFromInteractionUse" ;
	rdfs:comment "A ValueSpecification that is the argument of this InteractionUse. Based on the UML property 'InteractionUse-argument' which is described as: The actual arguments of the Interaction."@en ;
	rdfs:domain uml-class:InteractionUse ;
	rdfs:range uml-class:ValueSpecification ;
	mms-ontology:umlPropertySource uml-property:InteractionUse-argument .

mms-property:argumentInputPin a mms-ontology:UmlObjectProperty ;
	mms-ontology:cardinality "*"^^uml-model-dt:cardinalityRange ;
	mms-ontology:key "argumentIds" ;
	rdfs:label "argumentInputPin" ;
	rdfs:comment "A InputPin that is the argument of this InvocationAction. Based on the UML property 'InvocationAction-argument' which is described as: The InputPins that provide the argument values passed in the invocation request."@en ;
	rdfs:domain uml-class:InvocationAction ;
	rdfs:range uml-class:InputPin ;
	mms-ontology:umlPropertySource uml-property:InvocationAction-argument .

mms-property:inStructuredNodeStructuredActivityNodeFromActivityEdge a mms-ontology:UmlObjectProperty ;
	mms-ontology:cardinality "1"^^uml-model-dt:cardinalityRange ;
	mms-ontology:key "inStructuredNodeId" ;
	rdfs:label "inStructuredNodeStructuredActivityNodeFromActivityEdge" ;
	rdfs:comment "The StructuredActivityNode that is the inStructuredNode of this ActivityEdge. Based on the UML property 'ActivityEdge-inStructuredNode' which is described as: The StructuredActivityNode containing the ActivityEdge, if it is owned by a StructuredActivityNode."@en ;
	rdfs:domain uml-class:ActivityEdge ;
	rdfs:range uml-class:StructuredActivityNode ;
	mms-ontology:umlPropertySource uml-property:ActivityEdge-inStructuredNode .

mms-property:inStructuredNodeStructuredActivityNodeFromActivityNode a mms-ontology:UmlObjectProperty ;
	mms-ontology:cardinality "1"^^uml-model-dt:cardinalityRange ;
	mms-ontology:key "inStructuredNodeId" ;
	rdfs:label "inStructuredNodeStructuredActivityNodeFromActivityNode" ;
	rdfs:comment "The StructuredActivityNode that is the inStructuredNode of this ActivityNode. Based on the UML property 'ActivityNode-inStructuredNode' which is described as: The StructuredActivityNode containing the ActvityNode, if it is directly owned by a StructuredActivityNode."@en ;
	rdfs:domain uml-class:ActivityNode ;
	rdfs:range uml-class:StructuredActivityNode ;
	mms-ontology:umlPropertySource uml-property:ActivityNode-inStructuredNode .

mms-property:insertAtInputPinFromAddStructuralFeatureValueAction a mms-ontology:UmlObjectProperty ;
	mms-ontology:cardinality "1"^^uml-model-dt:cardinalityRange ;
	mms-ontology:key "insertAtId" ;
	rdfs:label "insertAtInputPinFromAddStructuralFeatureValueAction" ;
	rdfs:comment "The InputPin that is the insertAt of this AddStructuralFeatureValueAction. Based on the UML property 'AddStructuralFeatureValueAction-insertAt' which is described as: The InputPin that gives the position at which to insert the value in an ordered StructuralFeature. The type of the insertAt InputPin is UnlimitedNatural, but the value cannot be zero. It is omitted for unordered StructuralFeatures."@en ;
	rdfs:domain uml-class:AddStructuralFeatureValueAction ;
	rdfs:range uml-class:InputPin ;
	mms-ontology:umlPropertySource uml-property:AddStructuralFeatureValueAction-insertAt .

mms-property:insertAtInputPinFromAddVariableValueAction a mms-ontology:UmlObjectProperty ;
	mms-ontology:cardinality "1"^^uml-model-dt:cardinalityRange ;
	mms-ontology:key "insertAtId" ;
	rdfs:label "insertAtInputPinFromAddVariableValueAction" ;
	rdfs:comment "The InputPin that is the insertAt of this AddVariableValueAction. Based on the UML property 'AddVariableValueAction-insertAt' which is described as: The InputPin that gives the position at which to insert a new value or move an existing value in ordered Variables. The type of the insertAt InputPin is UnlimitedNatural, but the value cannot be zero. It is omitted for unordered Variables."@en ;
	rdfs:domain uml-class:AddVariableValueAction ;
	rdfs:range uml-class:InputPin ;
	mms-ontology:umlPropertySource uml-property:AddVariableValueAction-insertAt .

mms-property:insertAtInputPinFromLinkEndCreationData a mms-ontology:UmlObjectProperty ;
	mms-ontology:cardinality "1"^^uml-model-dt:cardinalityRange ;
	mms-ontology:key "insertAtId" ;
	rdfs:label "insertAtInputPinFromLinkEndCreationData" ;
	rdfs:comment "The InputPin that is the insertAt of this LinkEndCreationData. Based on the UML property 'LinkEndCreationData-insertAt' which is described as: For ordered Association ends, the InputPin that provides the position where the new link should be inserted or where an existing link should be moved to. The type of the insertAt InputPin is UnlimitedNatural, but the input cannot be zero. It is omitted for Association ends that are not ordered."@en ;
	rdfs:domain uml-class:LinkEndCreationData ;
	rdfs:range uml-class:InputPin ;
	mms-ontology:umlPropertySource uml-property:LinkEndCreationData-insertAt .

mms-property:sourceVertex a mms-ontology:UmlObjectProperty ;
	mms-ontology:cardinality "1"^^uml-model-dt:cardinalityRange ;
	mms-ontology:key "sourceId" ;
	rdfs:label "sourceVertex" ;
	rdfs:comment "The Vertex that is the source of this Transition. Based on the UML property 'Transition-source' which is described as: Designates the originating Vertex (State or Pseudostate) of the Transition."@en ;
	rdfs:domain uml-class:Transition ;
	rdfs:range uml-class:Vertex ;
	mms-ontology:umlPropertySource uml-property:Transition-source .

mms-property:sourceElement a mms-ontology:UmlObjectProperty ;
	mms-ontology:cardinality "*"^^uml-model-dt:cardinalityRange ;
	mms-ontology:key "sourceIds" ;
	rdfs:label "sourceElement" ;
	rdfs:comment "A Element that is the source of this DirectedRelationship. Based on the UML property 'DirectedRelationship-source' which is described as: Specifies the source Element(s) of the DirectedRelationship."@en ;
	rdfs:domain uml-class:DirectedRelationship ;
	rdfs:range uml-class:Element ;
	mms-ontology:umlPropertySource uml-property:DirectedRelationship-source .

mms-property:sourceActivityNode a mms-ontology:UmlObjectProperty ;
	mms-ontology:cardinality "1"^^uml-model-dt:cardinalityRange ;
	mms-ontology:key "sourceId" ;
	rdfs:label "sourceActivityNode" ;
	rdfs:comment "The ActivityNode that is the source of this ActivityEdge. Based on the UML property 'ActivityEdge-source' which is described as: The ActivityNode from which tokens are taken when they traverse the ActivityEdge."@en ;
	rdfs:domain uml-class:ActivityEdge ;
	rdfs:range uml-class:ActivityNode ;
	mms-ontology:umlPropertySource uml-property:ActivityEdge-source .

mms-property:metaclassReference a mms-ontology:UmlObjectProperty ;
	mms-ontology:cardinality "*"^^uml-model-dt:cardinalityRange ;
	mms-ontology:key "metaclassReferenceIds" ;
	rdfs:label "metaclassReference" ;
	rdfs:comment "A ElementImport that is the metaclassReference of this Profile. Based on the UML property 'Profile-metaclassReference' which is described as: References a metaclass that may be extended."@en ;
	rdfs:domain uml-class:Profile ;
	rdfs:range uml-class:ElementImport ;
	mms-ontology:umlPropertySource uml-property:Profile-metaclassReference .

mms-property:isRelative a mms-ontology:UmlDatatypeProperty ;
	mms-ontology:key "isRelative" ;
	rdfs:label "isRelative" ;
	rdfs:comment "Specifies whether the TimeEvent is specified as an absolute or relative time."@en ;
	rdfs:domain uml-class:TimeEvent ;
	rdfs:range xsd:boolean ;
	mms-ontology:umlPropertySource uml-property:TimeEvent-isRelative .

mms-property:isRelativeTimeEvent a mms-ontology:UmlDatatypeProperty ;
	owl:equivalentProperty mms-property:isRelative .

mms-property:enumeration a mms-ontology:UmlObjectProperty ;
	mms-ontology:cardinality "1"^^uml-model-dt:cardinalityRange ;
	mms-ontology:key "enumerationId" ;
	rdfs:label "enumeration" ;
	rdfs:comment "The Enumeration that belongs to this EnumerationLiteral. Based on the UML property 'EnumerationLiteral-enumeration' which is described as: The Enumeration that this EnumerationLiteral is a member of."@en ;
	rdfs:domain uml-class:EnumerationLiteral ;
	rdfs:range uml-class:Enumeration ;
	mms-ontology:umlPropertySource uml-property:EnumerationLiteral-enumeration .

mms-property:ownedRule a mms-ontology:UmlObjectProperty ;
	mms-ontology:cardinality "*"^^uml-model-dt:cardinalityRange ;
	mms-ontology:key "ownedRuleIds" ;
	rdfs:label "ownedRule" ;
	rdfs:comment "A Constraint that is the ownedRule of this Namespace. Based on the UML property 'Namespace-ownedRule' which is described as: Specifies a set of Constraints owned by this Namespace."@en ;
	rdfs:domain uml-class:Namespace ;
	rdfs:range uml-class:Constraint ;
	mms-ontology:umlPropertySource uml-property:Namespace-ownedRule .

mms-property:lifeline a mms-ontology:UmlObjectProperty ;
	mms-ontology:cardinality "*"^^uml-model-dt:cardinalityRange ;
	mms-ontology:key "lifelineIds" ;
	rdfs:label "lifeline" ;
	rdfs:comment "A Lifeline that belongs to this Interaction. Based on the UML property 'Interaction-lifeline' which is described as: Specifies the participants in this Interaction."@en ;
	rdfs:domain uml-class:Interaction ;
	rdfs:range uml-class:Lifeline ;
	mms-ontology:umlPropertySource uml-property:Interaction-lifeline .

mms-property:extendedSignature a mms-ontology:UmlObjectProperty ;
	mms-ontology:cardinality "*"^^uml-model-dt:cardinalityRange ;
	mms-ontology:key "extendedSignatureIds" ;
	rdfs:label "extendedSignature" ;
	rdfs:comment "A RedefinableTemplateSignature that is the extendedSignature of this RedefinableTemplateSignature. Based on the UML property 'RedefinableTemplateSignature-extendedSignature' which is described as: The signatures extended by this RedefinableTemplateSignature."@en ;
	rdfs:domain uml-class:RedefinableTemplateSignature ;
	rdfs:range uml-class:RedefinableTemplateSignature ;
	mms-ontology:umlPropertySource uml-property:RedefinableTemplateSignature-extendedSignature .

mms-property:informationTarget a mms-ontology:UmlObjectProperty ;
	mms-ontology:cardinality "*"^^uml-model-dt:cardinalityRange ;
	mms-ontology:key "informationTargetIds" ;
	rdfs:label "informationTarget" ;
	rdfs:comment "A NamedElement that is the informationTarget of this InformationFlow. Based on the UML property 'InformationFlow-informationTarget' which is described as: Defines to which target the conveyed InformationItems are directed."@en ;
	rdfs:domain uml-class:InformationFlow ;
	rdfs:range uml-class:NamedElement ;
	mms-ontology:umlPropertySource uml-property:InformationFlow-informationTarget .

mms-property:stateFromRegion a mms-ontology:UmlObjectProperty ;
	mms-ontology:cardinality "1"^^uml-model-dt:cardinalityRange ;
	mms-ontology:key "stateId" ;
	rdfs:label "stateFromRegion" ;
	rdfs:comment "The State that belongs to this Region. Based on the UML property 'Region-state' which is described as: The State that owns the Region. If a Region is owned by a State, then it cannot also be owned by a StateMachine."@en ;
	rdfs:domain uml-class:Region ;
	rdfs:range uml-class:State ;
	mms-ontology:umlPropertySource uml-property:Region-state .

mms-property:stateFromPseudostate a mms-ontology:UmlObjectProperty ;
	mms-ontology:cardinality "1"^^uml-model-dt:cardinalityRange ;
	mms-ontology:key "stateId" ;
	rdfs:label "stateFromPseudostate" ;
	rdfs:comment "The State that belongs to this Pseudostate. Based on the UML property 'Pseudostate-state' which is described as: The State that owns this Pseudostate and in which it appears."@en ;
	rdfs:domain uml-class:Pseudostate ;
	rdfs:range uml-class:State ;
	mms-ontology:umlPropertySource uml-property:Pseudostate-state .

mms-property:stateFromConnectionPointReference a mms-ontology:UmlObjectProperty ;
	mms-ontology:cardinality "1"^^uml-model-dt:cardinalityRange ;
	mms-ontology:key "stateId" ;
	rdfs:label "stateFromConnectionPointReference" ;
	rdfs:comment "The State that belongs to this ConnectionPointReference. Based on the UML property 'ConnectionPointReference-state' which is described as: The State in which the ConnectionPointReference is defined."@en ;
	rdfs:domain uml-class:ConnectionPointReference ;
	rdfs:range uml-class:State ;
	mms-ontology:umlPropertySource uml-property:ConnectionPointReference-state .

mms-property:formalGate a mms-ontology:UmlObjectProperty ;
	mms-ontology:cardinality "*"^^uml-model-dt:cardinalityRange ;
	mms-ontology:key "formalGateIds" ;
	rdfs:label "formalGate" ;
	rdfs:comment "A Gate that belongs to this Interaction. Based on the UML property 'Interaction-formalGate' which is described as: Specifies the gates that form the message interface between this Interaction and any InteractionUses which reference it."@en ;
	rdfs:domain uml-class:Interaction ;
	rdfs:range uml-class:Gate ;
	mms-ontology:umlPropertySource uml-property:Interaction-formalGate .

mms-property:isDerivedProperty a mms-ontology:UmlDatatypeProperty ;
	mms-ontology:key "isDerived" ;
	rdfs:label "isDerivedProperty" ;
	rdfs:comment "Specifies whether the Property is derived, i.e., whether its value or values can be computed from other information."@en ;
	rdfs:domain uml-class:Property ;
	rdfs:range xsd:boolean ;
	mms-ontology:umlPropertySource uml-property:Property-isDerived .

mms-property:isDerivedAssociation a mms-ontology:UmlDatatypeProperty ;
	mms-ontology:key "isDerived" ;
	rdfs:label "isDerivedAssociation" ;
	rdfs:comment "Specifies whether the Association is derived from other model elements such as other Associations."@en ;
	rdfs:domain uml-class:Association ;
	rdfs:range xsd:boolean ;
	mms-ontology:umlPropertySource uml-property:Association-isDerived .

mms-property:templateParameterOperationTemplateParameter a mms-ontology:UmlObjectProperty ;
	mms-ontology:cardinality "1"^^uml-model-dt:cardinalityRange ;
	mms-ontology:key "templateParameterId" ;
	rdfs:label "templateParameterOperationTemplateParameter" ;
	rdfs:comment "The OperationTemplateParameter that is the templateParameter of this Operation. Based on the UML property 'Operation-templateParameter' which is described as: The OperationTemplateParameter that exposes this element as a formal parameter."@en ;
	rdfs:domain uml-class:Operation ;
	rdfs:range uml-class:OperationTemplateParameter ;
	mms-ontology:umlPropertySource uml-property:Operation-templateParameter .

mms-property:templateParameterConnectableElementTemplateParameter a mms-ontology:UmlObjectProperty ;
	mms-ontology:cardinality "1"^^uml-model-dt:cardinalityRange ;
	mms-ontology:key "templateParameterId" ;
	rdfs:label "templateParameterConnectableElementTemplateParameter" ;
	rdfs:comment "The ConnectableElementTemplateParameter that is the templateParameter of this ConnectableElement. Based on the UML property 'ConnectableElement-templateParameter' which is described as: The ConnectableElementTemplateParameter for this ConnectableElement parameter."@en ;
	rdfs:domain uml-class:ConnectableElement ;
	rdfs:range uml-class:ConnectableElementTemplateParameter ;
	mms-ontology:umlPropertySource uml-property:ConnectableElement-templateParameter .

mms-property:templateParameterClassifierTemplateParameter a mms-ontology:UmlObjectProperty ;
	mms-ontology:cardinality "1"^^uml-model-dt:cardinalityRange ;
	mms-ontology:key "templateParameterId" ;
	rdfs:label "templateParameterClassifierTemplateParameter" ;
	rdfs:comment "The ClassifierTemplateParameter that is the templateParameter of this Classifier. Based on the UML property 'Classifier-templateParameter' which is described as: TheClassifierTemplateParameter that exposes this element as a formal parameter."@en ;
	rdfs:domain uml-class:Classifier ;
	rdfs:range uml-class:ClassifierTemplateParameter ;
	mms-ontology:umlPropertySource uml-property:Classifier-templateParameter .

mms-property:templateParameter a mms-ontology:UmlObjectProperty ;
	mms-ontology:cardinality "1"^^uml-model-dt:cardinalityRange ;
	mms-ontology:key "templateParameterId" ;
	rdfs:label "templateParameter" ;
	rdfs:comment "The TemplateParameter that belongs to this ParameterableElement. Based on the UML property 'ParameterableElement-templateParameter' which is described as: The TemplateParameter that exposes this ParameterableElement as a formal parameter."@en ;
	rdfs:domain uml-class:ParameterableElement ;
	rdfs:range uml-class:TemplateParameter ;
	mms-ontology:umlPropertySource uml-property:ParameterableElement-templateParameter .

mms-property:classifierFromInstanceSpecification a mms-ontology:UmlObjectProperty ;
	mms-ontology:cardinality "*"^^uml-model-dt:cardinalityRange ;
	mms-ontology:key "classifierIds" ;
	rdfs:label "classifierFromInstanceSpecification" ;
	rdfs:comment "A Classifier that belongs to this InstanceSpecification. Based on the UML property 'InstanceSpecification-classifier' which is described as: The Classifier or Classifiers of the represented instance. If multiple Classifiers are specified, the instance is classified by all of them."@en ;
	rdfs:domain uml-class:InstanceSpecification ;
	rdfs:range uml-class:Classifier ;
	mms-ontology:umlPropertySource uml-property:InstanceSpecification-classifier .

mms-property:classifierFromRedefinableTemplateSignature a mms-ontology:UmlObjectProperty ;
	mms-ontology:cardinality "1"^^uml-model-dt:cardinalityRange ;
	mms-ontology:key "classifierId" ;
	rdfs:label "classifierFromRedefinableTemplateSignature" ;
	rdfs:comment "The Classifier that belongs to this RedefinableTemplateSignature. Based on the UML property 'RedefinableTemplateSignature-classifier' which is described as: The Classifier that owns this RedefinableTemplateSignature."@en ;
	rdfs:domain uml-class:RedefinableTemplateSignature ;
	rdfs:range uml-class:Classifier ;
	mms-ontology:umlPropertySource uml-property:RedefinableTemplateSignature-classifier .

mms-property:classifierFromReadIsClassifiedObjectAction a mms-ontology:UmlObjectProperty ;
	mms-ontology:cardinality "1"^^uml-model-dt:cardinalityRange ;
	mms-ontology:key "classifierId" ;
	rdfs:label "classifierFromReadIsClassifiedObjectAction" ;
	rdfs:comment "The Classifier that belongs to this ReadIsClassifiedObjectAction. Based on the UML property 'ReadIsClassifiedObjectAction-classifier' which is described as: The Classifier against which the classification of the input object is tested."@en ;
	rdfs:domain uml-class:ReadIsClassifiedObjectAction ;
	rdfs:range uml-class:Classifier ;
	mms-ontology:umlPropertySource uml-property:ReadIsClassifiedObjectAction-classifier .

mms-property:classifierFromReadExtentAction a mms-ontology:UmlObjectProperty ;
	mms-ontology:cardinality "1"^^uml-model-dt:cardinalityRange ;
	mms-ontology:key "classifierId" ;
	rdfs:label "classifierFromReadExtentAction" ;
	rdfs:comment "The Classifier that belongs to this ReadExtentAction. Based on the UML property 'ReadExtentAction-classifier' which is described as: The Classifier whose instances are to be retrieved."@en ;
	rdfs:domain uml-class:ReadExtentAction ;
	rdfs:range uml-class:Classifier ;
	mms-ontology:umlPropertySource uml-property:ReadExtentAction-classifier .

mms-property:classifierFromCreateObjectAction a mms-ontology:UmlObjectProperty ;
	mms-ontology:cardinality "1"^^uml-model-dt:cardinalityRange ;
	mms-ontology:key "classifierId" ;
	rdfs:label "classifierFromCreateObjectAction" ;
	rdfs:comment "The Classifier that belongs to this CreateObjectAction. Based on the UML property 'CreateObjectAction-classifier' which is described as: The Classifier to be instantiated."@en ;
	rdfs:domain uml-class:CreateObjectAction ;
	rdfs:range uml-class:Classifier ;
	mms-ontology:umlPropertySource uml-property:CreateObjectAction-classifier .

mms-property:classifierEnumeration a mms-ontology:UmlObjectProperty ;
	mms-ontology:cardinality "1"^^uml-model-dt:cardinalityRange ;
	mms-ontology:key "classifierId" ;
	rdfs:label "classifierEnumeration" ;
	rdfs:comment "The Enumeration that is the classifier of this EnumerationLiteral. Based on the UML property 'EnumerationLiteral-classifier' which is described as: The classifier of this EnumerationLiteral derived to be equal to its Enumeration."@en ;
	rdfs:domain uml-class:EnumerationLiteral ;
	rdfs:range uml-class:Enumeration ;
	mms-ontology:umlPropertySource uml-property:EnumerationLiteral-classifier .

mms-property:operationFromCallEvent a mms-ontology:UmlObjectProperty ;
	mms-ontology:cardinality "1"^^uml-model-dt:cardinalityRange ;
	mms-ontology:key "operationId" ;
	rdfs:label "operationFromCallEvent" ;
	rdfs:comment "The Operation that belongs to this CallEvent. Based on the UML property 'CallEvent-operation' which is described as: Designates the Operation whose invocation raised the CalEvent."@en ;
	rdfs:domain uml-class:CallEvent ;
	rdfs:range uml-class:Operation ;
	mms-ontology:umlPropertySource uml-property:CallEvent-operation .

mms-property:operationFromParameter a mms-ontology:UmlObjectProperty ;
	mms-ontology:cardinality "1"^^uml-model-dt:cardinalityRange ;
	mms-ontology:key "operationId" ;
	rdfs:label "operationFromParameter" ;
	rdfs:comment "The Operation that belongs to this Parameter. Based on the UML property 'Parameter-operation' which is described as: The Operation owning this parameter."@en ;
	rdfs:domain uml-class:Parameter ;
	rdfs:range uml-class:Operation ;
	mms-ontology:umlPropertySource uml-property:Parameter-operation .

mms-property:operationFromCallOperationAction a mms-ontology:UmlObjectProperty ;
	mms-ontology:cardinality "1"^^uml-model-dt:cardinalityRange ;
	mms-ontology:key "operationId" ;
	rdfs:label "operationFromCallOperationAction" ;
	rdfs:comment "The Operation that belongs to this CallOperationAction. Based on the UML property 'CallOperationAction-operation' which is described as: The Operation being invoked."@en ;
	rdfs:domain uml-class:CallOperationAction ;
	rdfs:range uml-class:Operation ;
	mms-ontology:umlPropertySource uml-property:CallOperationAction-operation .

mms-property:containerRegionFromVertex a mms-ontology:UmlObjectProperty ;
	mms-ontology:cardinality "1"^^uml-model-dt:cardinalityRange ;
	mms-ontology:key "containerId" ;
	rdfs:label "containerRegionFromVertex" ;
	rdfs:comment "The Region that is the container of this Vertex. Based on the UML property 'Vertex-container' which is described as: The Region that contains this Vertex."@en ;
	rdfs:domain uml-class:Vertex ;
	rdfs:range uml-class:Region ;
	mms-ontology:umlPropertySource uml-property:Vertex-container .

mms-property:containerRegionFromTransition a mms-ontology:UmlObjectProperty ;
	mms-ontology:cardinality "1"^^uml-model-dt:cardinalityRange ;
	mms-ontology:key "containerId" ;
	rdfs:label "containerRegionFromTransition" ;
	rdfs:comment "The Region that is the container of this Transition. Based on the UML property 'Transition-container' which is described as: Designates the Region that owns this Transition."@en ;
	rdfs:domain uml-class:Transition ;
	rdfs:range uml-class:Region ;
	mms-ontology:umlPropertySource uml-property:Transition-container .

mms-property:allowSubstitutableBoolean a mms-ontology:UmlDatatypeProperty ;
	mms-ontology:cardinality "1"^^uml-model-dt:cardinalityRange ;
	mms-ontology:key "allowSubstitutableId" ;
	rdfs:label "allowSubstitutableBoolean" ;
	rdfs:comment "The Boolean that is the allowSubstitutable of this ClassifierTemplateParameter. Based on the UML property 'ClassifierTemplateParameter-allowSubstitutable' which is described as: Constrains the required relationship between an actual parameter and the parameteredElement for this formal parameter."@en ;
	rdfs:domain uml-class:ClassifierTemplateParameter ;
	rdfs:range xsd:boolean ;
	mms-ontology:umlPropertySource uml-property:ClassifierTemplateParameter-allowSubstitutable .

mms-property:isDisjoint a mms-ontology:UmlDatatypeProperty ;
	mms-ontology:key "isDisjoint" ;
	rdfs:label "isDisjoint" ;
	rdfs:comment "Indicates whether or not the set of specific Classifiers in a Generalization relationship have instance in common. If isDisjoint is true, the specific Classifiers for a particular GeneralizationSet have no members in common; that is, their intersection is empty. If isDisjoint is false, the specific Classifiers in a particular GeneralizationSet have one or more members in common; that is, their intersection is not empty."@en ;
	rdfs:domain uml-class:GeneralizationSet ;
	rdfs:range xsd:boolean ;
	mms-ontology:umlPropertySource uml-property:GeneralizationSet-isDisjoint .

mms-property:isDisjointGeneralizationSet a mms-ontology:UmlDatatypeProperty ;
	owl:equivalentProperty mms-property:isDisjoint .

mms-property:specificClassifier a mms-ontology:UmlObjectProperty ;
	mms-ontology:cardinality "1"^^uml-model-dt:cardinalityRange ;
	mms-ontology:key "specificId" ;
	rdfs:label "specificClassifier" ;
	rdfs:comment "The Classifier that is the specific of this Generalization. Based on the UML property 'Generalization-specific' which is described as: The specializing Classifier in the Generalization relationship."@en ;
	rdfs:domain uml-class:Generalization ;
	rdfs:range uml-class:Classifier ;
	mms-ontology:umlPropertySource uml-property:Generalization-specific .

mms-property:nestedArtifact a mms-ontology:UmlObjectProperty ;
	mms-ontology:cardinality "*"^^uml-model-dt:cardinalityRange ;
	mms-ontology:key "nestedArtifactIds" ;
	rdfs:label "nestedArtifact" ;
	rdfs:comment "A Artifact that belongs to this Artifact. Based on the UML property 'Artifact-nestedArtifact' which is described as: The Artifacts that are defined (nested) within the Artifact. The association is a specialization of the ownedMember association from Namespace to NamedElement."@en ;
	rdfs:domain uml-class:Artifact ;
	rdfs:range uml-class:Artifact ;
	mms-ontology:umlPropertySource uml-property:Artifact-nestedArtifact .

mms-property:preConditionConstraint a mms-ontology:UmlObjectProperty ;
	mms-ontology:cardinality "1"^^uml-model-dt:cardinalityRange ;
	mms-ontology:key "preConditionId" ;
	rdfs:label "preConditionConstraint" ;
	rdfs:comment "The Constraint that is the preCondition of this ProtocolTransition. Based on the UML property 'ProtocolTransition-preCondition' which is described as: Specifies the precondition of the Transition. It specifies the Condition that should be verified before triggering the Transition. This guard condition added to the source State will be evaluated as part of the precondition of the Operation referred by the Transition if any."@en ;
	rdfs:domain uml-class:ProtocolTransition ;
	rdfs:range uml-class:Constraint ;
	mms-ontology:umlPropertySource uml-property:ProtocolTransition-preCondition .

mms-property:bodyPart a mms-ontology:UmlObjectProperty ;
	mms-ontology:cardinality "*"^^uml-model-dt:cardinalityRange ;
	mms-ontology:key "bodyPartIds" ;
	rdfs:label "bodyPart" ;
	rdfs:comment "A ExecutableNode that is the bodyPart of this LoopNode. Based on the UML property 'LoopNode-bodyPart' which is described as: The set of ExecutableNodes that perform the repetitive computations of the loop. The bodyPart is executed as long as the test section produces a true value."@en ;
	rdfs:domain uml-class:LoopNode ;
	rdfs:range uml-class:ExecutableNode ;
	mms-ontology:umlPropertySource uml-property:LoopNode-bodyPart .

mms-property:additionUseCase a mms-ontology:UmlObjectProperty ;
	mms-ontology:cardinality "1"^^uml-model-dt:cardinalityRange ;
	mms-ontology:key "additionId" ;
	rdfs:label "additionUseCase" ;
	rdfs:comment "The UseCase that is the addition of this Include. Based on the UML property 'Include-addition' which is described as: The UseCase that is to be included."@en ;
	rdfs:domain uml-class:Include ;
	rdfs:range uml-class:UseCase ;
	mms-ontology:umlPropertySource uml-property:Include-addition .

mms-property:removeAtInputPinFromRemoveStructuralFeatureValueAction a mms-ontology:UmlObjectProperty ;
	mms-ontology:cardinality "1"^^uml-model-dt:cardinalityRange ;
	mms-ontology:key "removeAtId" ;
	rdfs:label "removeAtInputPinFromRemoveStructuralFeatureValueAction" ;
	rdfs:comment "The InputPin that is the removeAt of this RemoveStructuralFeatureValueAction. Based on the UML property 'RemoveStructuralFeatureValueAction-removeAt' which is described as: An InputPin that provides the position of an existing value to remove in ordered, nonunique structural features. The type of the removeAt InputPin is UnlimitedNatural, but the value cannot be zero or unlimited."@en ;
	rdfs:domain uml-class:RemoveStructuralFeatureValueAction ;
	rdfs:range uml-class:InputPin ;
	mms-ontology:umlPropertySource uml-property:RemoveStructuralFeatureValueAction-removeAt .

mms-property:removeAtInputPinFromRemoveVariableValueAction a mms-ontology:UmlObjectProperty ;
	mms-ontology:cardinality "1"^^uml-model-dt:cardinalityRange ;
	mms-ontology:key "removeAtId" ;
	rdfs:label "removeAtInputPinFromRemoveVariableValueAction" ;
	rdfs:comment "The InputPin that is the removeAt of this RemoveVariableValueAction. Based on the UML property 'RemoveVariableValueAction-removeAt' which is described as: An InputPin that provides the position of an existing value to remove in ordered, nonunique Variables. The type of the removeAt InputPin is UnlimitedNatural, but the value cannot be zero or unlimited."@en ;
	rdfs:domain uml-class:RemoveVariableValueAction ;
	rdfs:range uml-class:InputPin ;
	mms-ontology:umlPropertySource uml-property:RemoveVariableValueAction-removeAt .

mms-property:endDataLinkEndData a mms-ontology:UmlObjectProperty ;
	mms-ontology:cardinality "*"^^uml-model-dt:cardinalityRange ;
	mms-ontology:key "endDataIds" ;
	rdfs:label "endDataLinkEndData" ;
	rdfs:comment "A LinkEndData that is the endData of this LinkAction. Based on the UML property 'LinkAction-endData' which is described as: The LinkEndData identifying the values on the ends of the links acting on by this LinkAction."@en ;
	rdfs:domain uml-class:LinkAction ;
	rdfs:range uml-class:LinkEndData ;
	mms-ontology:umlPropertySource uml-property:LinkAction-endData .

mms-property:endDataLinkEndCreationData a mms-ontology:UmlObjectProperty ;
	mms-ontology:cardinality "*"^^uml-model-dt:cardinalityRange ;
	mms-ontology:key "endDataIds" ;
	rdfs:label "endDataLinkEndCreationData" ;
	rdfs:comment "A LinkEndCreationData that is the endData of this CreateLinkAction. Based on the UML property 'CreateLinkAction-endData' which is described as: The LinkEndData that specifies the values to be placed on the Association ends for the new link."@en ;
	rdfs:domain uml-class:CreateLinkAction ;
	rdfs:range uml-class:LinkEndCreationData ;
	mms-ontology:umlPropertySource uml-property:CreateLinkAction-endData .

mms-property:endDataLinkEndDestructionData a mms-ontology:UmlObjectProperty ;
	mms-ontology:cardinality "*"^^uml-model-dt:cardinalityRange ;
	mms-ontology:key "endDataIds" ;
	rdfs:label "endDataLinkEndDestructionData" ;
	rdfs:comment "A LinkEndDestructionData that is the endData of this DestroyLinkAction. Based on the UML property 'DestroyLinkAction-endData' which is described as: The LinkEndData that the values of the Association ends for the links to be destroyed."@en ;
	rdfs:domain uml-class:DestroyLinkAction ;
	rdfs:range uml-class:LinkEndDestructionData ;
	mms-ontology:umlPropertySource uml-property:DestroyLinkAction-endData .

mms-property:contextBehavioredClassifier a mms-ontology:UmlObjectProperty ;
	mms-ontology:cardinality "1"^^uml-model-dt:cardinalityRange ;
	mms-ontology:key "contextId" ;
	rdfs:label "contextBehavioredClassifier" ;
	rdfs:comment "The BehavioredClassifier that is the context of this Behavior. Based on the UML property 'Behavior-context' which is described as: The BehavioredClassifier that is the context for the execution of the Behavior. A Behavior that is directly owned as a nestedClassifier does not have a context. Otherwise, to determine the context of a Behavior, find the first BehavioredClassifier reached by following the chain of owner relationships from the Behavior, if any. If there is such a BehavioredClassifier, then it is the context, unless it is itself a Behavior with a non-empty context, in which case that is also the context for the original Behavior. For example, following this algorithm, the context of an entry Behavior in a StateMachine is the BehavioredClassifier that owns the StateMachine. The features of the context BehavioredClassifier as well as the Elements visible to the context Classifier are visible to the Behavior."@en ;
	rdfs:domain uml-class:Behavior ;
	rdfs:range uml-class:BehavioredClassifier ;
	mms-ontology:umlPropertySource uml-property:Behavior-context .

mms-property:contextClassifier a mms-ontology:UmlObjectProperty ;
	mms-ontology:cardinality "1"^^uml-model-dt:cardinalityRange ;
	mms-ontology:key "contextId" ;
	rdfs:label "contextClassifier" ;
	rdfs:comment "The Classifier that is the context of this Action. Based on the UML property 'Action-context' which is described as: The context Classifier of the Behavior that contains this Action, or the Behavior itself if it has no context."@en ;
	rdfs:domain uml-class:Action ;
	rdfs:range uml-class:Classifier ;
	mms-ontology:umlPropertySource uml-property:Action-context .

mms-property:contextNamespace a mms-ontology:UmlObjectProperty ;
	mms-ontology:cardinality "1"^^uml-model-dt:cardinalityRange ;
	mms-ontology:key "contextId" ;
	rdfs:label "contextNamespace" ;
	rdfs:comment "The Namespace that is the context of this Constraint. Based on the UML property 'Constraint-context' which is described as: Specifies the Namespace that owns the Constraint."@en ;
	rdfs:domain uml-class:Constraint ;
	rdfs:range uml-class:Namespace ;
	mms-ontology:umlPropertySource uml-property:Constraint-context .

mms-property:profile a mms-ontology:UmlObjectProperty ;
	mms-ontology:cardinality "1"^^uml-model-dt:cardinalityRange ;
	mms-ontology:key "profileId" ;
	rdfs:label "profile" ;
	rdfs:comment "The Profile that belongs to this Stereotype. Based on the UML property 'Stereotype-profile' which is described as: The profile that directly or indirectly contains this stereotype."@en ;
	rdfs:domain uml-class:Stereotype ;
	rdfs:range uml-class:Profile ;
	mms-ontology:umlPropertySource uml-property:Stereotype-profile .

mms-property:attribute a mms-ontology:UmlObjectProperty ;
	mms-ontology:cardinality "*"^^uml-model-dt:cardinalityRange ;
	mms-ontology:key "attributeIds" ;
	rdfs:label "attribute" ;
	rdfs:comment "A Property that is the attribute of this Classifier. Based on the UML property 'Classifier-attribute' which is described as: All of the Properties that are direct (i.e., not inherited or imported) attributes of the Classifier."@en ;
	rdfs:domain uml-class:Classifier ;
	rdfs:range uml-class:Property ;
	mms-ontology:umlPropertySource uml-property:Classifier-attribute .

mms-property:generalizationFromClassifier a mms-ontology:UmlObjectProperty ;
	mms-ontology:cardinality "*"^^uml-model-dt:cardinalityRange ;
	mms-ontology:key "generalizationIds" ;
	rdfs:label "generalizationFromClassifier" ;
	rdfs:comment "A Generalization that belongs to this Classifier. Based on the UML property 'Classifier-generalization' which is described as: The Generalization relationships for this Classifier. These Generalizations navigate to more general Classifiers in the generalization hierarchy."@en ;
	rdfs:domain uml-class:Classifier ;
	rdfs:range uml-class:Generalization ;
	mms-ontology:umlPropertySource uml-property:Classifier-generalization .

mms-property:generalizationFromGeneralizationSet a mms-ontology:UmlObjectProperty ;
	mms-ontology:cardinality "*"^^uml-model-dt:cardinalityRange ;
	mms-ontology:key "generalizationIds" ;
	rdfs:label "generalizationFromGeneralizationSet" ;
	rdfs:comment "A Generalization that belongs to this GeneralizationSet. Based on the UML property 'GeneralizationSet-generalization' which is described as: Designates the instances of Generalization that are members of this GeneralizationSet."@en ;
	rdfs:domain uml-class:GeneralizationSet ;
	rdfs:range uml-class:Generalization ;
	mms-ontology:umlPropertySource uml-property:GeneralizationSet-generalization .

mms-property:substitutingClassifier a mms-ontology:UmlObjectProperty ;
	mms-ontology:cardinality "1"^^uml-model-dt:cardinalityRange ;
	mms-ontology:key "substitutingClassifierId" ;
	rdfs:label "substitutingClassifier" ;
	rdfs:comment "The Classifier that belongs to this Substitution. Based on the UML property 'Substitution-substitutingClassifier' which is described as: Instances of the substituting classifier are runtime substitutable where instances of the contract classifier are expected."@en ;
	rdfs:domain uml-class:Substitution ;
	rdfs:range uml-class:Classifier ;
	mms-ontology:umlPropertySource uml-property:Substitution-substitutingClassifier .

mms-property:isStream a mms-ontology:UmlDatatypeProperty ;
	mms-ontology:key "isStream" ;
	rdfs:label "isStream" ;
	rdfs:comment "Tells whether an input parameter may accept values while its behavior is executing, or whether an output parameter may post values while the behavior is executing."@en ;
	rdfs:domain uml-class:Parameter ;
	rdfs:range xsd:boolean ;
	mms-ontology:umlPropertySource uml-property:Parameter-isStream .

mms-property:isStreamParameter a mms-ontology:UmlDatatypeProperty ;
	owl:equivalentProperty mms-property:isStream .

mms-property:specificationDurationInterval a mms-ontology:UmlObjectProperty ;
	mms-ontology:cardinality "1"^^uml-model-dt:cardinalityRange ;
	mms-ontology:key "specificationId" ;
	rdfs:label "specificationDurationInterval" ;
	rdfs:comment "The DurationInterval that is the specification of this DurationConstraint. Based on the UML property 'DurationConstraint-specification' which is described as: The DurationInterval constraining the duration."@en ;
	rdfs:domain uml-class:DurationConstraint ;
	rdfs:range uml-class:DurationInterval ;
	mms-ontology:umlPropertySource uml-property:DurationConstraint-specification .

mms-property:specificationValueSpecificationFromConstraint a mms-ontology:UmlObjectProperty ;
	mms-ontology:cardinality "1"^^uml-model-dt:cardinalityRange ;
	mms-ontology:key "specificationId" ;
	rdfs:label "specificationValueSpecificationFromConstraint" ;
	rdfs:comment "The ValueSpecification that is the specification of this Constraint. Based on the UML property 'Constraint-specification' which is described as: A condition that must be true when evaluated in order for the Constraint to be satisfied."@en ;
	rdfs:domain uml-class:Constraint ;
	rdfs:range uml-class:ValueSpecification ;
	mms-ontology:umlPropertySource uml-property:Constraint-specification .

mms-property:specificationValueSpecificationFromInstanceSpecification a mms-ontology:UmlObjectProperty ;
	mms-ontology:cardinality "1"^^uml-model-dt:cardinalityRange ;
	mms-ontology:key "specificationId" ;
	rdfs:label "specificationValueSpecificationFromInstanceSpecification" ;
	rdfs:comment "The ValueSpecification that is the specification of this InstanceSpecification. Based on the UML property 'InstanceSpecification-specification' which is described as: A specification of how to compute, derive, or construct the instance."@en ;
	rdfs:domain uml-class:InstanceSpecification ;
	rdfs:range uml-class:ValueSpecification ;
	mms-ontology:umlPropertySource uml-property:InstanceSpecification-specification .

mms-property:specificationTimeInterval a mms-ontology:UmlObjectProperty ;
	mms-ontology:cardinality "1"^^uml-model-dt:cardinalityRange ;
	mms-ontology:key "specificationId" ;
	rdfs:label "specificationTimeInterval" ;
	rdfs:comment "The TimeInterval that is the specification of this TimeConstraint. Based on the UML property 'TimeConstraint-specification' which is described as: TheTimeInterval constraining the duration."@en ;
	rdfs:domain uml-class:TimeConstraint ;
	rdfs:range uml-class:TimeInterval ;
	mms-ontology:umlPropertySource uml-property:TimeConstraint-specification .

mms-property:specificationBehavioralFeature a mms-ontology:UmlObjectProperty ;
	mms-ontology:cardinality "1"^^uml-model-dt:cardinalityRange ;
	mms-ontology:key "specificationId" ;
	rdfs:label "specificationBehavioralFeature" ;
	rdfs:comment "The BehavioralFeature that is the specification of this Behavior. Based on the UML property 'Behavior-specification' which is described as: Designates a BehavioralFeature that the Behavior implements. The BehavioralFeature must be owned by the BehavioredClassifier that owns the Behavior or be inherited by it. The Parameters of the BehavioralFeature and the implementing Behavior must match. A Behavior does not need to have a specification, in which case it either is the classifierBehavior of a BehavioredClassifier or it can only be invoked by another Behavior of the Classifier."@en ;
	rdfs:domain uml-class:Behavior ;
	rdfs:range uml-class:BehavioralFeature ;
	mms-ontology:umlPropertySource uml-property:Behavior-specification .

mms-property:specificationInterval a mms-ontology:UmlObjectProperty ;
	mms-ontology:cardinality "1"^^uml-model-dt:cardinalityRange ;
	mms-ontology:key "specificationId" ;
	rdfs:label "specificationInterval" ;
	rdfs:comment "The Interval that is the specification of this IntervalConstraint. Based on the UML property 'IntervalConstraint-specification' which is described as: The Interval that specifies the condition of the IntervalConstraint."@en ;
	rdfs:domain uml-class:IntervalConstraint ;
	rdfs:range uml-class:Interval ;
	mms-ontology:umlPropertySource uml-property:IntervalConstraint-specification .

mms-property:firstEventsFromDurationConstraint a mms-ontology:UmlDatatypeProperty ;
	mms-ontology:cardinality "2"^^uml-model-dt:cardinalityRange ;
	mms-ontology:key "firstEventIds" ;
	rdfs:label "firstEventsFromDurationConstraint" ;
	rdfs:comment "List of Booleans that are the firstEvent of this DurationConstraint. Based on the UML property 'DurationConstraint-firstEvent' which is described as: The value of firstEvent[i] is related to constrainedElement[i] (where i is 1 or 2). If firstEvent[i] is true, then the corresponding observation event is the first time instant the execution enters constrainedElement[i]. If firstEvent[i] is false, then the corresponding observation event is the last time instant the execution is within constrainedElement[i]."@en ;
	rdfs:domain uml-class:DurationConstraint ;
	rdfs:range mms-class:FirstEventsFromDurationConstraintList ;
	mms-ontology:listItemRange xsd:boolean ;
	mms-ontology:umlPropertySource uml-property:DurationConstraint-firstEvent .

mms-class:FirstEventsFromDurationConstraintList a owl:Class ;
	mms-ontology:category mms-class:ElementList ;
	rdfs:subClassOf [
		rdf:type owl:Class ;
		owl:intersectionOf (
			rdf:List
			[
				rdf:type owl:Restriction ;
				owl:onProperty rdf:first ;
				owl:allValuesFrom xsd:boolean ;
			]
			[
				rdf:type owl:Restriction ;
				owl:onProperty rdf:rest ;
				owl:allValuesFrom mms-class:FirstEventsFromDurationConstraintList ;
			]
		) ;
	] .

mms-property:firstEventsFromDurationObservation a mms-ontology:UmlDatatypeProperty ;
	mms-ontology:cardinality "2"^^uml-model-dt:cardinalityRange ;
	mms-ontology:key "firstEventIds" ;
	rdfs:label "firstEventsFromDurationObservation" ;
	rdfs:comment "List of Booleans that are the firstEvent of this DurationObservation. Based on the UML property 'DurationObservation-firstEvent' which is described as: The value of firstEvent[i] is related to event[i] (where i is 1 or 2). If firstEvent[i] is true, then the corresponding observation event is the first time instant the execution enters event[i]. If firstEvent[i] is false, then the corresponding observation event is the time instant the execution exits event[i]."@en ;
	rdfs:domain uml-class:DurationObservation ;
	rdfs:range mms-class:FirstEventsFromDurationObservationList ;
	mms-ontology:listItemRange xsd:boolean ;
	mms-ontology:umlPropertySource uml-property:DurationObservation-firstEvent .

mms-class:FirstEventsFromDurationObservationList a owl:Class ;
	mms-ontology:category mms-class:ElementList ;
	rdfs:subClassOf [
		rdf:type owl:Class ;
		owl:intersectionOf (
			rdf:List
			[
				rdf:type owl:Restriction ;
				owl:onProperty rdf:first ;
				owl:allValuesFrom xsd:boolean ;
			]
			[
				rdf:type owl:Restriction ;
				owl:onProperty rdf:rest ;
				owl:allValuesFrom mms-class:FirstEventsFromDurationObservationList ;
			]
		) ;
	] .

mms-property:firstEventBooleanFromTimeObservation a mms-ontology:UmlDatatypeProperty ;
	mms-ontology:cardinality "1"^^uml-model-dt:cardinalityRange ;
	mms-ontology:key "firstEventId" ;
	rdfs:label "firstEventBooleanFromTimeObservation" ;
	rdfs:comment "The Boolean that is the firstEvent of this TimeObservation. Based on the UML property 'TimeObservation-firstEvent' which is described as: The value of firstEvent is related to the event. If firstEvent is true, then the corresponding observation event is the first time instant the execution enters the event Element. If firstEvent is false, then the corresponding observation event is the time instant the execution exits the event Element."@en ;
	rdfs:domain uml-class:TimeObservation ;
	rdfs:range xsd:boolean ;
	mms-ontology:umlPropertySource uml-property:TimeObservation-firstEvent .

mms-property:firstEventBooleanFromTimeConstraint a mms-ontology:UmlDatatypeProperty ;
	mms-ontology:cardinality "1"^^uml-model-dt:cardinalityRange ;
	mms-ontology:key "firstEventId" ;
	rdfs:label "firstEventBooleanFromTimeConstraint" ;
	rdfs:comment "The Boolean that is the firstEvent of this TimeConstraint. Based on the UML property 'TimeConstraint-firstEvent' which is described as: The value of firstEvent is related to the constrainedElement. If firstEvent is true, then the corresponding observation event is the first time instant the execution enters the constrainedElement. If firstEvent is false, then the corresponding observation event is the last time instant the execution is within the constrainedElement."@en ;
	rdfs:domain uml-class:TimeConstraint ;
	rdfs:range xsd:boolean ;
	mms-ontology:umlPropertySource uml-property:TimeConstraint-firstEvent .

mms-property:locationString a mms-ontology:UmlDatatypeProperty ;
	mms-ontology:cardinality "1"^^uml-model-dt:cardinalityRange ;
	mms-ontology:key "locationId" ;
	rdfs:label "locationString" ;
	rdfs:comment "The String that is the location of this Image. Based on the UML property 'Image-location' which is described as: This contains a location that can be used by a tool to locate the image as an alternative to embedding it in the stereotype."@en ;
	rdfs:domain uml-class:Image ;
	rdfs:range xsd:string ;
	mms-ontology:umlPropertySource uml-property:Image-location .

mms-property:locationDeploymentTarget a mms-ontology:UmlObjectProperty ;
	mms-ontology:cardinality "1"^^uml-model-dt:cardinalityRange ;
	mms-ontology:key "locationId" ;
	rdfs:label "locationDeploymentTarget" ;
	rdfs:comment "The DeploymentTarget that is the location of this Deployment. Based on the UML property 'Deployment-location' which is described as: The DeployedTarget which is the target of a Deployment."@en ;
	rdfs:domain uml-class:Deployment ;
	rdfs:range uml-class:DeploymentTarget ;
	mms-ontology:umlPropertySource uml-property:Deployment-location .

mms-property:incomingActivityEdge a mms-ontology:UmlObjectProperty ;
	mms-ontology:cardinality "*"^^uml-model-dt:cardinalityRange ;
	mms-ontology:key "incomingIds" ;
	rdfs:label "incomingActivityEdge" ;
	rdfs:comment "A ActivityEdge that is the incoming of this ActivityNode. Based on the UML property 'ActivityNode-incoming' which is described as: ActivityEdges that have the ActivityNode as their target."@en ;
	rdfs:domain uml-class:ActivityNode ;
	rdfs:range uml-class:ActivityEdge ;
	mms-ontology:umlPropertySource uml-property:ActivityNode-incoming .

mms-property:incomingTransition a mms-ontology:UmlObjectProperty ;
	mms-ontology:cardinality "*"^^uml-model-dt:cardinalityRange ;
	mms-ontology:key "incomingIds" ;
	rdfs:label "incomingTransition" ;
	rdfs:comment "A Transition that is the incoming of this Vertex. Based on the UML property 'Vertex-incoming' which is described as: Specifies the Transitions entering this Vertex."@en ;
	rdfs:domain uml-class:Vertex ;
	rdfs:range uml-class:Transition ;
	mms-ontology:umlPropertySource uml-property:Vertex-incoming .

mms-property:upperValueValueSpecification a mms-ontology:UmlObjectProperty ;
	mms-ontology:cardinality "1"^^uml-model-dt:cardinalityRange ;
	mms-ontology:key "upperValueId" ;
	rdfs:label "upperValueValueSpecification" ;
	rdfs:comment "The ValueSpecification that is the upperValue of this MultiplicityElement. Based on the UML property 'MultiplicityElement-upperValue' which is described as: The specification of the upper bound for this multiplicity."@en ;
	rdfs:domain uml-class:MultiplicityElement ;
	rdfs:range uml-class:ValueSpecification ;
	mms-ontology:umlPropertySource uml-property:MultiplicityElement-upperValue .

mms-property:supplier a mms-ontology:UmlObjectProperty ;
	mms-ontology:cardinality "*"^^uml-model-dt:cardinalityRange ;
	mms-ontology:key "supplierIds" ;
	rdfs:label "supplier" ;
	rdfs:comment "A NamedElement that is the supplier of this Dependency. Based on the UML property 'Dependency-supplier' which is described as: The Element(s) on which the client Element(s) depend in some respect. The modeler may stipulate a sense of Dependency direction suitable for their domain."@en ;
	rdfs:domain uml-class:Dependency ;
	rdfs:range uml-class:NamedElement ;
	mms-ontology:umlPropertySource uml-property:Dependency-supplier .

mms-property:secondInputPin a mms-ontology:UmlObjectProperty ;
	mms-ontology:cardinality "1"^^uml-model-dt:cardinalityRange ;
	mms-ontology:key "secondId" ;
	rdfs:label "secondInputPin" ;
	rdfs:comment "The InputPin that is the second of this TestIdentityAction. Based on the UML property 'TestIdentityAction-second' which is described as: The OutputPin on which the second input object is placed."@en ;
	rdfs:domain uml-class:TestIdentityAction ;
	rdfs:range uml-class:InputPin ;
	mms-ontology:umlPropertySource uml-property:TestIdentityAction-second .

mms-property:minValueSpecification a mms-ontology:UmlObjectProperty ;
	mms-ontology:cardinality "1"^^uml-model-dt:cardinalityRange ;
	mms-ontology:key "minId" ;
	rdfs:label "minValueSpecification" ;
	rdfs:comment "The ValueSpecification that is the min of this Interval. Based on the UML property 'Interval-min' which is described as: Refers to the ValueSpecification denoting the minimum value of the range."@en ;
	rdfs:domain uml-class:Interval ;
	rdfs:range uml-class:ValueSpecification ;
	mms-ontology:umlPropertySource uml-property:Interval-min .

mms-property:minTimeExpression a mms-ontology:UmlObjectProperty ;
	mms-ontology:cardinality "1"^^uml-model-dt:cardinalityRange ;
	mms-ontology:key "minId" ;
	rdfs:label "minTimeExpression" ;
	rdfs:comment "The TimeExpression that is the min of this TimeInterval. Based on the UML property 'TimeInterval-min' which is described as: Refers to the TimeExpression denoting the minimum value of the range."@en ;
	rdfs:domain uml-class:TimeInterval ;
	rdfs:range uml-class:TimeExpression ;
	mms-ontology:umlPropertySource uml-property:TimeInterval-min .

mms-property:minDuration a mms-ontology:UmlObjectProperty ;
	mms-ontology:cardinality "1"^^uml-model-dt:cardinalityRange ;
	mms-ontology:key "minId" ;
	rdfs:label "minDuration" ;
	rdfs:comment "The Duration that is the min of this DurationInterval. Based on the UML property 'DurationInterval-min' which is described as: Refers to the Duration denoting the minimum value of the range."@en ;
	rdfs:domain uml-class:DurationInterval ;
	rdfs:range uml-class:Duration ;
	mms-ontology:umlPropertySource uml-property:DurationInterval-min .

mms-property:maxValueSpecification a mms-ontology:UmlObjectProperty ;
	mms-ontology:cardinality "1"^^uml-model-dt:cardinalityRange ;
	mms-ontology:key "maxId" ;
	rdfs:label "maxValueSpecification" ;
	rdfs:comment "The ValueSpecification that is the max of this Interval. Based on the UML property 'Interval-max' which is described as: Refers to the ValueSpecification denoting the maximum value of the range."@en ;
	rdfs:domain uml-class:Interval ;
	rdfs:range uml-class:ValueSpecification ;
	mms-ontology:umlPropertySource uml-property:Interval-max .

mms-property:maxTimeExpression a mms-ontology:UmlObjectProperty ;
	mms-ontology:cardinality "1"^^uml-model-dt:cardinalityRange ;
	mms-ontology:key "maxId" ;
	rdfs:label "maxTimeExpression" ;
	rdfs:comment "The TimeExpression that is the max of this TimeInterval. Based on the UML property 'TimeInterval-max' which is described as: Refers to the TimeExpression denoting the maximum value of the range."@en ;
	rdfs:domain uml-class:TimeInterval ;
	rdfs:range uml-class:TimeExpression ;
	mms-ontology:umlPropertySource uml-property:TimeInterval-max .

mms-property:maxDuration a mms-ontology:UmlObjectProperty ;
	mms-ontology:cardinality "1"^^uml-model-dt:cardinalityRange ;
	mms-ontology:key "maxId" ;
	rdfs:label "maxDuration" ;
	rdfs:comment "The Duration that is the max of this DurationInterval. Based on the UML property 'DurationInterval-max' which is described as: Refers to the Duration denoting the maximum value of the range."@en ;
	rdfs:domain uml-class:DurationInterval ;
	rdfs:range uml-class:Duration ;
	mms-ontology:umlPropertySource uml-property:DurationInterval-max .

mms-property:ownedParameterSetFromBehavioralFeature a mms-ontology:UmlObjectProperty ;
	mms-ontology:cardinality "*"^^uml-model-dt:cardinalityRange ;
	mms-ontology:key "ownedParameterSetIds" ;
	rdfs:label "ownedParameterSetFromBehavioralFeature" ;
	rdfs:comment "A ParameterSet that belongs to this BehavioralFeature. Based on the UML property 'BehavioralFeature-ownedParameterSet' which is described as: The ParameterSets owned by this BehavioralFeature."@en ;
	rdfs:domain uml-class:BehavioralFeature ;
	rdfs:range uml-class:ParameterSet ;
	mms-ontology:umlPropertySource uml-property:BehavioralFeature-ownedParameterSet .

mms-property:ownedParameterSetFromBehavior a mms-ontology:UmlObjectProperty ;
	mms-ontology:cardinality "*"^^uml-model-dt:cardinalityRange ;
	mms-ontology:key "ownedParameterSetIds" ;
	rdfs:label "ownedParameterSetFromBehavior" ;
	rdfs:comment "A ParameterSet that belongs to this Behavior. Based on the UML property 'Behavior-ownedParameterSet' which is described as: The ParameterSets owned by this Behavior."@en ;
	rdfs:domain uml-class:Behavior ;
	rdfs:range uml-class:ParameterSet ;
	mms-ontology:umlPropertySource uml-property:Behavior-ownedParameterSet .

mms-property:memberEnd a mms-ontology:UmlObjectProperty ;
	mms-ontology:cardinality "*"^^uml-model-dt:cardinalityRange ;
	mms-ontology:key "memberEndIds" ;
	rdfs:label "memberEnd" ;
	rdfs:comment "A Property that is the memberEnd of this Association. Based on the UML property 'Association-memberEnd' which is described as: Each end represents participation of instances of the Classifier connected to the end in links of the Association."@en ;
	rdfs:domain uml-class:Association ;
	rdfs:range uml-class:Property ;
	mms-ontology:umlPropertySource uml-property:Association-memberEnd .

mms-property:isQuery a mms-ontology:UmlDatatypeProperty ;
	mms-ontology:key "isQuery" ;
	rdfs:label "isQuery" ;
	rdfs:comment "Specifies whether an execution of the BehavioralFeature leaves the state of the system unchanged (isQuery=true) or whether side effects may occur (isQuery=false)."@en ;
	rdfs:domain uml-class:Operation ;
	rdfs:range xsd:boolean ;
	mms-ontology:umlPropertySource uml-property:Operation-isQuery .

mms-property:isQueryOperation a mms-ontology:UmlDatatypeProperty ;
	owl:equivalentProperty mms-property:isQuery .

mms-property:extensionUseCase a mms-ontology:UmlObjectProperty ;
	mms-ontology:cardinality "1"^^uml-model-dt:cardinalityRange ;
	mms-ontology:key "extensionId" ;
	rdfs:label "extensionUseCase" ;
	rdfs:comment "The UseCase that is the extension of this Extend. Based on the UML property 'Extend-extension' which is described as: The UseCase that represents the extension and owns the Extend relationship."@en ;
	rdfs:domain uml-class:Extend ;
	rdfs:range uml-class:UseCase ;
	mms-ontology:umlPropertySource uml-property:Extend-extension .

mms-property:extension a mms-ontology:UmlObjectProperty ;
	mms-ontology:cardinality "*"^^uml-model-dt:cardinalityRange ;
	mms-ontology:key "extensionIds" ;
	rdfs:label "extension" ;
	rdfs:comment "A Extension that belongs to this Class. Based on the UML property 'Class-extension' which is described as: This property is used when the Class is acting as a metaclass. It references the Extensions that specify additional properties of the metaclass. The property is derived from the Extensions whose memberEnds are typed by the Class."@en ;
	rdfs:domain uml-class:Class ;
	rdfs:range uml-class:Extension ;
	mms-ontology:umlPropertySource uml-property:Class-extension .

mms-property:requiredFromComponent a mms-ontology:UmlObjectProperty ;
	mms-ontology:cardinality "*"^^uml-model-dt:cardinalityRange ;
	mms-ontology:key "requiredIds" ;
	rdfs:label "requiredFromComponent" ;
	rdfs:comment "A Interface that is the required of this Component. Based on the UML property 'Component-required' which is described as: The Interfaces that the Component requires from other Components in its environment in order to be able to offer its full set of provided functionality. These Interfaces may be used by the Component or any of its realizingClassifiers, or they may be the Interfaces that are required by its public Ports."@en ;
	rdfs:domain uml-class:Component ;
	rdfs:range uml-class:Interface ;
	mms-ontology:umlPropertySource uml-property:Component-required .

mms-property:requiredFromPort a mms-ontology:UmlObjectProperty ;
	mms-ontology:cardinality "*"^^uml-model-dt:cardinalityRange ;
	mms-ontology:key "requiredIds" ;
	rdfs:label "requiredFromPort" ;
	rdfs:comment "A Interface that is the required of this Port. Based on the UML property 'Port-required' which is described as: The Interfaces specifying the set of Operations and Receptions that the EncapsulatedCassifier expects its environment to handle via this port. This association is derived according to the value of isConjugated. If isConjugated is false, required is derived as the union of the sets of Interfaces used by the type of the Port and its supertypes. If isConjugated is true, it is derived as the union of the sets of Interfaces realized by the type of the Port and its supertypes, or directly from the type of the Port if the Port is typed by an Interface."@en ;
	rdfs:domain uml-class:Port ;
	rdfs:range uml-class:Interface ;
	mms-ontology:umlPropertySource uml-property:Port-required .

mms-property:beforeOccurrenceSpecification a mms-ontology:UmlObjectProperty ;
	mms-ontology:cardinality "1"^^uml-model-dt:cardinalityRange ;
	mms-ontology:key "beforeId" ;
	rdfs:label "beforeOccurrenceSpecification" ;
	rdfs:comment "The OccurrenceSpecification that is the before of this GeneralOrdering. Based on the UML property 'GeneralOrdering-before' which is described as: The OccurrenceSpecification referenced comes before the OccurrenceSpecification referenced by after."@en ;
	rdfs:domain uml-class:GeneralOrdering ;
	rdfs:range uml-class:OccurrenceSpecification ;
	mms-ontology:umlPropertySource uml-property:GeneralOrdering-before .

mms-property:stateMachineFromPseudostate a mms-ontology:UmlObjectProperty ;
	mms-ontology:cardinality "1"^^uml-model-dt:cardinalityRange ;
	mms-ontology:key "stateMachineId" ;
	rdfs:label "stateMachineFromPseudostate" ;
	rdfs:comment "The StateMachine that belongs to this Pseudostate. Based on the UML property 'Pseudostate-stateMachine' which is described as: The StateMachine in which this Pseudostate is defined. This only applies to Pseudostates of the kind entryPoint or exitPoint."@en ;
	rdfs:domain uml-class:Pseudostate ;
	rdfs:range uml-class:StateMachine ;
	mms-ontology:umlPropertySource uml-property:Pseudostate-stateMachine .

mms-property:stateMachineFromRegion a mms-ontology:UmlObjectProperty ;
	mms-ontology:cardinality "1"^^uml-model-dt:cardinalityRange ;
	mms-ontology:key "stateMachineId" ;
	rdfs:label "stateMachineFromRegion" ;
	rdfs:comment "The StateMachine that belongs to this Region. Based on the UML property 'Region-stateMachine' which is described as: The StateMachine that owns the Region. If a Region is owned by a StateMachine, then it cannot also be owned by a State."@en ;
	rdfs:domain uml-class:Region ;
	rdfs:range uml-class:StateMachine ;
	mms-ontology:umlPropertySource uml-property:Region-stateMachine .

mms-property:subpartition a mms-ontology:UmlObjectProperty ;
	mms-ontology:cardinality "*"^^uml-model-dt:cardinalityRange ;
	mms-ontology:key "subpartitionIds" ;
	rdfs:label "subpartition" ;
	rdfs:comment "A ActivityPartition that is the subpartition of this ActivityPartition. Based on the UML property 'ActivityPartition-subpartition' which is described as: Other ActivityPartitions immediately contained in this ActivityPartition (as its subgroups)."@en ;
	rdfs:domain uml-class:ActivityPartition ;
	rdfs:range uml-class:ActivityPartition ;
	mms-ontology:umlPropertySource uml-property:ActivityPartition-subpartition .

mms-property:subgroup a mms-ontology:UmlObjectProperty ;
	mms-ontology:cardinality "*"^^uml-model-dt:cardinalityRange ;
	mms-ontology:key "subgroupIds" ;
	rdfs:label "subgroup" ;
	rdfs:comment "A ActivityGroup that is the subgroup of this ActivityGroup. Based on the UML property 'ActivityGroup-subgroup' which is described as: Other ActivityGroups immediately contained in this ActivityGroup."@en ;
	rdfs:domain uml-class:ActivityGroup ;
	rdfs:range uml-class:ActivityGroup ;
	mms-ontology:umlPropertySource uml-property:ActivityGroup-subgroup .

mms-property:unmarshallTypeClassifier a mms-ontology:UmlObjectProperty ;
	mms-ontology:cardinality "1"^^uml-model-dt:cardinalityRange ;
	mms-ontology:key "unmarshallTypeId" ;
	rdfs:label "unmarshallTypeClassifier" ;
	rdfs:comment "The Classifier that is the unmarshallType of this UnmarshallAction. Based on the UML property 'UnmarshallAction-unmarshallType' which is described as: The type of the object to be unmarshalled."@en ;
	rdfs:domain uml-class:UnmarshallAction ;
	rdfs:range uml-class:Classifier ;
	mms-ontology:umlPropertySource uml-property:UnmarshallAction-unmarshallType .

mms-property:datatypeFromProperty a mms-ontology:UmlObjectProperty ;
	mms-ontology:cardinality "1"^^uml-model-dt:cardinalityRange ;
	mms-ontology:key "datatypeId" ;
	rdfs:label "datatypeFromProperty" ;
	rdfs:comment "The DataType that belongs to this Property. Based on the UML property 'Property-datatype' which is described as: The DataType that owns this Property, if any."@en ;
	rdfs:domain uml-class:Property ;
	rdfs:range uml-class:DataType ;
	mms-ontology:umlPropertySource uml-property:Property-datatype .

mms-property:datatypeFromOperation a mms-ontology:UmlObjectProperty ;
	mms-ontology:cardinality "1"^^uml-model-dt:cardinalityRange ;
	mms-ontology:key "datatypeId" ;
	rdfs:label "datatypeFromOperation" ;
	rdfs:comment "The DataType that belongs to this Operation. Based on the UML property 'Operation-datatype' which is described as: The DataType that owns this Operation, if any."@en ;
	rdfs:domain uml-class:Operation ;
	rdfs:range uml-class:DataType ;
	mms-ontology:umlPropertySource uml-property:Operation-datatype .

mms-property:interfaceFromOperation a mms-ontology:UmlObjectProperty ;
	mms-ontology:cardinality "1"^^uml-model-dt:cardinalityRange ;
	mms-ontology:key "interfaceId" ;
	rdfs:label "interfaceFromOperation" ;
	rdfs:comment "The Interface that belongs to this Operation. Based on the UML property 'Operation-interface' which is described as: The Interface that owns this Operation, if any."@en ;
	rdfs:domain uml-class:Operation ;
	rdfs:range uml-class:Interface ;
	mms-ontology:umlPropertySource uml-property:Operation-interface .

mms-property:interfaceFromProperty a mms-ontology:UmlObjectProperty ;
	mms-ontology:cardinality "1"^^uml-model-dt:cardinalityRange ;
	mms-ontology:key "interfaceId" ;
	rdfs:label "interfaceFromProperty" ;
	rdfs:comment "The Interface that belongs to this Property. Based on the UML property 'Property-interface' which is described as: The Interface that owns this Property, if any."@en ;
	rdfs:domain uml-class:Property ;
	rdfs:range uml-class:Interface ;
	mms-ontology:umlPropertySource uml-property:Property-interface .

mms-property:port a mms-ontology:UmlObjectProperty ;
	mms-ontology:cardinality "*"^^uml-model-dt:cardinalityRange ;
	mms-ontology:key "portIds" ;
	rdfs:label "port" ;
	rdfs:comment "A Port that belongs to this Trigger. Based on the UML property 'Trigger-port' which is described as: A optional Port of through which the given effect is detected."@en ;
	rdfs:domain uml-class:Trigger ;
	rdfs:range uml-class:Port ;
	mms-ontology:umlPropertySource uml-property:Trigger-port .

mms-property:bodyConditionConstraint a mms-ontology:UmlObjectProperty ;
	mms-ontology:cardinality "1"^^uml-model-dt:cardinalityRange ;
	mms-ontology:key "bodyConditionId" ;
	rdfs:label "bodyConditionConstraint" ;
	rdfs:comment "The Constraint that is the bodyCondition of this Operation. Based on the UML property 'Operation-bodyCondition' which is described as: An optional Constraint on the result values of an invocation of this Operation."@en ;
	rdfs:domain uml-class:Operation ;
	rdfs:range uml-class:Constraint ;
	mms-ontology:umlPropertySource uml-property:Operation-bodyCondition .

mms-property:contractInterface a mms-ontology:UmlObjectProperty ;
	mms-ontology:cardinality "1"^^uml-model-dt:cardinalityRange ;
	mms-ontology:key "contractId" ;
	rdfs:label "contractInterface" ;
	rdfs:comment "The Interface that is the contract of this InterfaceRealization. Based on the UML property 'InterfaceRealization-contract' which is described as: References the Interface specifying the conformance contract."@en ;
	rdfs:domain uml-class:InterfaceRealization ;
	rdfs:range uml-class:Interface ;
	mms-ontology:umlPropertySource uml-property:InterfaceRealization-contract .

mms-property:contractClassifier a mms-ontology:UmlObjectProperty ;
	mms-ontology:cardinality "1"^^uml-model-dt:cardinalityRange ;
	mms-ontology:key "contractId" ;
	rdfs:label "contractClassifier" ;
	rdfs:comment "The Classifier that is the contract of this Substitution. Based on the UML property 'Substitution-contract' which is described as: The contract with which the substituting classifier complies."@en ;
	rdfs:domain uml-class:Substitution ;
	rdfs:range uml-class:Classifier ;
	mms-ontology:umlPropertySource uml-property:Substitution-contract .

mms-property:contractBehavior a mms-ontology:UmlObjectProperty ;
	mms-ontology:cardinality "*"^^uml-model-dt:cardinalityRange ;
	mms-ontology:key "contractIds" ;
	rdfs:label "contractBehavior" ;
	rdfs:comment "A Behavior that is the contract of this Connector. Based on the UML property 'Connector-contract' which is described as: The set of Behaviors that specify the valid interaction patterns across the Connector."@en ;
	rdfs:domain uml-class:Connector ;
	rdfs:range uml-class:Behavior ;
	mms-ontology:umlPropertySource uml-property:Connector-contract .

mms-property:ownerElement a mms-ontology:UmlObjectProperty ;
	mms-ontology:cardinality "1"^^uml-model-dt:cardinalityRange ;
	mms-ontology:key "ownerId" ;
	rdfs:label "ownerElement" ;
	rdfs:comment "The Element that is the owner of this Element. Based on the UML property 'Element-owner' which is described as: The Element that owns this Element."@en ;
	rdfs:domain uml-class:Element ;
	rdfs:range uml-class:Element ;
	mms-ontology:umlPropertySource uml-property:Element-owner .

mms-property:activityFromActivityNode a mms-ontology:UmlObjectProperty ;
	mms-ontology:cardinality "1"^^uml-model-dt:cardinalityRange ;
	mms-ontology:key "activityId" ;
	rdfs:label "activityFromActivityNode" ;
	rdfs:comment "The Activity that belongs to this ActivityNode. Based on the UML property 'ActivityNode-activity' which is described as: The Activity containing the ActivityNode, if it is directly owned by an Activity."@en ;
	rdfs:domain uml-class:ActivityNode ;
	rdfs:range uml-class:Activity ;
	mms-ontology:umlPropertySource uml-property:ActivityNode-activity .

mms-property:activityFromStructuredActivityNode a mms-ontology:UmlObjectProperty ;
	mms-ontology:cardinality "1"^^uml-model-dt:cardinalityRange ;
	mms-ontology:key "activityId" ;
	rdfs:label "activityFromStructuredActivityNode" ;
	rdfs:comment "The Activity that belongs to this StructuredActivityNode. Based on the UML property 'StructuredActivityNode-activity' which is described as: The Activity immediately containing the StructuredActivityNode, if it is not contained in another StructuredActivityNode."@en ;
	rdfs:domain uml-class:StructuredActivityNode ;
	rdfs:range uml-class:Activity ;
	mms-ontology:umlPropertySource uml-property:StructuredActivityNode-activity .

mms-property:activityFromActivityEdge a mms-ontology:UmlObjectProperty ;
	mms-ontology:cardinality "1"^^uml-model-dt:cardinalityRange ;
	mms-ontology:key "activityId" ;
	rdfs:label "activityFromActivityEdge" ;
	rdfs:comment "The Activity that belongs to this ActivityEdge. Based on the UML property 'ActivityEdge-activity' which is described as: The Activity containing the ActivityEdge, if it is directly owned by an Activity."@en ;
	rdfs:domain uml-class:ActivityEdge ;
	rdfs:range uml-class:Activity ;
	mms-ontology:umlPropertySource uml-property:ActivityEdge-activity .

mms-property:inPartitionFromActivityNode a mms-ontology:UmlObjectProperty ;
	mms-ontology:cardinality "*"^^uml-model-dt:cardinalityRange ;
	mms-ontology:key "inPartitionIds" ;
	rdfs:label "inPartitionFromActivityNode" ;
	rdfs:comment "A ActivityPartition that is the inPartition of this ActivityNode. Based on the UML property 'ActivityNode-inPartition' which is described as: ActivityPartitions containing the ActivityNode."@en ;
	rdfs:domain uml-class:ActivityNode ;
	rdfs:range uml-class:ActivityPartition ;
	mms-ontology:umlPropertySource uml-property:ActivityNode-inPartition .

mms-property:inPartitionFromActivityEdge a mms-ontology:UmlObjectProperty ;
	mms-ontology:cardinality "*"^^uml-model-dt:cardinalityRange ;
	mms-ontology:key "inPartitionIds" ;
	rdfs:label "inPartitionFromActivityEdge" ;
	rdfs:comment "A ActivityPartition that is the inPartition of this ActivityEdge. Based on the UML property 'ActivityEdge-inPartition' which is described as: ActivityPartitions containing the ActivityEdge."@en ;
	rdfs:domain uml-class:ActivityEdge ;
	rdfs:range uml-class:ActivityPartition ;
	mms-ontology:umlPropertySource uml-property:ActivityEdge-inPartition .

mms-property:representsElement a mms-ontology:UmlObjectProperty ;
	mms-ontology:cardinality "1"^^uml-model-dt:cardinalityRange ;
	mms-ontology:key "representsId" ;
	rdfs:label "representsElement" ;
	rdfs:comment "The Element that is the represents of this ActivityPartition. Based on the UML property 'ActivityPartition-represents' which is described as: An Element represented by the functionality modeled within the ActivityPartition."@en ;
	rdfs:domain uml-class:ActivityPartition ;
	rdfs:range uml-class:Element ;
	mms-ontology:umlPropertySource uml-property:ActivityPartition-represents .

mms-property:representsConnectableElement a mms-ontology:UmlObjectProperty ;
	mms-ontology:cardinality "1"^^uml-model-dt:cardinalityRange ;
	mms-ontology:key "representsId" ;
	rdfs:label "representsConnectableElement" ;
	rdfs:comment "The ConnectableElement that is the represents of this Lifeline. Based on the UML property 'Lifeline-represents' which is described as: References the ConnectableElement within the classifier that contains the enclosing interaction."@en ;
	rdfs:domain uml-class:Lifeline ;
	rdfs:range uml-class:ConnectableElement ;
	mms-ontology:umlPropertySource uml-property:Lifeline-represents .

mms-property:replyValue a mms-ontology:UmlObjectProperty ;
	mms-ontology:cardinality "*"^^uml-model-dt:cardinalityRange ;
	mms-ontology:key "replyValueIds" ;
	rdfs:label "replyValue" ;
	rdfs:comment "A InputPin that is the replyValue of this ReplyAction. Based on the UML property 'ReplyAction-replyValue' which is described as: A list of InputPins providing the values for the output (inout, out, and return) Parameters of the Operation. These values are returned to the caller."@en ;
	rdfs:domain uml-class:ReplyAction ;
	rdfs:range uml-class:InputPin ;
	mms-ontology:umlPropertySource uml-property:ReplyAction-replyValue .

mms-property:mustIsolateBoolean a mms-ontology:UmlDatatypeProperty ;
	mms-ontology:cardinality "1"^^uml-model-dt:cardinalityRange ;
	mms-ontology:key "mustIsolateId" ;
	rdfs:label "mustIsolateBoolean" ;
	rdfs:comment "The Boolean that is the mustIsolate of this StructuredActivityNode. Based on the UML property 'StructuredActivityNode-mustIsolate' which is described as: If true, then any object used by an Action within the StructuredActivityNode cannot be accessed by any Action outside the node until the StructuredActivityNode as a whole completes. Any concurrent Actions that would result in accessing such objects are required to have their execution deferred until the completion of the StructuredActivityNode.&#xD;&#xA;"@en ;
	rdfs:domain uml-class:StructuredActivityNode ;
	rdfs:range xsd:boolean ;
	mms-ontology:umlPropertySource uml-property:StructuredActivityNode-mustIsolate .

mms-property:operandInteractionOperand a mms-ontology:UmlObjectProperty ;
	mms-ontology:cardinality "*"^^uml-model-dt:cardinalityRange ;
	mms-ontology:key "operandIds" ;
	rdfs:label "operandInteractionOperand" ;
	rdfs:comment "A InteractionOperand that is the operand of this CombinedFragment. Based on the UML property 'CombinedFragment-operand' which is described as: The set of operands of the combined fragment."@en ;
	rdfs:domain uml-class:CombinedFragment ;
	rdfs:range uml-class:InteractionOperand ;
	mms-ontology:umlPropertySource uml-property:CombinedFragment-operand .

mms-property:operandValueSpecification a mms-ontology:UmlObjectProperty ;
	mms-ontology:cardinality "*"^^uml-model-dt:cardinalityRange ;
	mms-ontology:key "operandIds" ;
	rdfs:label "operandValueSpecification" ;
	rdfs:comment "A ValueSpecification that is the operand of this Expression. Based on the UML property 'Expression-operand' which is described as: Specifies a sequence of operand ValueSpecifications."@en ;
	rdfs:domain uml-class:Expression ;
	rdfs:range uml-class:ValueSpecification ;
	mms-ontology:umlPropertySource uml-property:Expression-operand .

mms-property:parameteredElementOperation a mms-ontology:UmlObjectProperty ;
	mms-ontology:cardinality "1"^^uml-model-dt:cardinalityRange ;
	mms-ontology:key "parameteredElementId" ;
	rdfs:label "parameteredElementOperation" ;
	rdfs:comment "The Operation that is the parameteredElement of this OperationTemplateParameter. Based on the UML property 'OperationTemplateParameter-parameteredElement' which is described as: The Operation exposed by this OperationTemplateParameter."@en ;
	rdfs:domain uml-class:OperationTemplateParameter ;
	rdfs:range uml-class:Operation ;
	mms-ontology:umlPropertySource uml-property:OperationTemplateParameter-parameteredElement .

mms-property:parameteredElementParameterableElement a mms-ontology:UmlObjectProperty ;
	mms-ontology:cardinality "1"^^uml-model-dt:cardinalityRange ;
	mms-ontology:key "parameteredElementId" ;
	rdfs:label "parameteredElementParameterableElement" ;
	rdfs:comment "The ParameterableElement that is the parameteredElement of this TemplateParameter. Based on the UML property 'TemplateParameter-parameteredElement' which is described as: The ParameterableElement exposed by this TemplateParameter."@en ;
	rdfs:domain uml-class:TemplateParameter ;
	rdfs:range uml-class:ParameterableElement ;
	mms-ontology:umlPropertySource uml-property:TemplateParameter-parameteredElement .

mms-property:parameteredElementClassifier a mms-ontology:UmlObjectProperty ;
	mms-ontology:cardinality "1"^^uml-model-dt:cardinalityRange ;
	mms-ontology:key "parameteredElementId" ;
	rdfs:label "parameteredElementClassifier" ;
	rdfs:comment "The Classifier that is the parameteredElement of this ClassifierTemplateParameter. Based on the UML property 'ClassifierTemplateParameter-parameteredElement' which is described as: The Classifier exposed by this ClassifierTemplateParameter."@en ;
	rdfs:domain uml-class:ClassifierTemplateParameter ;
	rdfs:range uml-class:Classifier ;
	mms-ontology:umlPropertySource uml-property:ClassifierTemplateParameter-parameteredElement .

mms-property:parameteredElementConnectableElement a mms-ontology:UmlObjectProperty ;
	mms-ontology:cardinality "1"^^uml-model-dt:cardinalityRange ;
	mms-ontology:key "parameteredElementId" ;
	rdfs:label "parameteredElementConnectableElement" ;
	rdfs:comment "The ConnectableElement that is the parameteredElement of this ConnectableElementTemplateParameter. Based on the UML property 'ConnectableElementTemplateParameter-parameteredElement' which is described as: The ConnectableElement for this ConnectableElementTemplateParameter."@en ;
	rdfs:domain uml-class:ConnectableElementTemplateParameter ;
	rdfs:range uml-class:ConnectableElement ;
	mms-ontology:umlPropertySource uml-property:ConnectableElementTemplateParameter-parameteredElement .

mms-property:providedFromPort a mms-ontology:UmlObjectProperty ;
	mms-ontology:cardinality "*"^^uml-model-dt:cardinalityRange ;
	mms-ontology:key "providedIds" ;
	rdfs:label "providedFromPort" ;
	rdfs:comment "A Interface that is the provided of this Port. Based on the UML property 'Port-provided' which is described as: The Interfaces specifying the set of Operations and Receptions that the EncapsulatedCclassifier offers to its environment via this Port, and which it will handle either directly or by forwarding it to a part of its internal structure. This association is derived according to the value of isConjugated. If isConjugated is false, provided is derived as the union of the sets of Interfaces realized by the type of the port and its supertypes, or directly from the type of the Port if the Port is typed by an Interface. If isConjugated is true, it is derived as the union of the sets of Interfaces used by the type of the Port and its supertypes."@en ;
	rdfs:domain uml-class:Port ;
	rdfs:range uml-class:Interface ;
	mms-ontology:umlPropertySource uml-property:Port-provided .

mms-property:providedFromComponent a mms-ontology:UmlObjectProperty ;
	mms-ontology:cardinality "*"^^uml-model-dt:cardinalityRange ;
	mms-ontology:key "providedIds" ;
	rdfs:label "providedFromComponent" ;
	rdfs:comment "A Interface that is the provided of this Component. Based on the UML property 'Component-provided' which is described as: The Interfaces that the Component exposes to its environment. These Interfaces may be Realized by the Component or any of its realizingClassifiers, or they may be the Interfaces that are provided by its public Ports."@en ;
	rdfs:domain uml-class:Component ;
	rdfs:range uml-class:Interface ;
	mms-ontology:umlPropertySource uml-property:Component-provided .

mms-property:lowerValueValueSpecification a mms-ontology:UmlObjectProperty ;
	mms-ontology:cardinality "1"^^uml-model-dt:cardinalityRange ;
	mms-ontology:key "lowerValueId" ;
	rdfs:label "lowerValueValueSpecification" ;
	rdfs:comment "The ValueSpecification that is the lowerValue of this MultiplicityElement. Based on the UML property 'MultiplicityElement-lowerValue' which is described as: The specification of the lower bound for this multiplicity."@en ;
	rdfs:domain uml-class:MultiplicityElement ;
	rdfs:range uml-class:ValueSpecification ;
	mms-ontology:umlPropertySource uml-property:MultiplicityElement-lowerValue .

mms-property:extendedCaseUseCase a mms-ontology:UmlObjectProperty ;
	mms-ontology:cardinality "1"^^uml-model-dt:cardinalityRange ;
	mms-ontology:key "extendedCaseId" ;
	rdfs:label "extendedCaseUseCase" ;
	rdfs:comment "The UseCase that is the extendedCase of this Extend. Based on the UML property 'Extend-extendedCase' which is described as: The UseCase that is being extended."@en ;
	rdfs:domain uml-class:Extend ;
	rdfs:range uml-class:UseCase ;
	mms-ontology:umlPropertySource uml-property:Extend-extendedCase .

mms-property:successorClause a mms-ontology:UmlObjectProperty ;
	mms-ontology:cardinality "*"^^uml-model-dt:cardinalityRange ;
	mms-ontology:key "successorClauseIds" ;
	rdfs:label "successorClause" ;
	rdfs:comment "A Clause that belongs to this Clause. Based on the UML property 'Clause-successorClause' which is described as: A set of Clauses that may not evaluate their tests unless the test for this Clause evaluates to false."@en ;
	rdfs:domain uml-class:Clause ;
	rdfs:range uml-class:Clause ;
	mms-ontology:umlPropertySource uml-property:Clause-successorClause .

mms-property:packagedElementFromComponent a mms-ontology:UmlObjectProperty ;
	mms-ontology:cardinality "*"^^uml-model-dt:cardinalityRange ;
	mms-ontology:key "packagedElementIds" ;
	rdfs:label "packagedElementFromComponent" ;
	rdfs:comment "A PackageableElement that is the packagedElement of this Component. Based on the UML property 'Component-packagedElement' which is described as: The set of PackageableElements that a Component owns. In the namespace of a Component, all model elements that are involved in or related to its definition may be owned or imported explicitly. These may include e.g., Classes, Interfaces, Components, Packages, UseCases, Dependencies (e.g., mappings), and Artifacts."@en ;
	rdfs:domain uml-class:Component ;
	rdfs:range uml-class:PackageableElement ;
	mms-ontology:umlPropertySource uml-property:Component-packagedElement .

mms-property:packagedElementFromPackage a mms-ontology:UmlObjectProperty ;
	mms-ontology:cardinality "*"^^uml-model-dt:cardinalityRange ;
	mms-ontology:key "packagedElementIds" ;
	rdfs:label "packagedElementFromPackage" ;
	rdfs:comment "A PackageableElement that is the packagedElement of this Package. Based on the UML property 'Package-packagedElement' which is described as: Specifies the packageable elements that are owned by this Package."@en ;
	rdfs:domain uml-class:Package ;
	rdfs:range uml-class:PackageableElement ;
	mms-ontology:umlPropertySource uml-property:Package-packagedElement .

mms-property:ownedConnector a mms-ontology:UmlObjectProperty ;
	mms-ontology:cardinality "*"^^uml-model-dt:cardinalityRange ;
	mms-ontology:key "ownedConnectorIds" ;
	rdfs:label "ownedConnector" ;
	rdfs:comment "A Connector that belongs to this StructuredClassifier. Based on the UML property 'StructuredClassifier-ownedConnector' which is described as: The connectors owned by the StructuredClassifier."@en ;
	rdfs:domain uml-class:StructuredClassifier ;
	rdfs:range uml-class:Connector ;
	mms-ontology:umlPropertySource uml-property:StructuredClassifier-ownedConnector .

mms-property:requestInputPin a mms-ontology:UmlObjectProperty ;
	mms-ontology:cardinality "1"^^uml-model-dt:cardinalityRange ;
	mms-ontology:key "requestId" ;
	rdfs:label "requestInputPin" ;
	rdfs:comment "The InputPin that is the request of this SendObjectAction. Based on the UML property 'SendObjectAction-request' which is described as: The request object, which is transmitted to the target object. The object may be copied in transmission, so identity might not be preserved."@en ;
	rdfs:domain uml-class:SendObjectAction ;
	rdfs:range uml-class:InputPin ;
	mms-ontology:umlPropertySource uml-property:SendObjectAction-request .

mms-property:setupPart a mms-ontology:UmlObjectProperty ;
	mms-ontology:cardinality "*"^^uml-model-dt:cardinalityRange ;
	mms-ontology:key "setupPartIds" ;
	rdfs:label "setupPart" ;
	rdfs:comment "A ExecutableNode that is the setupPart of this LoopNode. Based on the UML property 'LoopNode-setupPart' which is described as: The set of ExecutableNodes executed before the first iteration of the loop, in order to initialize values or perform other setup computations."@en ;
	rdfs:domain uml-class:LoopNode ;
	rdfs:range uml-class:ExecutableNode ;
	mms-ontology:umlPropertySource uml-property:LoopNode-setupPart .

mms-property:realizingMessage a mms-ontology:UmlObjectProperty ;
	mms-ontology:cardinality "*"^^uml-model-dt:cardinalityRange ;
	mms-ontology:key "realizingMessageIds" ;
	rdfs:label "realizingMessage" ;
	rdfs:comment "A Message that belongs to this InformationFlow. Based on the UML property 'InformationFlow-realizingMessage' which is described as: Determines which Messages will realize the specified flow."@en ;
	rdfs:domain uml-class:InformationFlow ;
	rdfs:range uml-class:Message ;
	mms-ontology:umlPropertySource uml-property:InformationFlow-realizingMessage .

mms-property:include a mms-ontology:UmlObjectProperty ;
	mms-ontology:cardinality "*"^^uml-model-dt:cardinalityRange ;
	mms-ontology:key "includeIds" ;
	rdfs:label "include" ;
	rdfs:comment "A Include that belongs to this UseCase. Based on the UML property 'UseCase-include' which is described as: The Include relationships owned by this UseCase."@en ;
	rdfs:domain uml-class:UseCase ;
	rdfs:range uml-class:Include ;
	mms-ontology:umlPropertySource uml-property:UseCase-include .

mms-property:owningTemplateParameter a mms-ontology:UmlObjectProperty ;
	mms-ontology:cardinality "1"^^uml-model-dt:cardinalityRange ;
	mms-ontology:key "owningTemplateParameterId" ;
	rdfs:label "owningTemplateParameter" ;
	rdfs:comment "The TemplateParameter that belongs to this ParameterableElement. Based on the UML property 'ParameterableElement-owningTemplateParameter' which is described as: The formal TemplateParameter that owns this ParameterableElement."@en ;
	rdfs:domain uml-class:ParameterableElement ;
	rdfs:range uml-class:TemplateParameter ;
	mms-ontology:umlPropertySource uml-property:ParameterableElement-owningTemplateParameter .

mms-property:ownedTemplateSignatureRedefinableTemplateSignature a mms-ontology:UmlObjectProperty ;
	mms-ontology:cardinality "1"^^uml-model-dt:cardinalityRange ;
	mms-ontology:key "ownedTemplateSignatureId" ;
	rdfs:label "ownedTemplateSignatureRedefinableTemplateSignature" ;
	rdfs:comment "The RedefinableTemplateSignature that is the ownedTemplateSignature of this Classifier. Based on the UML property 'Classifier-ownedTemplateSignature' which is described as: The optional RedefinableTemplateSignature specifying the formal template parameters."@en ;
	rdfs:domain uml-class:Classifier ;
	rdfs:range uml-class:RedefinableTemplateSignature ;
	mms-ontology:umlPropertySource uml-property:Classifier-ownedTemplateSignature .

mms-property:ownedTemplateSignature a mms-ontology:UmlObjectProperty ;
	mms-ontology:cardinality "1"^^uml-model-dt:cardinalityRange ;
	mms-ontology:key "ownedTemplateSignatureId" ;
	rdfs:label "ownedTemplateSignature" ;
	rdfs:comment "The TemplateSignature that belongs to this TemplateableElement. Based on the UML property 'TemplateableElement-ownedTemplateSignature' which is described as: The optional TemplateSignature specifying the formal TemplateParameters for this TemplateableElement. If a TemplateableElement has a TemplateSignature, then it is a template."@en ;
	rdfs:domain uml-class:TemplateableElement ;
	rdfs:range uml-class:TemplateSignature ;
	mms-ontology:umlPropertySource uml-property:TemplateableElement-ownedTemplateSignature .

mms-property:structuredNodeOutput a mms-ontology:UmlObjectProperty ;
	mms-ontology:cardinality "*"^^uml-model-dt:cardinalityRange ;
	mms-ontology:key "structuredNodeOutputIds" ;
	rdfs:label "structuredNodeOutput" ;
	rdfs:comment "A OutputPin that is the structuredNodeOutput of this StructuredActivityNode. Based on the UML property 'StructuredActivityNode-structuredNodeOutput' which is described as: The OutputPins owned by the StructuredActivityNode."@en ;
	rdfs:domain uml-class:StructuredActivityNode ;
	rdfs:range uml-class:OutputPin ;
	mms-ontology:umlPropertySource uml-property:StructuredActivityNode-structuredNodeOutput .

mms-property:subvertex a mms-ontology:UmlObjectProperty ;
	mms-ontology:cardinality "*"^^uml-model-dt:cardinalityRange ;
	mms-ontology:key "subvertexIds" ;
	rdfs:label "subvertex" ;
	rdfs:comment "A Vertex that is the subvertex of this Region. Based on the UML property 'Region-subvertex' which is described as: The set of Vertices that are owned by this Region."@en ;
	rdfs:domain uml-class:Region ;
	rdfs:range uml-class:Vertex ;
	mms-ontology:umlPropertySource uml-property:Region-subvertex .

mms-property:event a mms-ontology:UmlObjectProperty ;
	mms-ontology:cardinality "1"^^uml-model-dt:cardinalityRange ;
	mms-ontology:key "eventId" ;
	rdfs:label "event" ;
	rdfs:comment "The Event that belongs to this Trigger. Based on the UML property 'Trigger-event' which is described as: The Event that detected by the Trigger."@en ;
	rdfs:domain uml-class:Trigger ;
	rdfs:range uml-class:Event ;
	mms-ontology:umlPropertySource uml-property:Trigger-event .

mms-property:eventNamedElementsFromDurationObservation a mms-ontology:UmlObjectProperty ;
	mms-ontology:cardinality "2"^^uml-model-dt:cardinalityRange ;
	mms-ontology:key "eventIds" ;
	rdfs:label "eventNamedElementsFromDurationObservation" ;
	rdfs:comment "List of NamedElements that are the event of this DurationObservation. Based on the UML property 'DurationObservation-event' which is described as: The DurationObservation is determined as the duration between the entering or exiting of a single event Element during execution, or the entering/exiting of one event Element and the entering/exiting of a second."@en ;
	rdfs:domain uml-class:DurationObservation ;
	rdfs:range mms-class:EventNamedElementsFromDurationObservationList ;
	mms-ontology:listItemRange uml-class:NamedElement ;
	mms-ontology:umlPropertySource uml-property:DurationObservation-event .

mms-class:EventNamedElementsFromDurationObservationList a owl:Class ;
	mms-ontology:category mms-class:ElementList ;
	rdfs:subClassOf [
		rdf:type owl:Class ;
		owl:intersectionOf (
			rdf:List
			[
				rdf:type owl:Restriction ;
				owl:onProperty rdf:first ;
				owl:allValuesFrom uml-class:NamedElement ;
			]
			[
				rdf:type owl:Restriction ;
				owl:onProperty rdf:rest ;
				owl:allValuesFrom mms-class:EventNamedElementsFromDurationObservationList ;
			]
		) ;
	] .

mms-property:eventNamedElementFromTimeObservation a mms-ontology:UmlObjectProperty ;
	mms-ontology:cardinality "1"^^uml-model-dt:cardinalityRange ;
	mms-ontology:key "eventId" ;
	rdfs:label "eventNamedElementFromTimeObservation" ;
	rdfs:comment "The NamedElement that is the event of this TimeObservation. Based on the UML property 'TimeObservation-event' which is described as: The TimeObservation is determined by the entering or exiting of the event Element during execution."@en ;
	rdfs:domain uml-class:TimeObservation ;
	rdfs:range uml-class:NamedElement ;
	mms-ontology:umlPropertySource uml-property:TimeObservation-event .

mms-property:deciderOutputPinFromLoopNode a mms-ontology:UmlObjectProperty ;
	mms-ontology:cardinality "1"^^uml-model-dt:cardinalityRange ;
	mms-ontology:key "deciderId" ;
	rdfs:label "deciderOutputPinFromLoopNode" ;
	rdfs:comment "The OutputPin that is the decider of this LoopNode. Based on the UML property 'LoopNode-decider' which is described as: An OutputPin on an Action in the test section whose Boolean value determines whether to continue executing the loop bodyPart."@en ;
	rdfs:domain uml-class:LoopNode ;
	rdfs:range uml-class:OutputPin ;
	mms-ontology:umlPropertySource uml-property:LoopNode-decider .

mms-property:deciderOutputPinFromClause a mms-ontology:UmlObjectProperty ;
	mms-ontology:cardinality "1"^^uml-model-dt:cardinalityRange ;
	mms-ontology:key "deciderId" ;
	rdfs:label "deciderOutputPinFromClause" ;
	rdfs:comment "The OutputPin that is the decider of this Clause. Based on the UML property 'Clause-decider' which is described as: An OutputPin on an Action in the test section whose Boolean value determines the result of the test."@en ;
	rdfs:domain uml-class:Clause ;
	rdfs:range uml-class:OutputPin ;
	mms-ontology:umlPropertySource uml-property:Clause-decider .

mms-property:messageFromInteraction a mms-ontology:UmlObjectProperty ;
	mms-ontology:cardinality "*"^^uml-model-dt:cardinalityRange ;
	mms-ontology:key "messageIds" ;
	rdfs:label "messageFromInteraction" ;
	rdfs:comment "A Message that belongs to this Interaction. Based on the UML property 'Interaction-message' which is described as: The Messages contained in this Interaction."@en ;
	rdfs:domain uml-class:Interaction ;
	rdfs:range uml-class:Message ;
	mms-ontology:umlPropertySource uml-property:Interaction-message .

mms-property:messageFromMessageEnd a mms-ontology:UmlObjectProperty ;
	mms-ontology:cardinality "1"^^uml-model-dt:cardinalityRange ;
	mms-ontology:key "messageId" ;
	rdfs:label "messageFromMessageEnd" ;
	rdfs:comment "The Message that belongs to this MessageEnd. Based on the UML property 'MessageEnd-message' which is described as: References a Message."@en ;
	rdfs:domain uml-class:MessageEnd ;
	rdfs:range uml-class:Message ;
	mms-ontology:umlPropertySource uml-property:MessageEnd-message .

mms-property:messageNamedElement a mms-ontology:UmlObjectProperty ;
	mms-ontology:cardinality "*"^^uml-model-dt:cardinalityRange ;
	mms-ontology:key "messageIds" ;
	rdfs:label "messageNamedElement" ;
	rdfs:comment "A NamedElement that is the message of this ConsiderIgnoreFragment. Based on the UML property 'ConsiderIgnoreFragment-message' which is described as: The set of messages that apply to this fragment."@en ;
	rdfs:domain uml-class:ConsiderIgnoreFragment ;
	rdfs:range uml-class:NamedElement ;
	mms-ontology:umlPropertySource uml-property:ConsiderIgnoreFragment-message .

mms-property:partWithPortProperty a mms-ontology:UmlObjectProperty ;
	mms-ontology:cardinality "1"^^uml-model-dt:cardinalityRange ;
	mms-ontology:key "partWithPortId" ;
	rdfs:label "partWithPortProperty" ;
	rdfs:comment "The Property that is the partWithPort of this ConnectorEnd. Based on the UML property 'ConnectorEnd-partWithPort' which is described as: Indicates the role of the internal structure of a Classifier with the Port to which the ConnectorEnd is attached."@en ;
	rdfs:domain uml-class:ConnectorEnd ;
	rdfs:range uml-class:Property ;
	mms-ontology:umlPropertySource uml-property:ConnectorEnd-partWithPort .

mms-property:ownedReceptionFromClass a mms-ontology:UmlObjectProperty ;
	mms-ontology:cardinality "*"^^uml-model-dt:cardinalityRange ;
	mms-ontology:key "ownedReceptionIds" ;
	rdfs:label "ownedReceptionFromClass" ;
	rdfs:comment "A Reception that belongs to this Class. Based on the UML property 'Class-ownedReception' which is described as: The Receptions owned by the Class."@en ;
	rdfs:domain uml-class:Class ;
	rdfs:range uml-class:Reception ;
	mms-ontology:umlPropertySource uml-property:Class-ownedReception .

mms-property:ownedReceptionFromInterface a mms-ontology:UmlObjectProperty ;
	mms-ontology:cardinality "*"^^uml-model-dt:cardinalityRange ;
	mms-ontology:key "ownedReceptionIds" ;
	rdfs:label "ownedReceptionFromInterface" ;
	rdfs:comment "A Reception that belongs to this Interface. Based on the UML property 'Interface-ownedReception' which is described as: Receptions that objects providing this Interface are willing to accept."@en ;
	rdfs:domain uml-class:Interface ;
	rdfs:range uml-class:Reception ;
	mms-ontology:umlPropertySource uml-property:Interface-ownedReception .

mms-property:representationCollaborationUse a mms-ontology:UmlObjectProperty ;
	mms-ontology:cardinality "1"^^uml-model-dt:cardinalityRange ;
	mms-ontology:key "representationId" ;
	rdfs:label "representationCollaborationUse" ;
	rdfs:comment "The CollaborationUse that is the representation of this Classifier. Based on the UML property 'Classifier-representation' which is described as: A CollaborationUse which indicates the Collaboration that represents this Classifier."@en ;
	rdfs:domain uml-class:Classifier ;
	rdfs:range uml-class:CollaborationUse ;
	mms-ontology:umlPropertySource uml-property:Classifier-representation .

mms-property:conveyed a mms-ontology:UmlObjectProperty ;
	mms-ontology:cardinality "*"^^uml-model-dt:cardinalityRange ;
	mms-ontology:key "conveyedIds" ;
	rdfs:label "conveyed" ;
	rdfs:comment "A Classifier that is the conveyed of this InformationFlow. Based on the UML property 'InformationFlow-conveyed' which is described as: Specifies the information items that may circulate on this information flow."@en ;
	rdfs:domain uml-class:InformationFlow ;
	rdfs:range uml-class:Classifier ;
	mms-ontology:umlPropertySource uml-property:InformationFlow-conveyed .

mms-property:owningAssociation a mms-ontology:UmlObjectProperty ;
	mms-ontology:cardinality "1"^^uml-model-dt:cardinalityRange ;
	mms-ontology:key "owningAssociationId" ;
	rdfs:label "owningAssociation" ;
	rdfs:comment "The Association that belongs to this Property. Based on the UML property 'Property-owningAssociation' which is described as: The owning association of this property, if any."@en ;
	rdfs:domain uml-class:Property ;
	rdfs:range uml-class:Association ;
	mms-ontology:umlPropertySource uml-property:Property-owningAssociation .

mms-property:refersToInteraction a mms-ontology:UmlObjectProperty ;
	mms-ontology:cardinality "1"^^uml-model-dt:cardinalityRange ;
	mms-ontology:key "refersToId" ;
	rdfs:label "refersToInteraction" ;
	rdfs:comment "The Interaction that is the refersTo of this InteractionUse. Based on the UML property 'InteractionUse-refersTo' which is described as: Refers to the Interaction that defines its meaning."@en ;
	rdfs:domain uml-class:InteractionUse ;
	rdfs:range uml-class:Interaction ;
	mms-ontology:umlPropertySource uml-property:InteractionUse-refersTo .

mms-property:triggerFromTransition a mms-ontology:UmlObjectProperty ;
	mms-ontology:cardinality "*"^^uml-model-dt:cardinalityRange ;
	mms-ontology:key "triggerIds" ;
	rdfs:label "triggerFromTransition" ;
	rdfs:comment "A Trigger that belongs to this Transition. Based on the UML property 'Transition-trigger' which is described as: Specifies the Triggers that may fire the transition."@en ;
	rdfs:domain uml-class:Transition ;
	rdfs:range uml-class:Trigger ;
	mms-ontology:umlPropertySource uml-property:Transition-trigger .

mms-property:triggerFromAcceptEventAction a mms-ontology:UmlObjectProperty ;
	mms-ontology:cardinality "*"^^uml-model-dt:cardinalityRange ;
	mms-ontology:key "triggerIds" ;
	rdfs:label "triggerFromAcceptEventAction" ;
	rdfs:comment "A Trigger that belongs to this AcceptEventAction. Based on the UML property 'AcceptEventAction-trigger' which is described as: The Triggers specifying the Events of which the AcceptEventAction waits for occurrences."@en ;
	rdfs:domain uml-class:AcceptEventAction ;
	rdfs:range uml-class:Trigger ;
	mms-ontology:umlPropertySource uml-property:AcceptEventAction-trigger .

mms-property:isLeaf a mms-ontology:UmlDatatypeProperty ;
	mms-ontology:key "isLeaf" ;
	rdfs:label "isLeaf" ;
	rdfs:comment "Indicates whether it is possible to further redefine a RedefinableElement. If the value is true, then it is not possible to further redefine the RedefinableElement."@en ;
	rdfs:domain uml-class:RedefinableElement ;
	rdfs:range xsd:boolean ;
	mms-ontology:umlPropertySource uml-property:RedefinableElement-isLeaf .

mms-property:isLeafRedefinableElement a mms-ontology:UmlDatatypeProperty ;
	owl:equivalentProperty mms-property:isLeaf .

mms-property:redefinedOperation a mms-ontology:UmlObjectProperty ;
	mms-ontology:cardinality "*"^^uml-model-dt:cardinalityRange ;
	mms-ontology:key "redefinedOperationIds" ;
	rdfs:label "redefinedOperation" ;
	rdfs:comment "A Operation that belongs to this Operation. Based on the UML property 'Operation-redefinedOperation' which is described as: The Operations that are redefined by this Operation."@en ;
	rdfs:domain uml-class:Operation ;
	rdfs:range uml-class:Operation ;
	mms-ontology:umlPropertySource uml-property:Operation-redefinedOperation .

mms-property:isReplaceAllAddVariableValueAction a mms-ontology:UmlDatatypeProperty ;
	mms-ontology:key "isReplaceAll" ;
	rdfs:label "isReplaceAllAddVariableValueAction" ;
	rdfs:comment "Specifies whether existing values of the Variable should be removed before adding the new value."@en ;
	rdfs:domain uml-class:AddVariableValueAction ;
	rdfs:range xsd:boolean ;
	mms-ontology:umlPropertySource uml-property:AddVariableValueAction-isReplaceAll .

mms-property:isReplaceAllReclassifyObjectAction a mms-ontology:UmlDatatypeProperty ;
	mms-ontology:key "isReplaceAll" ;
	rdfs:label "isReplaceAllReclassifyObjectAction" ;
	rdfs:comment "Specifies whether existing Classifiers should be removed before adding the new Classifiers."@en ;
	rdfs:domain uml-class:ReclassifyObjectAction ;
	rdfs:range xsd:boolean ;
	mms-ontology:umlPropertySource uml-property:ReclassifyObjectAction-isReplaceAll .

mms-property:isReplaceAllAddStructuralFeatureValueAction a mms-ontology:UmlDatatypeProperty ;
	mms-ontology:key "isReplaceAll" ;
	rdfs:label "isReplaceAllAddStructuralFeatureValueAction" ;
	rdfs:comment "Specifies whether existing values of the StructuralFeature should be removed before adding the new value."@en ;
	rdfs:domain uml-class:AddStructuralFeatureValueAction ;
	rdfs:range xsd:boolean ;
	mms-ontology:umlPropertySource uml-property:AddStructuralFeatureValueAction-isReplaceAll .

mms-property:isReplaceAllLinkEndCreationData a mms-ontology:UmlDatatypeProperty ;
	mms-ontology:key "isReplaceAll" ;
	rdfs:label "isReplaceAllLinkEndCreationData" ;
	rdfs:comment "Specifies whether the existing links emanating from the object on this end should be destroyed before creating a new link."@en ;
	rdfs:domain uml-class:LinkEndCreationData ;
	rdfs:range xsd:boolean ;
	mms-ontology:umlPropertySource uml-property:LinkEndCreationData-isReplaceAll .

mms-property:deploymentFromDeploymentTarget a mms-ontology:UmlObjectProperty ;
	mms-ontology:cardinality "*"^^uml-model-dt:cardinalityRange ;
	mms-ontology:key "deploymentIds" ;
	rdfs:label "deploymentFromDeploymentTarget" ;
	rdfs:comment "A Deployment that belongs to this DeploymentTarget. Based on the UML property 'DeploymentTarget-deployment' which is described as: The set of Deployments for a DeploymentTarget."@en ;
	rdfs:domain uml-class:DeploymentTarget ;
	rdfs:range uml-class:Deployment ;
	mms-ontology:umlPropertySource uml-property:DeploymentTarget-deployment .

mms-property:deploymentFromDeploymentSpecification a mms-ontology:UmlObjectProperty ;
	mms-ontology:cardinality "1"^^uml-model-dt:cardinalityRange ;
	mms-ontology:key "deploymentId" ;
	rdfs:label "deploymentFromDeploymentSpecification" ;
	rdfs:comment "The Deployment that belongs to this DeploymentSpecification. Based on the UML property 'DeploymentSpecification-deployment' which is described as: The deployment with which the DeploymentSpecification is associated."@en ;
	rdfs:domain uml-class:DeploymentSpecification ;
	rdfs:range uml-class:Deployment ;
	mms-ontology:umlPropertySource uml-property:DeploymentSpecification-deployment .

mms-property:targetInputPinFromSendObjectAction a mms-ontology:UmlObjectProperty ;
	mms-ontology:cardinality "1"^^uml-model-dt:cardinalityRange ;
	mms-ontology:key "targetId" ;
	rdfs:label "targetInputPinFromSendObjectAction" ;
	rdfs:comment "The InputPin that is the target of this SendObjectAction. Based on the UML property 'SendObjectAction-target' which is described as: The target object to which the object is sent."@en ;
	rdfs:domain uml-class:SendObjectAction ;
	rdfs:range uml-class:InputPin ;
	mms-ontology:umlPropertySource uml-property:SendObjectAction-target .

mms-property:targetInputPinFromCallOperationAction a mms-ontology:UmlObjectProperty ;
	mms-ontology:cardinality "1"^^uml-model-dt:cardinalityRange ;
	mms-ontology:key "targetId" ;
	rdfs:label "targetInputPinFromCallOperationAction" ;
	rdfs:comment "The InputPin that is the target of this CallOperationAction. Based on the UML property 'CallOperationAction-target' which is described as: The InputPin that provides the target object to which the Operation call request is sent."@en ;
	rdfs:domain uml-class:CallOperationAction ;
	rdfs:range uml-class:InputPin ;
	mms-ontology:umlPropertySource uml-property:CallOperationAction-target .

mms-property:targetInputPinFromDestroyObjectAction a mms-ontology:UmlObjectProperty ;
	mms-ontology:cardinality "1"^^uml-model-dt:cardinalityRange ;
	mms-ontology:key "targetId" ;
	rdfs:label "targetInputPinFromDestroyObjectAction" ;
	rdfs:comment "The InputPin that is the target of this DestroyObjectAction. Based on the UML property 'DestroyObjectAction-target' which is described as: The InputPin providing the object to be destroyed."@en ;
	rdfs:domain uml-class:DestroyObjectAction ;
	rdfs:range uml-class:InputPin ;
	mms-ontology:umlPropertySource uml-property:DestroyObjectAction-target .

mms-property:targetInputPinFromSendSignalAction a mms-ontology:UmlObjectProperty ;
	mms-ontology:cardinality "1"^^uml-model-dt:cardinalityRange ;
	mms-ontology:key "targetId" ;
	rdfs:label "targetInputPinFromSendSignalAction" ;
	rdfs:comment "The InputPin that is the target of this SendSignalAction. Based on the UML property 'SendSignalAction-target' which is described as: The InputPin that provides the target object to which the Signal instance is sent."@en ;
	rdfs:domain uml-class:SendSignalAction ;
	rdfs:range uml-class:InputPin ;
	mms-ontology:umlPropertySource uml-property:SendSignalAction-target .

mms-property:targetVertex a mms-ontology:UmlObjectProperty ;
	mms-ontology:cardinality "1"^^uml-model-dt:cardinalityRange ;
	mms-ontology:key "targetId" ;
	rdfs:label "targetVertex" ;
	rdfs:comment "The Vertex that is the target of this Transition. Based on the UML property 'Transition-target' which is described as: Designates the target Vertex that is reached when the Transition is taken."@en ;
	rdfs:domain uml-class:Transition ;
	rdfs:range uml-class:Vertex ;
	mms-ontology:umlPropertySource uml-property:Transition-target .

mms-property:targetElement a mms-ontology:UmlObjectProperty ;
	mms-ontology:cardinality "*"^^uml-model-dt:cardinalityRange ;
	mms-ontology:key "targetIds" ;
	rdfs:label "targetElement" ;
	rdfs:comment "A Element that is the target of this DirectedRelationship. Based on the UML property 'DirectedRelationship-target' which is described as: Specifies the target Element(s) of the DirectedRelationship."@en ;
	rdfs:domain uml-class:DirectedRelationship ;
	rdfs:range uml-class:Element ;
	mms-ontology:umlPropertySource uml-property:DirectedRelationship-target .

mms-property:targetActivityNode a mms-ontology:UmlObjectProperty ;
	mms-ontology:cardinality "1"^^uml-model-dt:cardinalityRange ;
	mms-ontology:key "targetId" ;
	rdfs:label "targetActivityNode" ;
	rdfs:comment "The ActivityNode that is the target of this ActivityEdge. Based on the UML property 'ActivityEdge-target' which is described as: The ActivityNode to which tokens are put when they traverse the ActivityEdge."@en ;
	rdfs:domain uml-class:ActivityEdge ;
	rdfs:range uml-class:ActivityNode ;
	mms-ontology:umlPropertySource uml-property:ActivityEdge-target .

mms-property:raisedExceptionFromOperation a mms-ontology:UmlObjectProperty ;
	mms-ontology:cardinality "*"^^uml-model-dt:cardinalityRange ;
	mms-ontology:key "raisedExceptionIds" ;
	rdfs:label "raisedExceptionFromOperation" ;
	rdfs:comment "A Type that is the raisedException of this Operation. Based on the UML property 'Operation-raisedException' which is described as: The Types representing exceptions that may be raised during an invocation of this operation."@en ;
	rdfs:domain uml-class:Operation ;
	rdfs:range uml-class:Type ;
	mms-ontology:umlPropertySource uml-property:Operation-raisedException .

mms-property:raisedExceptionFromBehavioralFeature a mms-ontology:UmlObjectProperty ;
	mms-ontology:cardinality "*"^^uml-model-dt:cardinalityRange ;
	mms-ontology:key "raisedExceptionIds" ;
	rdfs:label "raisedExceptionFromBehavioralFeature" ;
	rdfs:comment "A Type that is the raisedException of this BehavioralFeature. Based on the UML property 'BehavioralFeature-raisedException' which is described as: The Types representing exceptions that may be raised during an invocation of this BehavioralFeature."@en ;
	rdfs:domain uml-class:BehavioralFeature ;
	rdfs:range uml-class:Type ;
	mms-ontology:umlPropertySource uml-property:BehavioralFeature-raisedException .

mms-property:defaultValueValueSpecificationFromParameter a mms-ontology:UmlObjectProperty ;
	mms-ontology:cardinality "1"^^uml-model-dt:cardinalityRange ;
	mms-ontology:key "defaultValueId" ;
	rdfs:label "defaultValueValueSpecificationFromParameter" ;
	rdfs:comment "The ValueSpecification that is the defaultValue of this Parameter. Based on the UML property 'Parameter-defaultValue' which is described as: Specifies a ValueSpecification that represents a value to be used when no argument is supplied for the Parameter."@en ;
	rdfs:domain uml-class:Parameter ;
	rdfs:range uml-class:ValueSpecification ;
	mms-ontology:umlPropertySource uml-property:Parameter-defaultValue .

mms-property:defaultValueValueSpecificationFromProperty a mms-ontology:UmlObjectProperty ;
	mms-ontology:cardinality "1"^^uml-model-dt:cardinalityRange ;
	mms-ontology:key "defaultValueId" ;
	rdfs:label "defaultValueValueSpecificationFromProperty" ;
	rdfs:comment "The ValueSpecification that is the defaultValue of this Property. Based on the UML property 'Property-defaultValue' which is described as: A ValueSpecification that is evaluated to give a default value for the Property when an instance of the owning Classifier is instantiated."@en ;
	rdfs:domain uml-class:Property ;
	rdfs:range uml-class:ValueSpecification ;
	mms-ontology:umlPropertySource uml-property:Property-defaultValue .

mms-property:redefinedInterface a mms-ontology:UmlObjectProperty ;
	mms-ontology:cardinality "*"^^uml-model-dt:cardinalityRange ;
	mms-ontology:key "redefinedInterfaceIds" ;
	rdfs:label "redefinedInterface" ;
	rdfs:comment "A Interface that belongs to this Interface. Based on the UML property 'Interface-redefinedInterface' which is described as: References all the Interfaces redefined by this Interface."@en ;
	rdfs:domain uml-class:Interface ;
	rdfs:range uml-class:Interface ;
	mms-ontology:umlPropertySource uml-property:Interface-redefinedInterface .

mms-property:isCompositeState a mms-ontology:UmlDatatypeProperty ;
	mms-ontology:key "isComposite" ;
	rdfs:label "isCompositeState" ;
	rdfs:comment "A state with isComposite=true is said to be a composite State. A composite State is a State that contains at least one Region."@en ;
	rdfs:domain uml-class:State ;
	rdfs:range xsd:boolean ;
	mms-ontology:umlPropertySource uml-property:State-isComposite .

mms-property:isCompositeProperty a mms-ontology:UmlDatatypeProperty ;
	mms-ontology:key "isComposite" ;
	rdfs:label "isCompositeProperty" ;
	rdfs:comment "If isComposite is true, the object containing the attribute is a container for the object or value contained in the attribute. This is a derived value, indicating whether the aggregation of the Property is composite or not."@en ;
	rdfs:domain uml-class:Property ;
	rdfs:range xsd:boolean ;
	mms-ontology:umlPropertySource uml-property:Property-isComposite .

mms-property:group a mms-ontology:UmlObjectProperty ;
	mms-ontology:cardinality "*"^^uml-model-dt:cardinalityRange ;
	mms-ontology:key "groupIds" ;
	rdfs:label "group" ;
	rdfs:comment "A ActivityGroup that is the group of this Activity. Based on the UML property 'Activity-group' which is described as: Top-level ActivityGroups in the Activity."@en ;
	rdfs:domain uml-class:Activity ;
	rdfs:range uml-class:ActivityGroup ;
	mms-ontology:umlPropertySource uml-property:Activity-group .

mms-property:enclosingOperandInteractionOperand a mms-ontology:UmlObjectProperty ;
	mms-ontology:cardinality "1"^^uml-model-dt:cardinalityRange ;
	mms-ontology:key "enclosingOperandId" ;
	rdfs:label "enclosingOperandInteractionOperand" ;
	rdfs:comment "The InteractionOperand that is the enclosingOperand of this InteractionFragment. Based on the UML property 'InteractionFragment-enclosingOperand' which is described as: The operand enclosing this InteractionFragment (they may nest recursively)."@en ;
	rdfs:domain uml-class:InteractionFragment ;
	rdfs:range uml-class:InteractionOperand ;
	mms-ontology:umlPropertySource uml-property:InteractionFragment-enclosingOperand .

mms-property:postConditionConstraint a mms-ontology:UmlObjectProperty ;
	mms-ontology:cardinality "1"^^uml-model-dt:cardinalityRange ;
	mms-ontology:key "postConditionId" ;
	rdfs:label "postConditionConstraint" ;
	rdfs:comment "The Constraint that is the postCondition of this ProtocolTransition. Based on the UML property 'ProtocolTransition-postCondition' which is described as: Specifies the post condition of the Transition which is the Condition that should be obtained once the Transition is triggered. This post condition is part of the post condition of the Operation connected to the Transition."@en ;
	rdfs:domain uml-class:ProtocolTransition ;
	rdfs:range uml-class:Constraint ;
	mms-ontology:umlPropertySource uml-property:ProtocolTransition-postCondition .

mms-property:generalizationSet a mms-ontology:UmlObjectProperty ;
	mms-ontology:cardinality "*"^^uml-model-dt:cardinalityRange ;
	mms-ontology:key "generalizationSetIds" ;
	rdfs:label "generalizationSet" ;
	rdfs:comment "A GeneralizationSet that belongs to this Generalization. Based on the UML property 'Generalization-generalizationSet' which is described as: Represents a set of instances of Generalization.  A Generalization may appear in many GeneralizationSets."@en ;
	rdfs:domain uml-class:Generalization ;
	rdfs:range uml-class:GeneralizationSet ;
	mms-ontology:umlPropertySource uml-property:Generalization-generalizationSet .

mms-property:fragmentFromInteractionOperand a mms-ontology:UmlObjectProperty ;
	mms-ontology:cardinality "*"^^uml-model-dt:cardinalityRange ;
	mms-ontology:key "fragmentIds" ;
	rdfs:label "fragmentFromInteractionOperand" ;
	rdfs:comment "A InteractionFragment that is the fragment of this InteractionOperand. Based on the UML property 'InteractionOperand-fragment' which is described as: The fragments of the operand."@en ;
	rdfs:domain uml-class:InteractionOperand ;
	rdfs:range uml-class:InteractionFragment ;
	mms-ontology:umlPropertySource uml-property:InteractionOperand-fragment .

mms-property:fragmentFromInteraction a mms-ontology:UmlObjectProperty ;
	mms-ontology:cardinality "*"^^uml-model-dt:cardinalityRange ;
	mms-ontology:key "fragmentIds" ;
	rdfs:label "fragmentFromInteraction" ;
	rdfs:comment "A InteractionFragment that is the fragment of this Interaction. Based on the UML property 'Interaction-fragment' which is described as: The ordered set of fragments in the Interaction."@en ;
	rdfs:domain uml-class:Interaction ;
	rdfs:range uml-class:InteractionFragment ;
	mms-ontology:umlPropertySource uml-property:Interaction-fragment .

mms-property:isAbstractBehavioralFeature a mms-ontology:UmlDatatypeProperty ;
	mms-ontology:key "isAbstract" ;
	rdfs:label "isAbstractBehavioralFeature" ;
	rdfs:comment "If true, then the BehavioralFeature does not have an implementation, and one must be supplied by a more specific Classifier. If false, the BehavioralFeature must have an implementation in the Classifier or one must be inherited."@en ;
	rdfs:domain uml-class:BehavioralFeature ;
	rdfs:range xsd:boolean ;
	mms-ontology:umlPropertySource uml-property:BehavioralFeature-isAbstract .

mms-property:isAbstractClass a mms-ontology:UmlDatatypeProperty ;
	mms-ontology:key "isAbstract" ;
	rdfs:label "isAbstractClass" ;
	rdfs:comment "If true, the Class does not provide a complete declaration and cannot be instantiated. An abstract Class is typically used as a target of Associations or Generalizations."@en ;
	rdfs:domain uml-class:Class ;
	rdfs:range xsd:boolean ;
	mms-ontology:umlPropertySource uml-property:Class-isAbstract .

mms-property:isAbstractClassifier a mms-ontology:UmlDatatypeProperty ;
	mms-ontology:key "isAbstract" ;
	rdfs:label "isAbstractClassifier" ;
	rdfs:comment "If true, the Classifier can only be instantiated by instantiating one of its specializations. An abstract Classifier is intended to be used by other Classifiers e.g., as the target of Associations or Generalizations."@en ;
	rdfs:domain uml-class:Classifier ;
	rdfs:range xsd:boolean ;
	mms-ontology:umlPropertySource uml-property:Classifier-isAbstract .

mms-property:activityScopeActivity a mms-ontology:UmlObjectProperty ;
	mms-ontology:cardinality "1"^^uml-model-dt:cardinalityRange ;
	mms-ontology:key "activityScopeId" ;
	rdfs:label "activityScopeActivity" ;
	rdfs:comment "The Activity that is the activityScope of this Variable. Based on the UML property 'Variable-activityScope' which is described as: An Activity that owns the Variable."@en ;
	rdfs:domain uml-class:Variable ;
	rdfs:range uml-class:Activity ;
	mms-ontology:umlPropertySource uml-property:Variable-activityScope .

mms-property:ownedOperationFromArtifact a mms-ontology:UmlObjectProperty ;
	mms-ontology:cardinality "*"^^uml-model-dt:cardinalityRange ;
	mms-ontology:key "ownedOperationIds" ;
	rdfs:label "ownedOperationFromArtifact" ;
	rdfs:comment "A Operation that belongs to this Artifact. Based on the UML property 'Artifact-ownedOperation' which is described as: The Operations defined for the Artifact. The association is a specialization of the ownedMember association."@en ;
	rdfs:domain uml-class:Artifact ;
	rdfs:range uml-class:Operation ;
	mms-ontology:umlPropertySource uml-property:Artifact-ownedOperation .

mms-property:ownedOperationFromInterface a mms-ontology:UmlObjectProperty ;
	mms-ontology:cardinality "*"^^uml-model-dt:cardinalityRange ;
	mms-ontology:key "ownedOperationIds" ;
	rdfs:label "ownedOperationFromInterface" ;
	rdfs:comment "A Operation that belongs to this Interface. Based on the UML property 'Interface-ownedOperation' which is described as: The Operations owned by the Interface."@en ;
	rdfs:domain uml-class:Interface ;
	rdfs:range uml-class:Operation ;
	mms-ontology:umlPropertySource uml-property:Interface-ownedOperation .

mms-property:ownedOperationFromDataType a mms-ontology:UmlObjectProperty ;
	mms-ontology:cardinality "*"^^uml-model-dt:cardinalityRange ;
	mms-ontology:key "ownedOperationIds" ;
	rdfs:label "ownedOperationFromDataType" ;
	rdfs:comment "A Operation that belongs to this DataType. Based on the UML property 'DataType-ownedOperation' which is described as: The Operations owned by the DataType."@en ;
	rdfs:domain uml-class:DataType ;
	rdfs:range uml-class:Operation ;
	mms-ontology:umlPropertySource uml-property:DataType-ownedOperation .

mms-property:ownedOperationFromClass a mms-ontology:UmlObjectProperty ;
	mms-ontology:cardinality "*"^^uml-model-dt:cardinalityRange ;
	mms-ontology:key "ownedOperationIds" ;
	rdfs:label "ownedOperationFromClass" ;
	rdfs:comment "A Operation that belongs to this Class. Based on the UML property 'Class-ownedOperation' which is described as: The Operations owned by the Class."@en ;
	rdfs:domain uml-class:Class ;
	rdfs:range uml-class:Operation ;
	mms-ontology:umlPropertySource uml-property:Class-ownedOperation .

mms-property:firstInputPin a mms-ontology:UmlObjectProperty ;
	mms-ontology:cardinality "1"^^uml-model-dt:cardinalityRange ;
	mms-ontology:key "firstId" ;
	rdfs:label "firstInputPin" ;
	rdfs:comment "The InputPin that is the first of this TestIdentityAction. Based on the UML property 'TestIdentityAction-first' which is described as: The InputPin on which the first input object is placed."@en ;
	rdfs:domain uml-class:TestIdentityAction ;
	rdfs:range uml-class:InputPin ;
	mms-ontology:umlPropertySource uml-property:TestIdentityAction-first .

mms-property:exceptionType a mms-ontology:UmlObjectProperty ;
	mms-ontology:cardinality "*"^^uml-model-dt:cardinalityRange ;
	mms-ontology:key "exceptionTypeIds" ;
	rdfs:label "exceptionType" ;
	rdfs:comment "A Classifier that is the exceptionType of this ExceptionHandler. Based on the UML property 'ExceptionHandler-exceptionType' which is described as: The Classifiers whose instances the ExceptionHandler catches as exceptions. If an exception occurs whose type is any exceptionType, the ExceptionHandler catches the exception and executes the handlerBody."@en ;
	rdfs:domain uml-class:ExceptionHandler ;
	rdfs:range uml-class:Classifier ;
	mms-ontology:umlPropertySource uml-property:ExceptionHandler-exceptionType .

mms-property:associationEndProperty a mms-ontology:UmlObjectProperty ;
	mms-ontology:cardinality "1"^^uml-model-dt:cardinalityRange ;
	mms-ontology:key "associationEndId" ;
	rdfs:label "associationEndProperty" ;
	rdfs:comment "The Property that is the associationEnd of this Property. Based on the UML property 'Property-associationEnd' which is described as: Designates the optional association end that owns a qualifier attribute."@en ;
	rdfs:domain uml-class:Property ;
	rdfs:range uml-class:Property ;
	mms-ontology:umlPropertySource uml-property:Property-associationEnd .

mms-property:isFinalSpecialization a mms-ontology:UmlDatatypeProperty ;
	mms-ontology:key "isFinalSpecialization" ;
	rdfs:label "isFinalSpecialization" ;
	rdfs:comment "If true, the Classifier cannot be specialized."@en ;
	rdfs:domain uml-class:Classifier ;
	rdfs:range xsd:boolean ;
	mms-ontology:umlPropertySource uml-property:Classifier-isFinalSpecialization .

mms-property:isFinalSpecializationClassifier a mms-ontology:UmlDatatypeProperty ;
	owl:equivalentProperty mms-property:isFinalSpecialization .

mms-property:regionFromState a mms-ontology:UmlObjectProperty ;
	mms-ontology:cardinality "*"^^uml-model-dt:cardinalityRange ;
	mms-ontology:key "regionIds" ;
	rdfs:label "regionFromState" ;
	rdfs:comment "A Region that belongs to this State. Based on the UML property 'State-region' which is described as: The Regions owned directly by the State."@en ;
	rdfs:domain uml-class:State ;
	rdfs:range uml-class:Region ;
	mms-ontology:umlPropertySource uml-property:State-region .

mms-property:regionFromStateMachine a mms-ontology:UmlObjectProperty ;
	mms-ontology:cardinality "*"^^uml-model-dt:cardinalityRange ;
	mms-ontology:key "regionIds" ;
	rdfs:label "regionFromStateMachine" ;
	rdfs:comment "A Region that belongs to this StateMachine. Based on the UML property 'StateMachine-region' which is described as: The Regions owned directly by the StateMachine."@en ;
	rdfs:domain uml-class:StateMachine ;
	rdfs:range uml-class:Region ;
	mms-ontology:umlPropertySource uml-property:StateMachine-region .

mms-property:onPort a mms-ontology:UmlObjectProperty ;
	mms-ontology:cardinality "1"^^uml-model-dt:cardinalityRange ;
	mms-ontology:key "onPortId" ;
	rdfs:label "onPort" ;
	rdfs:comment "The Port that belongs to this InvocationAction. Based on the UML property 'InvocationAction-onPort' which is described as: For CallOperationActions, SendSignalActions, and SendObjectActions, an optional Port of the target object through which the invocation request is sent."@en ;
	rdfs:domain uml-class:InvocationAction ;
	rdfs:range uml-class:Port ;
	mms-ontology:umlPropertySource uml-property:InvocationAction-onPort .

mms-property:exceptionInputObjectNode a mms-ontology:UmlObjectProperty ;
	mms-ontology:cardinality "1"^^uml-model-dt:cardinalityRange ;
	mms-ontology:key "exceptionInputId" ;
	rdfs:label "exceptionInputObjectNode" ;
	rdfs:comment "The ObjectNode that is the exceptionInput of this ExceptionHandler. Based on the UML property 'ExceptionHandler-exceptionInput' which is described as: An ObjectNode within the handlerBody. When the ExceptionHandler catches an exception, the exception token is placed on this ObjectNode, causing the handlerBody to execute."@en ;
	rdfs:domain uml-class:ExceptionHandler ;
	rdfs:range uml-class:ObjectNode ;
	mms-ontology:umlPropertySource uml-property:ExceptionHandler-exceptionInput .

mms-property:powertypeExtent a mms-ontology:UmlObjectProperty ;
	mms-ontology:cardinality "*"^^uml-model-dt:cardinalityRange ;
	mms-ontology:key "powertypeExtentIds" ;
	rdfs:label "powertypeExtent" ;
	rdfs:comment "A GeneralizationSet that is the powertypeExtent of this Classifier. Based on the UML property 'Classifier-powertypeExtent' which is described as: The GeneralizationSet of which this Classifier is a power type."@en ;
	rdfs:domain uml-class:Classifier ;
	rdfs:range uml-class:GeneralizationSet ;
	mms-ontology:umlPropertySource uml-property:Classifier-powertypeExtent .

mms-property:superPartitionActivityPartition a mms-ontology:UmlObjectProperty ;
	mms-ontology:cardinality "1"^^uml-model-dt:cardinalityRange ;
	mms-ontology:key "superPartitionId" ;
	rdfs:label "superPartitionActivityPartition" ;
	rdfs:comment "The ActivityPartition that is the superPartition of this ActivityPartition. Based on the UML property 'ActivityPartition-superPartition' which is described as: Other ActivityPartitions immediately containing this ActivityPartition (as its superGroups)."@en ;
	rdfs:domain uml-class:ActivityPartition ;
	rdfs:range uml-class:ActivityPartition ;
	mms-ontology:umlPropertySource uml-property:ActivityPartition-superPartition .

mms-property:isCombineDuplicate a mms-ontology:UmlDatatypeProperty ;
	mms-ontology:key "isCombineDuplicate" ;
	rdfs:label "isCombineDuplicate" ;
	rdfs:comment "Indicates whether incoming tokens having objects with the same identity are combined into one by the JoinNode."@en ;
	rdfs:domain uml-class:JoinNode ;
	rdfs:range xsd:boolean ;
	mms-ontology:umlPropertySource uml-property:JoinNode-isCombineDuplicate .

mms-property:isCombineDuplicateJoinNode a mms-ontology:UmlDatatypeProperty ;
	owl:equivalentProperty mms-property:isCombineDuplicate .

mms-property:actionFromActionExecutionSpecification a mms-ontology:UmlObjectProperty ;
	mms-ontology:cardinality "1"^^uml-model-dt:cardinalityRange ;
	mms-ontology:key "actionId" ;
	rdfs:label "actionFromActionExecutionSpecification" ;
	rdfs:comment "The Action that belongs to this ActionExecutionSpecification. Based on the UML property 'ActionExecutionSpecification-action' which is described as: Action whose execution is occurring."@en ;
	rdfs:domain uml-class:ActionExecutionSpecification ;
	rdfs:range uml-class:Action ;
	mms-ontology:umlPropertySource uml-property:ActionExecutionSpecification-action .

mms-property:actionFromInteraction a mms-ontology:UmlObjectProperty ;
	mms-ontology:cardinality "*"^^uml-model-dt:cardinalityRange ;
	mms-ontology:key "actionIds" ;
	rdfs:label "actionFromInteraction" ;
	rdfs:comment "A Action that belongs to this Interaction. Based on the UML property 'Interaction-action' which is described as: Actions owned by the Interaction."@en ;
	rdfs:domain uml-class:Interaction ;
	rdfs:range uml-class:Action ;
	mms-ontology:umlPropertySource uml-property:Interaction-action .

mms-property:structuralFeature a mms-ontology:UmlObjectProperty ;
	mms-ontology:cardinality "1"^^uml-model-dt:cardinalityRange ;
	mms-ontology:key "structuralFeatureId" ;
	rdfs:label "structuralFeature" ;
	rdfs:comment "The StructuralFeature that belongs to this StructuralFeatureAction. Based on the UML property 'StructuralFeatureAction-structuralFeature' which is described as: The StructuralFeature to be read or written."@en ;
	rdfs:domain uml-class:StructuralFeatureAction ;
	rdfs:range uml-class:StructuralFeature ;
	mms-ontology:umlPropertySource uml-property:StructuralFeatureAction-structuralFeature .

mms-property:aliasString a mms-ontology:UmlDatatypeProperty ;
	mms-ontology:cardinality "1"^^uml-model-dt:cardinalityRange ;
	mms-ontology:key "aliasId" ;
	rdfs:label "aliasString" ;
	rdfs:comment "The String that is the alias of this ElementImport. Based on the UML property 'ElementImport-alias' which is described as: Specifies the name that should be added to the importing Namespace in lieu of the name of the imported PackagableElement. The alias must not clash with any other member in the importing Namespace. By default, no alias is used."@en ;
	rdfs:domain uml-class:ElementImport ;
	rdfs:range xsd:string ;
	mms-ontology:umlPropertySource uml-property:ElementImport-alias .

mms-property:connection a mms-ontology:UmlObjectProperty ;
	mms-ontology:cardinality "*"^^uml-model-dt:cardinalityRange ;
	mms-ontology:key "connectionIds" ;
	rdfs:label "connection" ;
	rdfs:comment "A ConnectionPointReference that is the connection of this State. Based on the UML property 'State-connection' which is described as: The entry and exit connection points used in conjunction with this (submachine) State, i.e., as targets and sources, respectively, in the Region with the submachine State. A connection point reference references the corresponding definition of a connection point Pseudostate in the StateMachine referenced by the submachine State."@en ;
	rdfs:domain uml-class:State ;
	rdfs:range uml-class:ConnectionPointReference ;
	mms-ontology:umlPropertySource uml-property:State-connection .

mms-property:definingFeatureStructuralFeature a mms-ontology:UmlObjectProperty ;
	mms-ontology:cardinality "1"^^uml-model-dt:cardinalityRange ;
	mms-ontology:key "definingFeatureId" ;
	rdfs:label "definingFeatureStructuralFeature" ;
	rdfs:comment "The StructuralFeature that is the definingFeature of this Slot. Based on the UML property 'Slot-definingFeature' which is described as: The StructuralFeature that specifies the values that may be held by the Slot."@en ;
	rdfs:domain uml-class:Slot ;
	rdfs:range uml-class:StructuralFeature ;
	mms-ontology:umlPropertySource uml-property:Slot-definingFeature .

mms-property:redefinedTransition a mms-ontology:UmlObjectProperty ;
	mms-ontology:cardinality "1"^^uml-model-dt:cardinalityRange ;
	mms-ontology:key "redefinedTransitionId" ;
	rdfs:label "redefinedTransition" ;
	rdfs:comment "The Transition that belongs to this Transition. Based on the UML property 'Transition-redefinedTransition' which is described as: The Transition that is redefined by this Transition."@en ;
	rdfs:domain uml-class:Transition ;
	rdfs:range uml-class:Transition ;
	mms-ontology:umlPropertySource uml-property:Transition-redefinedTransition .

mms-property:realizingActivityEdge a mms-ontology:UmlObjectProperty ;
	mms-ontology:cardinality "*"^^uml-model-dt:cardinalityRange ;
	mms-ontology:key "realizingActivityEdgeIds" ;
	rdfs:label "realizingActivityEdge" ;
	rdfs:comment "A ActivityEdge that belongs to this InformationFlow. Based on the UML property 'InformationFlow-realizingActivityEdge' which is described as: Determines which ActivityEdges will realize the specified flow."@en ;
	rdfs:domain uml-class:InformationFlow ;
	rdfs:range uml-class:ActivityEdge ;
	mms-ontology:umlPropertySource uml-property:InformationFlow-realizingActivityEdge .

mms-property:isReadOnlyActivity a mms-ontology:UmlDatatypeProperty ;
	mms-ontology:key "isReadOnly" ;
	rdfs:label "isReadOnlyActivity" ;
	rdfs:comment "If true, this Activity must not make any changes to objects. The default is false (an Activity may make nonlocal changes). (This is an assertion, not an executable property. It may be used by an execution engine to optimize model execution. If the assertion is violated by the Activity, then the model is ill-formed.) "@en ;
	rdfs:domain uml-class:Activity ;
	rdfs:range xsd:boolean ;
	mms-ontology:umlPropertySource uml-property:Activity-isReadOnly .

mms-property:isReadOnlyStructuralFeature a mms-ontology:UmlDatatypeProperty ;
	mms-ontology:key "isReadOnly" ;
	rdfs:label "isReadOnlyStructuralFeature" ;
	rdfs:comment "If isReadOnly is true, the StructuralFeature may not be written to after initialization."@en ;
	rdfs:domain uml-class:StructuralFeature ;
	rdfs:range xsd:boolean ;
	mms-ontology:umlPropertySource uml-property:StructuralFeature-isReadOnly .

mms-property:decisionInputFlowObjectFlow a mms-ontology:UmlObjectProperty ;
	mms-ontology:cardinality "1"^^uml-model-dt:cardinalityRange ;
	mms-ontology:key "decisionInputFlowId" ;
	rdfs:label "decisionInputFlowObjectFlow" ;
	rdfs:comment "The ObjectFlow that is the decisionInputFlow of this DecisionNode. Based on the UML property 'DecisionNode-decisionInputFlow' which is described as: An additional ActivityEdge incoming to the DecisionNode that provides a decision input value for the guards ValueSpecifications on ActivityEdges outgoing from the DecisionNode."@en ;
	rdfs:domain uml-class:DecisionNode ;
	rdfs:range uml-class:ObjectFlow ;
	mms-ontology:umlPropertySource uml-property:DecisionNode-decisionInputFlow .

mms-property:inheritedMember a mms-ontology:UmlObjectProperty ;
	mms-ontology:cardinality "*"^^uml-model-dt:cardinalityRange ;
	mms-ontology:key "inheritedMemberIds" ;
	rdfs:label "inheritedMember" ;
	rdfs:comment "A NamedElement that is the inheritedMember of this Classifier. Based on the UML property 'Classifier-inheritedMember' which is described as: All elements inherited by this Classifier from its general Classifiers."@en ;
	rdfs:domain uml-class:Classifier ;
	rdfs:range uml-class:NamedElement ;
	mms-ontology:umlPropertySource uml-property:Classifier-inheritedMember .

mms-property:partition a mms-ontology:UmlObjectProperty ;
	mms-ontology:cardinality "*"^^uml-model-dt:cardinalityRange ;
	mms-ontology:key "partitionIds" ;
	rdfs:label "partition" ;
	rdfs:comment "A ActivityPartition that is the partition of this Activity. Based on the UML property 'Activity-partition' which is described as: Top-level ActivityPartitions in the Activity."@en ;
	rdfs:domain uml-class:Activity ;
	rdfs:range uml-class:ActivityPartition ;
	mms-ontology:umlPropertySource uml-property:Activity-partition .

mms-property:returnInformationInputPin a mms-ontology:UmlObjectProperty ;
	mms-ontology:cardinality "1"^^uml-model-dt:cardinalityRange ;
	mms-ontology:key "returnInformationId" ;
	rdfs:label "returnInformationInputPin" ;
	rdfs:comment "The InputPin that is the returnInformation of this ReplyAction. Based on the UML property 'ReplyAction-returnInformation' which is described as: An InputPin that holds the return information value produced by an earlier AcceptCallAction."@en ;
	rdfs:domain uml-class:ReplyAction ;
	rdfs:range uml-class:InputPin ;
	mms-ontology:umlPropertySource uml-property:ReplyAction-returnInformation .

mms-property:returnInformationOutputPin a mms-ontology:UmlObjectProperty ;
	mms-ontology:cardinality "1"^^uml-model-dt:cardinalityRange ;
	mms-ontology:key "returnInformationId" ;
	rdfs:label "returnInformationOutputPin" ;
	rdfs:comment "The OutputPin that is the returnInformation of this AcceptCallAction. Based on the UML property 'AcceptCallAction-returnInformation' which is described as: An OutputPin where a value is placed containing sufficient information to perform a subsequent ReplyAction and return control to the caller. The contents of this value are opaque. It can be passed and copied but it cannot be manipulated by the model."@en ;
	rdfs:domain uml-class:AcceptCallAction ;
	rdfs:range uml-class:OutputPin ;
	mms-ontology:umlPropertySource uml-property:AcceptCallAction-returnInformation .

mms-property:metamodelReference a mms-ontology:UmlObjectProperty ;
	mms-ontology:cardinality "*"^^uml-model-dt:cardinalityRange ;
	mms-ontology:key "metamodelReferenceIds" ;
	rdfs:label "metamodelReference" ;
	rdfs:comment "A PackageImport that is the metamodelReference of this Profile. Based on the UML property 'Profile-metamodelReference' which is described as: References a package containing (directly or indirectly) metaclasses that may be extended."@en ;
	rdfs:domain uml-class:Profile ;
	rdfs:range uml-class:PackageImport ;
	mms-ontology:umlPropertySource uml-property:Profile-metamodelReference .

mms-property:variableFromActivity a mms-ontology:UmlObjectProperty ;
	mms-ontology:cardinality "*"^^uml-model-dt:cardinalityRange ;
	mms-ontology:key "variableIds" ;
	rdfs:label "variableFromActivity" ;
	rdfs:comment "A Variable that belongs to this Activity. Based on the UML property 'Activity-variable' which is described as: Top-level Variables defined by the Activity."@en ;
	rdfs:domain uml-class:Activity ;
	rdfs:range uml-class:Variable ;
	mms-ontology:umlPropertySource uml-property:Activity-variable .

mms-property:variableFromVariableAction a mms-ontology:UmlObjectProperty ;
	mms-ontology:cardinality "1"^^uml-model-dt:cardinalityRange ;
	mms-ontology:key "variableId" ;
	rdfs:label "variableFromVariableAction" ;
	rdfs:comment "The Variable that belongs to this VariableAction. Based on the UML property 'VariableAction-variable' which is described as: The Variable to be read or written."@en ;
	rdfs:domain uml-class:VariableAction ;
	rdfs:range uml-class:Variable ;
	mms-ontology:umlPropertySource uml-property:VariableAction-variable .

mms-property:variableFromStructuredActivityNode a mms-ontology:UmlObjectProperty ;
	mms-ontology:cardinality "*"^^uml-model-dt:cardinalityRange ;
	mms-ontology:key "variableIds" ;
	rdfs:label "variableFromStructuredActivityNode" ;
	rdfs:comment "A Variable that belongs to this StructuredActivityNode. Based on the UML property 'StructuredActivityNode-variable' which is described as: The Variables defined in the scope of the StructuredActivityNode."@en ;
	rdfs:domain uml-class:StructuredActivityNode ;
	rdfs:range uml-class:Variable ;
	mms-ontology:umlPropertySource uml-property:StructuredActivityNode-variable .

mms-property:interruptingEdge a mms-ontology:UmlObjectProperty ;
	mms-ontology:cardinality "*"^^uml-model-dt:cardinalityRange ;
	mms-ontology:key "interruptingEdgeIds" ;
	rdfs:label "interruptingEdge" ;
	rdfs:comment "A ActivityEdge that is the interruptingEdge of this InterruptibleActivityRegion. Based on the UML property 'InterruptibleActivityRegion-interruptingEdge' which is described as: The ActivityEdges leaving the InterruptibleActivityRegion on which a traversing token will result in the termination of other tokens flowing in the InterruptibleActivityRegion."@en ;
	rdfs:domain uml-class:InterruptibleActivityRegion ;
	rdfs:range uml-class:ActivityEdge ;
	mms-ontology:umlPropertySource uml-property:InterruptibleActivityRegion-interruptingEdge .

mms-property:extendedStateMachine a mms-ontology:UmlObjectProperty ;
	mms-ontology:cardinality "*"^^uml-model-dt:cardinalityRange ;
	mms-ontology:key "extendedStateMachineIds" ;
	rdfs:label "extendedStateMachine" ;
	rdfs:comment "A StateMachine that belongs to this StateMachine. Based on the UML property 'StateMachine-extendedStateMachine' which is described as: The StateMachines of which this is an extension."@en ;
	rdfs:domain uml-class:StateMachine ;
	rdfs:range uml-class:StateMachine ;
	mms-ontology:umlPropertySource uml-property:StateMachine-extendedStateMachine .

mms-property:toBefore a mms-ontology:UmlObjectProperty ;
	mms-ontology:cardinality "*"^^uml-model-dt:cardinalityRange ;
	mms-ontology:key "toBeforeIds" ;
	rdfs:label "toBefore" ;
	rdfs:comment "A GeneralOrdering that is the toBefore of this OccurrenceSpecification. Based on the UML property 'OccurrenceSpecification-toBefore' which is described as: References the GeneralOrderings that specify EventOcurrences that must occur before this OccurrenceSpecification."@en ;
	rdfs:domain uml-class:OccurrenceSpecification ;
	rdfs:range uml-class:GeneralOrdering ;
	mms-ontology:umlPropertySource uml-property:OccurrenceSpecification-toBefore .

mms-property:extend a mms-ontology:UmlObjectProperty ;
	mms-ontology:cardinality "*"^^uml-model-dt:cardinalityRange ;
	mms-ontology:key "extendIds" ;
	rdfs:label "extend" ;
	rdfs:comment "A Extend that belongs to this UseCase. Based on the UML property 'UseCase-extend' which is described as: The Extend relationships owned by this UseCase."@en ;
	rdfs:domain uml-class:UseCase ;
	rdfs:range uml-class:Extend ;
	mms-ontology:umlPropertySource uml-property:UseCase-extend .

mms-property:loopVariable a mms-ontology:UmlObjectProperty ;
	mms-ontology:cardinality "*"^^uml-model-dt:cardinalityRange ;
	mms-ontology:key "loopVariableIds" ;
	rdfs:label "loopVariable" ;
	rdfs:comment "A OutputPin that is the loopVariable of this LoopNode. Based on the UML property 'LoopNode-loopVariable' which is described as: A list of OutputPins that hold the values of the loop variables during an execution of the loop. When the test fails, the values are moved to the result OutputPins of the loop."@en ;
	rdfs:domain uml-class:LoopNode ;
	rdfs:range uml-class:OutputPin ;
	mms-ontology:umlPropertySource uml-property:LoopNode-loopVariable .

mms-property:effectBehavior a mms-ontology:UmlObjectProperty ;
	mms-ontology:cardinality "1"^^uml-model-dt:cardinalityRange ;
	mms-ontology:key "effectId" ;
	rdfs:label "effectBehavior" ;
	rdfs:comment "The Behavior that is the effect of this Transition. Based on the UML property 'Transition-effect' which is described as: Specifies an optional behavior to be performed when the Transition fires."@en ;
	rdfs:domain uml-class:Transition ;
	rdfs:range uml-class:Behavior ;
	mms-ontology:umlPropertySource uml-property:Transition-effect .

mms-property:interactionFromMessage a mms-ontology:UmlObjectProperty ;
	mms-ontology:cardinality "1"^^uml-model-dt:cardinalityRange ;
	mms-ontology:key "interactionId" ;
	rdfs:label "interactionFromMessage" ;
	rdfs:comment "The Interaction that belongs to this Message. Based on the UML property 'Message-interaction' which is described as: The enclosing Interaction owning the Message."@en ;
	rdfs:domain uml-class:Message ;
	rdfs:range uml-class:Interaction ;
	mms-ontology:umlPropertySource uml-property:Message-interaction .

mms-property:interactionFromLifeline a mms-ontology:UmlObjectProperty ;
	mms-ontology:cardinality "1"^^uml-model-dt:cardinalityRange ;
	mms-ontology:key "interactionId" ;
	rdfs:label "interactionFromLifeline" ;
	rdfs:comment "The Interaction that belongs to this Lifeline. Based on the UML property 'Lifeline-interaction' which is described as: References the Interaction enclosing this Lifeline."@en ;
	rdfs:domain uml-class:Lifeline ;
	rdfs:range uml-class:Interaction ;
	mms-ontology:umlPropertySource uml-property:Lifeline-interaction .

mms-property:isActive a mms-ontology:UmlDatatypeProperty ;
	mms-ontology:key "isActive" ;
	rdfs:label "isActive" ;
	rdfs:comment "Determines whether an object specified by this Class is active or not. If true, then the owning Class is referred to as an active Class. If false, then such a Class is referred to as a passive Class."@en ;
	rdfs:domain uml-class:Class ;
	rdfs:range xsd:boolean ;
	mms-ontology:umlPropertySource uml-property:Class-isActive .

mms-property:isActiveClass a mms-ontology:UmlDatatypeProperty ;
	owl:equivalentProperty mms-property:isActive .

mms-property:selectionBehaviorFromObjectFlow a mms-ontology:UmlObjectProperty ;
	mms-ontology:cardinality "1"^^uml-model-dt:cardinalityRange ;
	mms-ontology:key "selectionId" ;
	rdfs:label "selectionBehaviorFromObjectFlow" ;
	rdfs:comment "The Behavior that is the selection of this ObjectFlow. Based on the UML property 'ObjectFlow-selection' which is described as: A Behavior used to select tokens from a source ObjectNode."@en ;
	rdfs:domain uml-class:ObjectFlow ;
	rdfs:range uml-class:Behavior ;
	mms-ontology:umlPropertySource uml-property:ObjectFlow-selection .

mms-property:selectionBehaviorFromObjectNode a mms-ontology:UmlObjectProperty ;
	mms-ontology:cardinality "1"^^uml-model-dt:cardinalityRange ;
	mms-ontology:key "selectionId" ;
	rdfs:label "selectionBehaviorFromObjectNode" ;
	rdfs:comment "The Behavior that is the selection of this ObjectNode. Based on the UML property 'ObjectNode-selection' which is described as: A Behavior used to select tokens to be offered on outgoing ActivityEdges."@en ;
	rdfs:domain uml-class:ObjectNode ;
	rdfs:range uml-class:Behavior ;
	mms-ontology:umlPropertySource uml-property:ObjectNode-selection .

mms-property:powertypeClassifier a mms-ontology:UmlObjectProperty ;
	mms-ontology:cardinality "1"^^uml-model-dt:cardinalityRange ;
	mms-ontology:key "powertypeId" ;
	rdfs:label "powertypeClassifier" ;
	rdfs:comment "The Classifier that is the powertype of this GeneralizationSet. Based on the UML property 'GeneralizationSet-powertype' which is described as: Designates the Classifier that is defined as the power type for the associated GeneralizationSet, if there is one."@en ;
	rdfs:domain uml-class:GeneralizationSet ;
	rdfs:range uml-class:Classifier ;
	mms-ontology:umlPropertySource uml-property:GeneralizationSet-powertype .

mms-property:bodyOutputFromClause a mms-ontology:UmlObjectProperty ;
	mms-ontology:cardinality "*"^^uml-model-dt:cardinalityRange ;
	mms-ontology:key "bodyOutputIds" ;
	rdfs:label "bodyOutputFromClause" ;
	rdfs:comment "A OutputPin that is the bodyOutput of this Clause. Based on the UML property 'Clause-bodyOutput' which is described as: The OutputPins on Actions within the body section whose values are moved to the result OutputPins of the containing ConditionalNode after execution of the body."@en ;
	rdfs:domain uml-class:Clause ;
	rdfs:range uml-class:OutputPin ;
	mms-ontology:umlPropertySource uml-property:Clause-bodyOutput .

mms-property:bodyOutputFromLoopNode a mms-ontology:UmlObjectProperty ;
	mms-ontology:cardinality "*"^^uml-model-dt:cardinalityRange ;
	mms-ontology:key "bodyOutputIds" ;
	rdfs:label "bodyOutputFromLoopNode" ;
	rdfs:comment "A OutputPin that is the bodyOutput of this LoopNode. Based on the UML property 'LoopNode-bodyOutput' which is described as: The OutputPins on Actions within the bodyPart, the values of which are moved to the loopVariable OutputPins after the completion of each execution of the bodyPart, before the next iteration of the loop begins or before the loop exits."@en ;
	rdfs:domain uml-class:LoopNode ;
	rdfs:range uml-class:OutputPin ;
	mms-ontology:umlPropertySource uml-property:LoopNode-bodyOutput .

mms-property:output a mms-ontology:UmlObjectProperty ;
	mms-ontology:cardinality "*"^^uml-model-dt:cardinalityRange ;
	mms-ontology:key "outputIds" ;
	rdfs:label "output" ;
	rdfs:comment "A OutputPin that is the output of this Action. Based on the UML property 'Action-output' which is described as: The ordered set of OutputPins representing outputs from the Action."@en ;
	rdfs:domain uml-class:Action ;
	rdfs:range uml-class:OutputPin ;
	mms-ontology:umlPropertySource uml-property:Action-output .

mms-property:inState a mms-ontology:UmlObjectProperty ;
	mms-ontology:cardinality "*"^^uml-model-dt:cardinalityRange ;
	mms-ontology:key "inStateIds" ;
	rdfs:label "inState" ;
	rdfs:comment "A State that belongs to this ObjectNode. Based on the UML property 'ObjectNode-inState' which is described as: The States required to be associated with the values held by tokens on this ObjectNode."@en ;
	rdfs:domain uml-class:ObjectNode ;
	rdfs:range uml-class:State ;
	mms-ontology:umlPropertySource uml-property:ObjectNode-inState .

mms-property:profileApplication a mms-ontology:UmlObjectProperty ;
	mms-ontology:cardinality "*"^^uml-model-dt:cardinalityRange ;
	mms-ontology:key "profileApplicationIds" ;
	rdfs:label "profileApplication" ;
	rdfs:comment "A ProfileApplication that belongs to this Package. Based on the UML property 'Package-profileApplication' which is described as: References the ProfileApplications that indicate which profiles have been applied to the Package."@en ;
	rdfs:domain uml-class:Package ;
	rdfs:range uml-class:ProfileApplication ;
	mms-ontology:umlPropertySource uml-property:Package-profileApplication .

mms-property:package a mms-ontology:UmlObjectProperty ;
	mms-ontology:cardinality "1"^^uml-model-dt:cardinalityRange ;
	mms-ontology:key "packageId" ;
	rdfs:label "package" ;
	rdfs:comment "The Package that belongs to this Type. Based on the UML property 'Type-package' which is described as: Specifies the owning Package of this Type, if any."@en ;
	rdfs:domain uml-class:Type ;
	rdfs:range uml-class:Package ;
	mms-ontology:umlPropertySource uml-property:Type-package .

mms-property:isOrthogonal a mms-ontology:UmlDatatypeProperty ;
	mms-ontology:key "isOrthogonal" ;
	rdfs:label "isOrthogonal" ;
	rdfs:comment "A State with isOrthogonal=true is said to be an orthogonal composite State An orthogonal composite State contains two or more Regions."@en ;
	rdfs:domain uml-class:State ;
	rdfs:range xsd:boolean ;
	mms-ontology:umlPropertySource uml-property:State-isOrthogonal .

mms-property:isOrthogonalState a mms-ontology:UmlDatatypeProperty ;
	owl:equivalentProperty mms-property:isOrthogonal .

mms-property:returnValueValueSpecification a mms-ontology:UmlObjectProperty ;
	mms-ontology:cardinality "1"^^uml-model-dt:cardinalityRange ;
	mms-ontology:key "returnValueId" ;
	rdfs:label "returnValueValueSpecification" ;
	rdfs:comment "The ValueSpecification that is the returnValue of this InteractionUse. Based on the UML property 'InteractionUse-returnValue' which is described as: The value of the executed Interaction."@en ;
	rdfs:domain uml-class:InteractionUse ;
	rdfs:range uml-class:ValueSpecification ;
	mms-ontology:umlPropertySource uml-property:InteractionUse-returnValue .

mms-property:nestedPackage a mms-ontology:UmlObjectProperty ;
	mms-ontology:cardinality "*"^^uml-model-dt:cardinalityRange ;
	mms-ontology:key "nestedPackageIds" ;
	rdfs:label "nestedPackage" ;
	rdfs:comment "A Package that belongs to this Package. Based on the UML property 'Package-nestedPackage' which is described as: References the packaged elements that are Packages."@en ;
	rdfs:domain uml-class:Package ;
	rdfs:range uml-class:Package ;
	mms-ontology:umlPropertySource uml-property:Package-nestedPackage .

mms-property:sendEventMessageEnd a mms-ontology:UmlObjectProperty ;
	mms-ontology:cardinality "1"^^uml-model-dt:cardinalityRange ;
	mms-ontology:key "sendEventId" ;
	rdfs:label "sendEventMessageEnd" ;
	rdfs:comment "The MessageEnd that is the sendEvent of this Message. Based on the UML property 'Message-sendEvent' which is described as: References the Sending of the Message."@en ;
	rdfs:domain uml-class:Message ;
	rdfs:range uml-class:MessageEnd ;
	mms-ontology:umlPropertySource uml-property:Message-sendEvent .

mms-property:oldClassifier a mms-ontology:UmlObjectProperty ;
	mms-ontology:cardinality "*"^^uml-model-dt:cardinalityRange ;
	mms-ontology:key "oldClassifierIds" ;
	rdfs:label "oldClassifier" ;
	rdfs:comment "A Classifier that belongs to this ReclassifyObjectAction. Based on the UML property 'ReclassifyObjectAction-oldClassifier' which is described as: A set of Classifiers to be removed from the Classifiers of the given object."@en ;
	rdfs:domain uml-class:ReclassifyObjectAction ;
	rdfs:range uml-class:Classifier ;
	mms-ontology:umlPropertySource uml-property:ReclassifyObjectAction-oldClassifier .

mms-property:isSubstitutable a mms-ontology:UmlDatatypeProperty ;
	mms-ontology:key "isSubstitutable" ;
	rdfs:label "isSubstitutable" ;
	rdfs:comment "Indicates whether the specific Classifier can be used wherever the general Classifier can be used. If true, the execution traces of the specific Classifier shall be a superset of the execution traces of the general Classifier. If false, there is no such constraint on execution traces. If unset, the modeler has not stated whether there is such a constraint or not."@en ;
	rdfs:domain uml-class:Generalization ;
	rdfs:range xsd:boolean ;
	mms-ontology:umlPropertySource uml-property:Generalization-isSubstitutable .

mms-property:isSubstitutableGeneralization a mms-ontology:UmlDatatypeProperty ;
	owl:equivalentProperty mms-property:isSubstitutable .

mms-property:isCovering a mms-ontology:UmlDatatypeProperty ;
	mms-ontology:key "isCovering" ;
	rdfs:label "isCovering" ;
	rdfs:comment "Indicates (via the associated Generalizations) whether or not the set of specific Classifiers are covering for a particular general classifier. When isCovering is true, every instance of a particular general Classifier is also an instance of at least one of its specific Classifiers for the GeneralizationSet. When isCovering is false, there are one or more instances of the particular general Classifier that are not instances of at least one of its specific Classifiers defined for the GeneralizationSet."@en ;
	rdfs:domain uml-class:GeneralizationSet ;
	rdfs:range xsd:boolean ;
	mms-ontology:umlPropertySource uml-property:GeneralizationSet-isCovering .

mms-property:isCoveringGeneralizationSet a mms-ontology:UmlDatatypeProperty ;
	owl:equivalentProperty mms-property:isCovering .

mms-property:localPostcondition a mms-ontology:UmlObjectProperty ;
	mms-ontology:cardinality "*"^^uml-model-dt:cardinalityRange ;
	mms-ontology:key "localPostconditionIds" ;
	rdfs:label "localPostcondition" ;
	rdfs:comment "A Constraint that is the localPostcondition of this Action. Based on the UML property 'Action-localPostcondition' which is described as: A Constraint that must be satisfied when execution of the Action is completed."@en ;
	rdfs:domain uml-class:Action ;
	rdfs:range uml-class:Constraint ;
	mms-ontology:umlPropertySource uml-property:Action-localPostcondition .

mms-property:nestedClassifierFromInterface a mms-ontology:UmlObjectProperty ;
	mms-ontology:cardinality "*"^^uml-model-dt:cardinalityRange ;
	mms-ontology:key "nestedClassifierIds" ;
	rdfs:label "nestedClassifierFromInterface" ;
	rdfs:comment "A Classifier that belongs to this Interface. Based on the UML property 'Interface-nestedClassifier' which is described as: References all the Classifiers that are defined (nested) within the Interface."@en ;
	rdfs:domain uml-class:Interface ;
	rdfs:range uml-class:Classifier ;
	mms-ontology:umlPropertySource uml-property:Interface-nestedClassifier .

mms-property:nestedClassifierFromClass a mms-ontology:UmlObjectProperty ;
	mms-ontology:cardinality "*"^^uml-model-dt:cardinalityRange ;
	mms-ontology:key "nestedClassifierIds" ;
	rdfs:label "nestedClassifierFromClass" ;
	rdfs:comment "A Classifier that belongs to this Class. Based on the UML property 'Class-nestedClassifier' which is described as: The Classifiers owned by the Class that are not ownedBehaviors."@en ;
	rdfs:domain uml-class:Class ;
	rdfs:range uml-class:Classifier ;
	mms-ontology:umlPropertySource uml-property:Class-nestedClassifier .

mms-property:decisionInputBehavior a mms-ontology:UmlObjectProperty ;
	mms-ontology:cardinality "1"^^uml-model-dt:cardinalityRange ;
	mms-ontology:key "decisionInputId" ;
	rdfs:label "decisionInputBehavior" ;
	rdfs:comment "The Behavior that is the decisionInput of this DecisionNode. Based on the UML property 'DecisionNode-decisionInput' which is described as: A Behavior that is executed to provide an input to guard ValueSpecifications on ActivityEdges outgoing from the DecisionNode."@en ;
	rdfs:domain uml-class:DecisionNode ;
	rdfs:range uml-class:Behavior ;
	mms-ontology:umlPropertySource uml-property:DecisionNode-decisionInput .

mms-property:isDirect a mms-ontology:UmlDatatypeProperty ;
	mms-ontology:key "isDirect" ;
	rdfs:label "isDirect" ;
	rdfs:comment "Indicates whether the input object must be directly classified by the given Classifier or whether it may also be an instance of a specialization of the given Classifier."@en ;
	rdfs:domain uml-class:ReadIsClassifiedObjectAction ;
	rdfs:range xsd:boolean ;
	mms-ontology:umlPropertySource uml-property:ReadIsClassifiedObjectAction-isDirect .

mms-property:isDirectReadIsClassifiedObjectAction a mms-ontology:UmlDatatypeProperty ;
	owl:equivalentProperty mms-property:isDirect .

mms-property:regionAsOutputExpansionRegion a mms-ontology:UmlObjectProperty ;
	mms-ontology:cardinality "1"^^uml-model-dt:cardinalityRange ;
	mms-ontology:key "regionAsOutputId" ;
	rdfs:label "regionAsOutputExpansionRegion" ;
	rdfs:comment "The ExpansionRegion that is the regionAsOutput of this ExpansionNode. Based on the UML property 'ExpansionNode-regionAsOutput' which is described as: The ExpansionRegion for which the ExpansionNode is an output."@en ;
	rdfs:domain uml-class:ExpansionNode ;
	rdfs:range uml-class:ExpansionRegion ;
	mms-ontology:umlPropertySource uml-property:ExpansionNode-regionAsOutput .

mms-property:receiveEventMessageEnd a mms-ontology:UmlObjectProperty ;
	mms-ontology:cardinality "1"^^uml-model-dt:cardinalityRange ;
	mms-ontology:key "receiveEventId" ;
	rdfs:label "receiveEventMessageEnd" ;
	rdfs:comment "The MessageEnd that is the receiveEvent of this Message. Based on the UML property 'Message-receiveEvent' which is described as: References the Receiving of the Message."@en ;
	rdfs:domain uml-class:Message ;
	rdfs:range uml-class:MessageEnd ;
	mms-ontology:umlPropertySource uml-property:Message-receiveEvent .

mms-property:actualParameterableElement a mms-ontology:UmlObjectProperty ;
	mms-ontology:cardinality "1"^^uml-model-dt:cardinalityRange ;
	mms-ontology:key "actualId" ;
	rdfs:label "actualParameterableElement" ;
	rdfs:comment "The ParameterableElement that is the actual of this TemplateParameterSubstitution. Based on the UML property 'TemplateParameterSubstitution-actual' which is described as: The ParameterableElement that is the actual parameter for this TemplateParameterSubstitution."@en ;
	rdfs:domain uml-class:TemplateParameterSubstitution ;
	rdfs:range uml-class:ParameterableElement ;
	mms-ontology:umlPropertySource uml-property:TemplateParameterSubstitution-actual .

mms-property:collectionInputPin a mms-ontology:UmlObjectProperty ;
	mms-ontology:cardinality "1"^^uml-model-dt:cardinalityRange ;
	mms-ontology:key "collectionId" ;
	rdfs:label "collectionInputPin" ;
	rdfs:comment "The InputPin that is the collection of this ReduceAction. Based on the UML property 'ReduceAction-collection' which is described as: The InputPin that provides the collection to be reduced."@en ;
	rdfs:domain uml-class:ReduceAction ;
	rdfs:range uml-class:InputPin ;
	mms-ontology:umlPropertySource uml-property:ReduceAction-collection .

mms-property:method a mms-ontology:UmlObjectProperty ;
	mms-ontology:cardinality "*"^^uml-model-dt:cardinalityRange ;
	mms-ontology:key "methodIds" ;
	rdfs:label "method" ;
	rdfs:comment "A Behavior that is the method of this BehavioralFeature. Based on the UML property 'BehavioralFeature-method' which is described as: A Behavior that implements the BehavioralFeature. There may be at most one Behavior for a particular pairing of a Classifier (as owner of the Behavior) and a BehavioralFeature (as specification of the Behavior)."@en ;
	rdfs:domain uml-class:BehavioralFeature ;
	rdfs:range uml-class:Behavior ;
	mms-ontology:umlPropertySource uml-property:BehavioralFeature-method .

mms-property:parameterSet a mms-ontology:UmlObjectProperty ;
	mms-ontology:cardinality "*"^^uml-model-dt:cardinalityRange ;
	mms-ontology:key "parameterSetIds" ;
	rdfs:label "parameterSet" ;
	rdfs:comment "A ParameterSet that belongs to this Parameter. Based on the UML property 'Parameter-parameterSet' which is described as: The ParameterSets containing the parameter. See ParameterSet."@en ;
	rdfs:domain uml-class:Parameter ;
	rdfs:range uml-class:ParameterSet ;
	mms-ontology:umlPropertySource uml-property:Parameter-parameterSet .

mms-property:executionLocationString a mms-ontology:UmlDatatypeProperty ;
	mms-ontology:cardinality "1"^^uml-model-dt:cardinalityRange ;
	mms-ontology:key "executionLocationId" ;
	rdfs:label "executionLocationString" ;
	rdfs:comment "The String that is the executionLocation of this DeploymentSpecification. Based on the UML property 'DeploymentSpecification-executionLocation' which is described as: The location where a component Artifact executes. This may be a local or remote location."@en ;
	rdfs:domain uml-class:DeploymentSpecification ;
	rdfs:range xsd:string ;
	mms-ontology:umlPropertySource uml-property:DeploymentSpecification-executionLocation .

mms-property:packageImport a mms-ontology:UmlObjectProperty ;
	mms-ontology:cardinality "*"^^uml-model-dt:cardinalityRange ;
	mms-ontology:key "packageImportIds" ;
	rdfs:label "packageImport" ;
	rdfs:comment "A PackageImport that belongs to this Namespace. Based on the UML property 'Namespace-packageImport' which is described as: References the PackageImports owned by the Namespace."@en ;
	rdfs:domain uml-class:Namespace ;
	rdfs:range uml-class:PackageImport ;
	mms-ontology:umlPropertySource uml-property:Namespace-packageImport .

mms-property:metaclassClass a mms-ontology:UmlObjectProperty ;
	mms-ontology:cardinality "1"^^uml-model-dt:cardinalityRange ;
	mms-ontology:key "metaclassId" ;
	rdfs:label "metaclassClass" ;
	rdfs:comment "The Class that is the metaclass of this Extension. Based on the UML property 'Extension-metaclass' which is described as: References the Class that is extended through an Extension. The property is derived from the type of the memberEnd that is not the ownedEnd."@en ;
	rdfs:domain uml-class:Extension ;
	rdfs:range uml-class:Class ;
	mms-ontology:umlPropertySource uml-property:Extension-metaclass .

mms-property:isDeterminate a mms-ontology:UmlDatatypeProperty ;
	mms-ontology:key "isDeterminate" ;
	rdfs:label "isDeterminate" ;
	rdfs:comment "If true, the modeler asserts that the test for at most one Clause of the ConditionalNode will succeed."@en ;
	rdfs:domain uml-class:ConditionalNode ;
	rdfs:range xsd:boolean ;
	mms-ontology:umlPropertySource uml-property:ConditionalNode-isDeterminate .

mms-property:isDeterminateConditionalNode a mms-ontology:UmlDatatypeProperty ;
	owl:equivalentProperty mms-property:isDeterminate .

mms-property:structuredNode a mms-ontology:UmlObjectProperty ;
	mms-ontology:cardinality "*"^^uml-model-dt:cardinalityRange ;
	mms-ontology:key "structuredNodeIds" ;
	rdfs:label "structuredNode" ;
	rdfs:comment "A StructuredActivityNode that is the structuredNode of this Activity. Based on the UML property 'Activity-structuredNode' which is described as: Top-level StructuredActivityNodes in the Activity."@en ;
	rdfs:domain uml-class:Activity ;
	rdfs:range uml-class:StructuredActivityNode ;
	mms-ontology:umlPropertySource uml-property:Activity-structuredNode .

mms-property:informationSource a mms-ontology:UmlObjectProperty ;
	mms-ontology:cardinality "*"^^uml-model-dt:cardinalityRange ;
	mms-ontology:key "informationSourceIds" ;
	rdfs:label "informationSource" ;
	rdfs:comment "A NamedElement that is the informationSource of this InformationFlow. Based on the UML property 'InformationFlow-informationSource' which is described as: Defines from which source the conveyed InformationItems are initiated."@en ;
	rdfs:domain uml-class:InformationFlow ;
	rdfs:range uml-class:NamedElement ;
	mms-ontology:umlPropertySource uml-property:InformationFlow-informationSource .

mms-property:whenTimeExpression a mms-ontology:UmlObjectProperty ;
	mms-ontology:cardinality "1"^^uml-model-dt:cardinalityRange ;
	mms-ontology:key "whenId" ;
	rdfs:label "whenTimeExpression" ;
	rdfs:comment "The TimeExpression that is the when of this TimeEvent. Based on the UML property 'TimeEvent-when' which is described as: Specifies the time of the TimeEvent."@en ;
	rdfs:domain uml-class:TimeEvent ;
	rdfs:range uml-class:TimeExpression ;
	mms-ontology:umlPropertySource uml-property:TimeEvent-when .

mms-property:superClass a mms-ontology:UmlObjectProperty ;
	mms-ontology:cardinality "*"^^uml-model-dt:cardinalityRange ;
	mms-ontology:key "superClassIds" ;
	rdfs:label "superClass" ;
	rdfs:comment "A Class that belongs to this Class. Based on the UML property 'Class-superClass' which is described as: The superclasses of a Class, derived from its Generalizations."@en ;
	rdfs:domain uml-class:Class ;
	rdfs:range uml-class:Class ;
	mms-ontology:umlPropertySource uml-property:Class-superClass .

mms-property:decomposedAsPartDecomposition a mms-ontology:UmlObjectProperty ;
	mms-ontology:cardinality "1"^^uml-model-dt:cardinalityRange ;
	mms-ontology:key "decomposedAsId" ;
	rdfs:label "decomposedAsPartDecomposition" ;
	rdfs:comment "The PartDecomposition that is the decomposedAs of this Lifeline. Based on the UML property 'Lifeline-decomposedAs' which is described as: References the Interaction that represents the decomposition."@en ;
	rdfs:domain uml-class:Lifeline ;
	rdfs:range uml-class:PartDecomposition ;
	mms-ontology:umlPropertySource uml-property:Lifeline-decomposedAs .

mms-property:postconditionFromBehavior a mms-ontology:UmlObjectProperty ;
	mms-ontology:cardinality "*"^^uml-model-dt:cardinalityRange ;
	mms-ontology:key "postconditionIds" ;
	rdfs:label "postconditionFromBehavior" ;
	rdfs:comment "A Constraint that is the postcondition of this Behavior. Based on the UML property 'Behavior-postcondition' which is described as: An optional set of Constraints specifying what is fulfilled after the execution of the Behavior is completed, if its precondition was fulfilled before its invocation."@en ;
	rdfs:domain uml-class:Behavior ;
	rdfs:range uml-class:Constraint ;
	mms-ontology:umlPropertySource uml-property:Behavior-postcondition .

mms-property:postconditionFromOperation a mms-ontology:UmlObjectProperty ;
	mms-ontology:cardinality "*"^^uml-model-dt:cardinalityRange ;
	mms-ontology:key "postconditionIds" ;
	rdfs:label "postconditionFromOperation" ;
	rdfs:comment "A Constraint that is the postcondition of this Operation. Based on the UML property 'Operation-postcondition' which is described as: An optional set of Constraints specifying the state of the system when the Operation is completed."@en ;
	rdfs:domain uml-class:Operation ;
	rdfs:range uml-class:Constraint ;
	mms-ontology:umlPropertySource uml-property:Operation-postcondition .

mms-property:isTestedFirst a mms-ontology:UmlDatatypeProperty ;
	mms-ontology:key "isTestedFirst" ;
	rdfs:label "isTestedFirst" ;
	rdfs:comment "If true, the test is performed before the first execution of the bodyPart. If false, the bodyPart is executed once before the test is performed."@en ;
	rdfs:domain uml-class:LoopNode ;
	rdfs:range xsd:boolean ;
	mms-ontology:umlPropertySource uml-property:LoopNode-isTestedFirst .

mms-property:isTestedFirstLoopNode a mms-ontology:UmlDatatypeProperty ;
	owl:equivalentProperty mms-property:isTestedFirst .

mms-property:mappingOpaqueExpression a mms-ontology:UmlObjectProperty ;
	mms-ontology:cardinality "1"^^uml-model-dt:cardinalityRange ;
	mms-ontology:key "mappingId" ;
	rdfs:label "mappingOpaqueExpression" ;
	rdfs:comment "The OpaqueExpression that is the mapping of this Abstraction. Based on the UML property 'Abstraction-mapping' which is described as: An OpaqueExpression that states the abstraction relationship between the supplier(s) and the client(s). In some cases, such as derivation, it is usually formal and unidirectional; in other cases, such as trace, it is usually informal and bidirectional. The mapping expression is optional and may be omitted if the precise relationship between the Elements is not specified."@en ;
	rdfs:domain uml-class:Abstraction ;
	rdfs:range uml-class:OpaqueExpression ;
	mms-ontology:umlPropertySource uml-property:Abstraction-mapping .

mms-property:owningInstanceInstanceSpecification a mms-ontology:UmlObjectProperty ;
	mms-ontology:cardinality "1"^^uml-model-dt:cardinalityRange ;
	mms-ontology:key "owningInstanceId" ;
	rdfs:label "owningInstanceInstanceSpecification" ;
	rdfs:comment "The InstanceSpecification that is the owningInstance of this Slot. Based on the UML property 'Slot-owningInstance' which is described as: The InstanceSpecification that owns this Slot."@en ;
	rdfs:domain uml-class:Slot ;
	rdfs:range uml-class:InstanceSpecification ;
	mms-ontology:umlPropertySource uml-property:Slot-owningInstance .

mms-property:submachineState a mms-ontology:UmlObjectProperty ;
	mms-ontology:cardinality "*"^^uml-model-dt:cardinalityRange ;
	mms-ontology:key "submachineStateIds" ;
	rdfs:label "submachineState" ;
	rdfs:comment "A State that belongs to this StateMachine. Based on the UML property 'StateMachine-submachineState' which is described as: References the submachine(s) in case of a submachine State. Multiple machines are referenced in case of a concurrent State."@en ;
	rdfs:domain uml-class:StateMachine ;
	rdfs:range uml-class:State ;
	mms-ontology:umlPropertySource uml-property:StateMachine-submachineState .

mms-property:generalMachineProtocolStateMachine a mms-ontology:UmlObjectProperty ;
	mms-ontology:cardinality "1"^^uml-model-dt:cardinalityRange ;
	mms-ontology:key "generalMachineId" ;
	rdfs:label "generalMachineProtocolStateMachine" ;
	rdfs:comment "The ProtocolStateMachine that is the generalMachine of this ProtocolConformance. Based on the UML property 'ProtocolConformance-generalMachine' which is described as: Specifies the ProtocolStateMachine to which the specific ProtocolStateMachine conforms."@en ;
	rdfs:domain uml-class:ProtocolConformance ;
	rdfs:range uml-class:ProtocolStateMachine ;
	mms-ontology:umlPropertySource uml-property:ProtocolConformance-generalMachine .

mms-property:extensionPoint a mms-ontology:UmlObjectProperty ;
	mms-ontology:cardinality "*"^^uml-model-dt:cardinalityRange ;
	mms-ontology:key "extensionPointIds" ;
	rdfs:label "extensionPoint" ;
	rdfs:comment "A ExtensionPoint that belongs to this UseCase. Based on the UML property 'UseCase-extensionPoint' which is described as: The ExtensionPoints owned by this UseCase."@en ;
	rdfs:domain uml-class:UseCase ;
	rdfs:range uml-class:ExtensionPoint ;
	mms-ontology:umlPropertySource uml-property:UseCase-extensionPoint .

mms-property:coveredBy a mms-ontology:UmlObjectProperty ;
	mms-ontology:cardinality "*"^^uml-model-dt:cardinalityRange ;
	mms-ontology:key "coveredByIds" ;
	rdfs:label "coveredBy" ;
	rdfs:comment "A InteractionFragment that is the coveredBy of this Lifeline. Based on the UML property 'Lifeline-coveredBy' which is described as: References the InteractionFragments in which this Lifeline takes part."@en ;
	rdfs:domain uml-class:Lifeline ;
	rdfs:range uml-class:InteractionFragment ;
	mms-ontology:umlPropertySource uml-property:Lifeline-coveredBy .

mms-property:deferrableTrigger a mms-ontology:UmlObjectProperty ;
	mms-ontology:cardinality "*"^^uml-model-dt:cardinalityRange ;
	mms-ontology:key "deferrableTriggerIds" ;
	rdfs:label "deferrableTrigger" ;
	rdfs:comment "A Trigger that belongs to this State. Based on the UML property 'State-deferrableTrigger' which is described as: A list of Triggers that are candidates to be retained by the StateMachine if they trigger no Transitions out of the State (not consumed). A deferred Trigger is retained until the StateMachine reaches a State configuration where it is no longer deferred."@en ;
	rdfs:domain uml-class:State ;
	rdfs:range uml-class:Trigger ;
	mms-ontology:umlPropertySource uml-property:State-deferrableTrigger .

mms-property:outputValue a mms-ontology:UmlObjectProperty ;
	mms-ontology:cardinality "*"^^uml-model-dt:cardinalityRange ;
	mms-ontology:key "outputValueIds" ;
	rdfs:label "outputValue" ;
	rdfs:comment "A OutputPin that is the outputValue of this OpaqueAction. Based on the UML property 'OpaqueAction-outputValue' which is described as: The OutputPins on which the OpaqueAction provides outputs."@en ;
	rdfs:domain uml-class:OpaqueAction ;
	rdfs:range uml-class:OutputPin ;
	mms-ontology:umlPropertySource uml-property:OpaqueAction-outputValue .

mms-property:guardInteractionConstraint a mms-ontology:UmlObjectProperty ;
	mms-ontology:cardinality "1"^^uml-model-dt:cardinalityRange ;
	mms-ontology:key "guardId" ;
	rdfs:label "guardInteractionConstraint" ;
	rdfs:comment "The InteractionConstraint that is the guard of this InteractionOperand. Based on the UML property 'InteractionOperand-guard' which is described as: Constraint of the operand."@en ;
	rdfs:domain uml-class:InteractionOperand ;
	rdfs:range uml-class:InteractionConstraint ;
	mms-ontology:umlPropertySource uml-property:InteractionOperand-guard .

mms-property:guardValueSpecification a mms-ontology:UmlObjectProperty ;
	mms-ontology:cardinality "1"^^uml-model-dt:cardinalityRange ;
	mms-ontology:key "guardId" ;
	rdfs:label "guardValueSpecification" ;
	rdfs:comment "The ValueSpecification that is the guard of this ActivityEdge. Based on the UML property 'ActivityEdge-guard' which is described as: A ValueSpecification that is evaluated to determine if a token can traverse the ActivityEdge. If an ActivityEdge has no guard, then there is no restriction on tokens traversing the edge."@en ;
	rdfs:domain uml-class:ActivityEdge ;
	rdfs:range uml-class:ValueSpecification ;
	mms-ontology:umlPropertySource uml-property:ActivityEdge-guard .

mms-property:guardConstraint a mms-ontology:UmlObjectProperty ;
	mms-ontology:cardinality "1"^^uml-model-dt:cardinalityRange ;
	mms-ontology:key "guardId" ;
	rdfs:label "guardConstraint" ;
	rdfs:comment "The Constraint that is the guard of this Transition. Based on the UML property 'Transition-guard' which is described as: A guard is a Constraint that provides a fine-grained control over the firing of the Transition. The guard is evaluated when an Event occurrence is dispatched by the StateMachine. If the guard is true at that time, the Transition may be enabled, otherwise, it is disabled. Guards should be pure expressions without side effects. Guard expressions with side effects are ill formed."@en ;
	rdfs:domain uml-class:Transition ;
	rdfs:range uml-class:Constraint ;
	mms-ontology:umlPropertySource uml-property:Transition-guard .

mms-property:deployedArtifact a mms-ontology:UmlObjectProperty ;
	mms-ontology:cardinality "*"^^uml-model-dt:cardinalityRange ;
	mms-ontology:key "deployedArtifactIds" ;
	rdfs:label "deployedArtifact" ;
	rdfs:comment "A DeployedArtifact that belongs to this Deployment. Based on the UML property 'Deployment-deployedArtifact' which is described as: The Artifacts that are deployed onto a Node. This association specializes the supplier association."@en ;
	rdfs:domain uml-class:Deployment ;
	rdfs:range uml-class:DeployedArtifact ;
	mms-ontology:umlPropertySource uml-property:Deployment-deployedArtifact .

mms-property:realizingClassifier a mms-ontology:UmlObjectProperty ;
	mms-ontology:cardinality "*"^^uml-model-dt:cardinalityRange ;
	mms-ontology:key "realizingClassifierIds" ;
	rdfs:label "realizingClassifier" ;
	rdfs:comment "A Classifier that belongs to this ComponentRealization. Based on the UML property 'ComponentRealization-realizingClassifier' which is described as: The Classifiers that are involved in the implementation of the Component that owns this Realization."@en ;
	rdfs:domain uml-class:ComponentRealization ;
	rdfs:range uml-class:Classifier ;
	mms-ontology:umlPropertySource uml-property:ComponentRealization-realizingClassifier .

mms-property:redefinedElement a mms-ontology:UmlObjectProperty ;
	mms-ontology:cardinality "*"^^uml-model-dt:cardinalityRange ;
	mms-ontology:key "redefinedElementIds" ;
	rdfs:label "redefinedElement" ;
	rdfs:comment "A RedefinableElement that is the redefinedElement of this RedefinableElement. Based on the UML property 'RedefinableElement-redefinedElement' which is described as: The RedefinableElement that is being redefined by this element."@en ;
	rdfs:domain uml-class:RedefinableElement ;
	rdfs:range uml-class:RedefinableElement ;
	mms-ontology:umlPropertySource uml-property:RedefinableElement-redefinedElement .

mms-property:deployedElement a mms-ontology:UmlObjectProperty ;
	mms-ontology:cardinality "*"^^uml-model-dt:cardinalityRange ;
	mms-ontology:key "deployedElementIds" ;
	rdfs:label "deployedElement" ;
	rdfs:comment "A PackageableElement that is the deployedElement of this DeploymentTarget. Based on the UML property 'DeploymentTarget-deployedElement' which is described as: The set of elements that are manifested in an Artifact that is involved in Deployment to a DeploymentTarget."@en ;
	rdfs:domain uml-class:DeploymentTarget ;
	rdfs:range uml-class:PackageableElement ;
	mms-ontology:umlPropertySource uml-property:DeploymentTarget-deployedElement .

mms-property:testFromClause a mms-ontology:UmlObjectProperty ;
	mms-ontology:cardinality "*"^^uml-model-dt:cardinalityRange ;
	mms-ontology:key "testIds" ;
	rdfs:label "testFromClause" ;
	rdfs:comment "A ExecutableNode that is the test of this Clause. Based on the UML property 'Clause-test' which is described as: The set of ExecutableNodes that are executed in order to provide a test result for the Clause."@en ;
	rdfs:domain uml-class:Clause ;
	rdfs:range uml-class:ExecutableNode ;
	mms-ontology:umlPropertySource uml-property:Clause-test .

mms-property:testFromLoopNode a mms-ontology:UmlObjectProperty ;
	mms-ontology:cardinality "*"^^uml-model-dt:cardinalityRange ;
	mms-ontology:key "testIds" ;
	rdfs:label "testFromLoopNode" ;
	rdfs:comment "A ExecutableNode that is the test of this LoopNode. Based on the UML property 'LoopNode-test' which is described as: The set of ExecutableNodes executed in order to provide the test result for the loop."@en ;
	rdfs:domain uml-class:LoopNode ;
	rdfs:range uml-class:ExecutableNode ;
	mms-ontology:umlPropertySource uml-property:LoopNode-test .

mms-property:doActivityBehavior a mms-ontology:UmlObjectProperty ;
	mms-ontology:cardinality "1"^^uml-model-dt:cardinalityRange ;
	mms-ontology:key "doActivityId" ;
	rdfs:label "doActivityBehavior" ;
	rdfs:comment "The Behavior that is the doActivity of this State. Based on the UML property 'State-doActivity' which is described as: An optional Behavior that is executed while being in the State. The execution starts when this State is entered, and ceases either by itself when done, or when the State is exited, whichever comes first."@en ;
	rdfs:domain uml-class:State ;
	rdfs:range uml-class:Behavior ;
	mms-ontology:umlPropertySource uml-property:State-doActivity .

mms-property:newClassifier a mms-ontology:UmlObjectProperty ;
	mms-ontology:cardinality "*"^^uml-model-dt:cardinalityRange ;
	mms-ontology:key "newClassifierIds" ;
	rdfs:label "newClassifier" ;
	rdfs:comment "A Classifier that belongs to this ReclassifyObjectAction. Based on the UML property 'ReclassifyObjectAction-newClassifier' which is described as: A set of Classifiers to be added to the Classifiers of the given object."@en ;
	rdfs:domain uml-class:ReclassifyObjectAction ;
	rdfs:range uml-class:Classifier ;
	mms-ontology:umlPropertySource uml-property:ReclassifyObjectAction-newClassifier .

mms-property:replyToCallTrigger a mms-ontology:UmlObjectProperty ;
	mms-ontology:cardinality "1"^^uml-model-dt:cardinalityRange ;
	mms-ontology:key "replyToCallId" ;
	rdfs:label "replyToCallTrigger" ;
	rdfs:comment "The Trigger that is the replyToCall of this ReplyAction. Based on the UML property 'ReplyAction-replyToCall' which is described as: The Trigger specifying the Operation whose call is being replied to."@en ;
	rdfs:domain uml-class:ReplyAction ;
	rdfs:range uml-class:Trigger ;
	mms-ontology:umlPropertySource uml-property:ReplyAction-replyToCall .

mms-property:isDestroyDuplicates a mms-ontology:UmlDatatypeProperty ;
	mms-ontology:key "isDestroyDuplicates" ;
	rdfs:label "isDestroyDuplicates" ;
	rdfs:comment "Specifies whether to destroy duplicates of the value in nonunique Association ends."@en ;
	rdfs:domain uml-class:LinkEndDestructionData ;
	rdfs:range xsd:boolean ;
	mms-ontology:umlPropertySource uml-property:LinkEndDestructionData-isDestroyDuplicates .

mms-property:isDestroyDuplicatesLinkEndDestructionData a mms-ontology:UmlDatatypeProperty ;
	owl:equivalentProperty mms-property:isDestroyDuplicates .

mms-property:isControl a mms-ontology:UmlDatatypeProperty ;
	mms-ontology:key "isControl" ;
	rdfs:label "isControl" ;
	rdfs:comment "Indicates whether the Pin provides data to the Action or just controls how the Action executes."@en ;
	rdfs:domain uml-class:Pin ;
	rdfs:range xsd:boolean ;
	mms-ontology:umlPropertySource uml-property:Pin-isControl .

mms-property:isControlPin a mms-ontology:UmlDatatypeProperty ;
	owl:equivalentProperty mms-property:isControl .

mms-property:input a mms-ontology:UmlObjectProperty ;
	mms-ontology:cardinality "*"^^uml-model-dt:cardinalityRange ;
	mms-ontology:key "inputIds" ;
	rdfs:label "input" ;
	rdfs:comment "A InputPin that is the input of this Action. Based on the UML property 'Action-input' which is described as: The ordered set of InputPins representing the inputs to the Action."@en ;
	rdfs:domain uml-class:Action ;
	rdfs:range uml-class:InputPin ;
	mms-ontology:umlPropertySource uml-property:Action-input .

mms-property:transition a mms-ontology:UmlObjectProperty ;
	mms-ontology:cardinality "*"^^uml-model-dt:cardinalityRange ;
	mms-ontology:key "transitionIds" ;
	rdfs:label "transition" ;
	rdfs:comment "A Transition that belongs to this Region. Based on the UML property 'Region-transition' which is described as: The set of Transitions owned by the Region."@en ;
	rdfs:domain uml-class:Region ;
	rdfs:range uml-class:Transition ;
	mms-ontology:umlPropertySource uml-property:Region-transition .

mms-property:isDerivedUnion a mms-ontology:UmlDatatypeProperty ;
	mms-ontology:key "isDerivedUnion" ;
	rdfs:label "isDerivedUnion" ;
	rdfs:comment "Specifies whether the property is derived as the union of all of the Properties that are constrained to subset it."@en ;
	rdfs:domain uml-class:Property ;
	rdfs:range xsd:boolean ;
	mms-ontology:umlPropertySource uml-property:Property-isDerivedUnion .

mms-property:isDerivedUnionProperty a mms-ontology:UmlDatatypeProperty ;
	owl:equivalentProperty mms-property:isDerivedUnion .

mms-property:isMultireceive a mms-ontology:UmlDatatypeProperty ;
	mms-ontology:key "isMultireceive" ;
	rdfs:label "isMultireceive" ;
	rdfs:comment "Indicates whether the objects in the ObjectFlow are gathered from respondents to multicasting."@en ;
	rdfs:domain uml-class:ObjectFlow ;
	rdfs:range xsd:boolean ;
	mms-ontology:umlPropertySource uml-property:ObjectFlow-isMultireceive .

mms-property:isMultireceiveObjectFlow a mms-ontology:UmlDatatypeProperty ;
	owl:equivalentProperty mms-property:isMultireceive .

mms-property:ownedParameteredElementParameterableElement a mms-ontology:UmlObjectProperty ;
	mms-ontology:cardinality "1"^^uml-model-dt:cardinalityRange ;
	mms-ontology:key "ownedParameteredElementId" ;
	rdfs:label "ownedParameteredElementParameterableElement" ;
	rdfs:comment "The ParameterableElement that is the ownedParameteredElement of this TemplateParameter. Based on the UML property 'TemplateParameter-ownedParameteredElement' which is described as: The ParameterableElement that is owned by this TemplateParameter for the purpose of exposing it as the parameteredElement."@en ;
	rdfs:domain uml-class:TemplateParameter ;
	rdfs:range uml-class:ParameterableElement ;
	mms-ontology:umlPropertySource uml-property:TemplateParameter-ownedParameteredElement .

mms-property:selectorValueSpecification a mms-ontology:UmlObjectProperty ;
	mms-ontology:cardinality "1"^^uml-model-dt:cardinalityRange ;
	mms-ontology:key "selectorId" ;
	rdfs:label "selectorValueSpecification" ;
	rdfs:comment "The ValueSpecification that is the selector of this Lifeline. Based on the UML property 'Lifeline-selector' which is described as: If the referenced ConnectableElement is multivalued, then this specifies the specific individual part within that set."@en ;
	rdfs:domain uml-class:Lifeline ;
	rdfs:range uml-class:ValueSpecification ;
	mms-ontology:umlPropertySource uml-property:Lifeline-selector .

mms-property:generalOrdering a mms-ontology:UmlObjectProperty ;
	mms-ontology:cardinality "*"^^uml-model-dt:cardinalityRange ;
	mms-ontology:key "generalOrderingIds" ;
	rdfs:label "generalOrdering" ;
	rdfs:comment "A GeneralOrdering that belongs to this InteractionFragment. Based on the UML property 'InteractionFragment-generalOrdering' which is described as: The general ordering relationships contained in this fragment."@en ;
	rdfs:domain uml-class:InteractionFragment ;
	rdfs:range uml-class:GeneralOrdering ;
	mms-ontology:umlPropertySource uml-property:InteractionFragment-generalOrdering .

mms-property:exitPseudostate a mms-ontology:UmlObjectProperty ;
	mms-ontology:cardinality "*"^^uml-model-dt:cardinalityRange ;
	mms-ontology:key "exitIds" ;
	rdfs:label "exitPseudostate" ;
	rdfs:comment "A Pseudostate that is the exit of this ConnectionPointReference. Based on the UML property 'ConnectionPointReference-exit' which is described as: The exitPoints kind Pseudostates corresponding to this connection point."@en ;
	rdfs:domain uml-class:ConnectionPointReference ;
	rdfs:range uml-class:Pseudostate ;
	mms-ontology:umlPropertySource uml-property:ConnectionPointReference-exit .

mms-property:exitBehavior a mms-ontology:UmlObjectProperty ;
	mms-ontology:cardinality "1"^^uml-model-dt:cardinalityRange ;
	mms-ontology:key "exitId" ;
	rdfs:label "exitBehavior" ;
	rdfs:comment "The Behavior that is the exit of this State. Based on the UML property 'State-exit' which is described as: An optional Behavior that is executed whenever this State is exited regardless of which Transition was taken out of the State. If defined, exit Behaviors are always executed to completion only after all internal and transition Behaviors have completed execution."@en ;
	rdfs:domain uml-class:State ;
	rdfs:range uml-class:Behavior ;
	mms-ontology:umlPropertySource uml-property:State-exit .

mms-property:isRemoveDuplicatesRemoveStructuralFeatureValueAction a mms-ontology:UmlDatatypeProperty ;
	mms-ontology:key "isRemoveDuplicates" ;
	rdfs:label "isRemoveDuplicatesRemoveStructuralFeatureValueAction" ;
	rdfs:comment "Specifies whether to remove duplicates of the value in nonunique StructuralFeatures."@en ;
	rdfs:domain uml-class:RemoveStructuralFeatureValueAction ;
	rdfs:range xsd:boolean ;
	mms-ontology:umlPropertySource uml-property:RemoveStructuralFeatureValueAction-isRemoveDuplicates .

mms-property:isRemoveDuplicatesRemoveVariableValueAction a mms-ontology:UmlDatatypeProperty ;
	mms-ontology:key "isRemoveDuplicates" ;
	rdfs:label "isRemoveDuplicatesRemoveVariableValueAction" ;
	rdfs:comment "Specifies whether to remove duplicates of the value in nonunique Variables."@en ;
	rdfs:domain uml-class:RemoveVariableValueAction ;
	rdfs:range xsd:boolean ;
	mms-ontology:umlPropertySource uml-property:RemoveVariableValueAction-isRemoveDuplicates .

mms-property:connector a mms-ontology:UmlObjectProperty ;
	mms-ontology:cardinality "1"^^uml-model-dt:cardinalityRange ;
	mms-ontology:key "connectorId" ;
	rdfs:label "connector" ;
	rdfs:comment "The Connector that belongs to this Message. Based on the UML property 'Message-connector' which is described as: The Connector on which this Message is sent."@en ;
	rdfs:domain uml-class:Message ;
	rdfs:range uml-class:Connector ;
	mms-ontology:umlPropertySource uml-property:Message-connector .

mms-property:protectedNodeExecutableNode a mms-ontology:UmlObjectProperty ;
	mms-ontology:cardinality "1"^^uml-model-dt:cardinalityRange ;
	mms-ontology:key "protectedNodeId" ;
	rdfs:label "protectedNodeExecutableNode" ;
	rdfs:comment "The ExecutableNode that is the protectedNode of this ExceptionHandler. Based on the UML property 'ExceptionHandler-protectedNode' which is described as: The ExecutableNode protected by the ExceptionHandler. If an exception propagates out of the protectedNode and has a type matching one of the exceptionTypes, then it is caught by this ExceptionHandler."@en ;
	rdfs:domain uml-class:ExceptionHandler ;
	rdfs:range uml-class:ExecutableNode ;
	mms-ontology:umlPropertySource uml-property:ExceptionHandler-protectedNode .

mms-property:toAfter a mms-ontology:UmlObjectProperty ;
	mms-ontology:cardinality "*"^^uml-model-dt:cardinalityRange ;
	mms-ontology:key "toAfterIds" ;
	rdfs:label "toAfter" ;
	rdfs:comment "A GeneralOrdering that is the toAfter of this OccurrenceSpecification. Based on the UML property 'OccurrenceSpecification-toAfter' which is described as: References the GeneralOrderings that specify EventOcurrences that must occur after this OccurrenceSpecification."@en ;
	rdfs:domain uml-class:OccurrenceSpecification ;
	rdfs:range uml-class:GeneralOrdering ;
	mms-ontology:umlPropertySource uml-property:OccurrenceSpecification-toAfter .

mms-property:packageMerge a mms-ontology:UmlObjectProperty ;
	mms-ontology:cardinality "*"^^uml-model-dt:cardinalityRange ;
	mms-ontology:key "packageMergeIds" ;
	rdfs:label "packageMerge" ;
	rdfs:comment "A PackageMerge that belongs to this Package. Based on the UML property 'Package-packageMerge' which is described as: References the PackageMerges that are owned by this Package."@en ;
	rdfs:domain uml-class:Package ;
	rdfs:range uml-class:PackageMerge ;
	mms-ontology:umlPropertySource uml-property:Package-packageMerge .

mms-property:invariantConstraint a mms-ontology:UmlObjectProperty ;
	mms-ontology:cardinality "1"^^uml-model-dt:cardinalityRange ;
	mms-ontology:key "invariantId" ;
	rdfs:label "invariantConstraint" ;
	rdfs:comment "The Constraint that is the invariant of this StateInvariant. Based on the UML property 'StateInvariant-invariant' which is described as: A Constraint that should hold at runtime for this StateInvariant."@en ;
	rdfs:domain uml-class:StateInvariant ;
	rdfs:range uml-class:Constraint ;
	mms-ontology:umlPropertySource uml-property:StateInvariant-invariant .

mms-property:joinSpecValueSpecification a mms-ontology:UmlObjectProperty ;
	mms-ontology:cardinality "1"^^uml-model-dt:cardinalityRange ;
	mms-ontology:key "joinSpecId" ;
	rdfs:label "joinSpecValueSpecification" ;
	rdfs:comment "The ValueSpecification that is the joinSpec of this JoinNode. Based on the UML property 'JoinNode-joinSpec' which is described as: A ValueSpecification giving the condition under which the JoinNode will offer a token on its outgoing ActivityEdge. If no joinSpec is specified, then the JoinNode will offer an outgoing token if tokens are offered on all of its incoming ActivityEdges (an &#34;and&#34; condition)."@en ;
	rdfs:domain uml-class:JoinNode ;
	rdfs:range uml-class:ValueSpecification ;
	mms-ontology:umlPropertySource uml-property:JoinNode-joinSpec .

mms-property:configuration a mms-ontology:UmlObjectProperty ;
	mms-ontology:cardinality "*"^^uml-model-dt:cardinalityRange ;
	mms-ontology:key "configurationIds" ;
	rdfs:label "configuration" ;
	rdfs:comment "A DeploymentSpecification that is the configuration of this Deployment. Based on the UML property 'Deployment-configuration' which is described as: The specification of properties that parameterize the deployment and execution of one or more Artifacts."@en ;
	rdfs:domain uml-class:Deployment ;
	rdfs:range uml-class:DeploymentSpecification ;
	mms-ontology:umlPropertySource uml-property:Deployment-configuration .

mms-property:redefinedVertex a mms-ontology:UmlObjectProperty ;
	mms-ontology:cardinality "1"^^uml-model-dt:cardinalityRange ;
	mms-ontology:key "redefinedVertexId" ;
	rdfs:label "redefinedVertex" ;
	rdfs:comment "The Vertex that belongs to this Vertex. Based on the UML property 'State-redefinedState' which is described as: The Vertex of which this Vertex is a redefinition."@en ;
	rdfs:domain uml-class:Vertex ;
	rdfs:range uml-class:Vertex ;
	mms-ontology:umlPropertySource uml-property:State-redefinedState .

mms-property:ownedActualParameterableElement a mms-ontology:UmlObjectProperty ;
	mms-ontology:cardinality "1"^^uml-model-dt:cardinalityRange ;
	mms-ontology:key "ownedActualId" ;
	rdfs:label "ownedActualParameterableElement" ;
	rdfs:comment "The ParameterableElement that is the ownedActual of this TemplateParameterSubstitution. Based on the UML property 'TemplateParameterSubstitution-ownedActual' which is described as: The ParameterableElement that is owned by this TemplateParameterSubstitution as its actual parameter."@en ;
	rdfs:domain uml-class:TemplateParameterSubstitution ;
	rdfs:range uml-class:ParameterableElement ;
	mms-ontology:umlPropertySource uml-property:TemplateParameterSubstitution-ownedActual .

mms-property:ownedEndExtensionEnd a mms-ontology:UmlObjectProperty ;
	mms-ontology:cardinality "1"^^uml-model-dt:cardinalityRange ;
	mms-ontology:key "ownedEndId" ;
	rdfs:label "ownedEndExtensionEnd" ;
	rdfs:comment "The ExtensionEnd that is the ownedEnd of this Extension. Based on the UML property 'Extension-ownedEnd' which is described as: References the end of the extension that is typed by a Stereotype."@en ;
	rdfs:domain uml-class:Extension ;
	rdfs:range uml-class:ExtensionEnd ;
	mms-ontology:umlPropertySource uml-property:Extension-ownedEnd .

mms-property:ownedEndProperty a mms-ontology:UmlObjectProperty ;
	mms-ontology:cardinality "*"^^uml-model-dt:cardinalityRange ;
	mms-ontology:key "ownedEndIds" ;
	rdfs:label "ownedEndProperty" ;
	rdfs:comment "A Property that is the ownedEnd of this Association. Based on the UML property 'Association-ownedEnd' which is described as: The ends that are owned by the Association itself."@en ;
	rdfs:domain uml-class:Association ;
	rdfs:range uml-class:Property ;
	mms-ontology:umlPropertySource uml-property:Association-ownedEnd .

mms-property:templateBindingFromTemplateParameterSubstitution a mms-ontology:UmlObjectProperty ;
	mms-ontology:cardinality "1"^^uml-model-dt:cardinalityRange ;
	mms-ontology:key "templateBindingId" ;
	rdfs:label "templateBindingFromTemplateParameterSubstitution" ;
	rdfs:comment "The TemplateBinding that belongs to this TemplateParameterSubstitution. Based on the UML property 'TemplateParameterSubstitution-templateBinding' which is described as: The TemplateBinding that owns this TemplateParameterSubstitution."@en ;
	rdfs:domain uml-class:TemplateParameterSubstitution ;
	rdfs:range uml-class:TemplateBinding ;
	mms-ontology:umlPropertySource uml-property:TemplateParameterSubstitution-templateBinding .

mms-property:templateBindingFromTemplateableElement a mms-ontology:UmlObjectProperty ;
	mms-ontology:cardinality "*"^^uml-model-dt:cardinalityRange ;
	mms-ontology:key "templateBindingIds" ;
	rdfs:label "templateBindingFromTemplateableElement" ;
	rdfs:comment "A TemplateBinding that belongs to this TemplateableElement. Based on the UML property 'TemplateableElement-templateBinding' which is described as: The optional TemplateBindings from this TemplateableElement to one or more templates."@en ;
	rdfs:domain uml-class:TemplateableElement ;
	rdfs:range uml-class:TemplateBinding ;
	mms-ontology:umlPropertySource uml-property:TemplateableElement-templateBinding .

mms-property:ownedStereotype a mms-ontology:UmlObjectProperty ;
	mms-ontology:cardinality "*"^^uml-model-dt:cardinalityRange ;
	mms-ontology:key "ownedStereotypeIds" ;
	rdfs:label "ownedStereotype" ;
	rdfs:comment "A Stereotype that belongs to this Package. Based on the UML property 'Package-ownedStereotype' which is described as: References the Stereotypes that are owned by the Package."@en ;
	rdfs:domain uml-class:Package ;
	rdfs:range uml-class:Stereotype ;
	mms-ontology:umlPropertySource uml-property:Package-ownedStereotype .

mms-property:isMulticast a mms-ontology:UmlDatatypeProperty ;
	mms-ontology:key "isMulticast" ;
	rdfs:label "isMulticast" ;
	rdfs:comment "Indicates whether the objects in the ObjectFlow are passed by multicasting."@en ;
	rdfs:domain uml-class:ObjectFlow ;
	rdfs:range xsd:boolean ;
	mms-ontology:umlPropertySource uml-property:ObjectFlow-isMulticast .

mms-property:isMulticastObjectFlow a mms-ontology:UmlDatatypeProperty ;
	owl:equivalentProperty mms-property:isMulticast .

mms-property:scopeStructuredActivityNode a mms-ontology:UmlObjectProperty ;
	mms-ontology:cardinality "1"^^uml-model-dt:cardinalityRange ;
	mms-ontology:key "scopeId" ;
	rdfs:label "scopeStructuredActivityNode" ;
	rdfs:comment "The StructuredActivityNode that is the scope of this Variable. Based on the UML property 'Variable-scope' which is described as: A StructuredActivityNode that owns the Variable."@en ;
	rdfs:domain uml-class:Variable ;
	rdfs:range uml-class:StructuredActivityNode ;
	mms-ontology:umlPropertySource uml-property:Variable-scope .

mms-property:ownedDefaultParameterableElement a mms-ontology:UmlObjectProperty ;
	mms-ontology:cardinality "1"^^uml-model-dt:cardinalityRange ;
	mms-ontology:key "ownedDefaultId" ;
	rdfs:label "ownedDefaultParameterableElement" ;
	rdfs:comment "The ParameterableElement that is the ownedDefault of this TemplateParameter. Based on the UML property 'TemplateParameter-ownedDefault' which is described as: The ParameterableElement that is owned by this TemplateParameter for the purpose of providing a default."@en ;
	rdfs:domain uml-class:TemplateParameter ;
	rdfs:range uml-class:ParameterableElement ;
	mms-ontology:umlPropertySource uml-property:TemplateParameter-ownedDefault .

mms-property:ownedUseCase a mms-ontology:UmlObjectProperty ;
	mms-ontology:cardinality "*"^^uml-model-dt:cardinalityRange ;
	mms-ontology:key "ownedUseCaseIds" ;
	rdfs:label "ownedUseCase" ;
	rdfs:comment "A UseCase that belongs to this Classifier. Based on the UML property 'Classifier-ownedUseCase' which is described as: The UseCases owned by this classifier."@en ;
	rdfs:domain uml-class:Classifier ;
	rdfs:range uml-class:UseCase ;
	mms-ontology:umlPropertySource uml-property:Classifier-ownedUseCase .

mms-property:upperBoundValueSpecification a mms-ontology:UmlObjectProperty ;
	mms-ontology:cardinality "1"^^uml-model-dt:cardinalityRange ;
	mms-ontology:key "upperBoundId" ;
	rdfs:label "upperBoundValueSpecification" ;
	rdfs:comment "The ValueSpecification that is the upperBound of this ObjectNode. Based on the UML property 'ObjectNode-upperBound' which is described as: The maximum number of tokens that may be held by this ObjectNode. Tokens cannot flow into the ObjectNode if the upperBound is reached. If no upperBound is specified, then there is no limit on how many tokens the ObjectNode can hold."@en ;
	rdfs:domain uml-class:ObjectNode ;
	rdfs:range uml-class:ValueSpecification ;
	mms-ontology:umlPropertySource uml-property:ObjectNode-upperBound .

mms-property:ownedComment a mms-ontology:UmlObjectProperty ;
	mms-ontology:cardinality "*"^^uml-model-dt:cardinalityRange ;
	mms-ontology:key "ownedCommentIds" ;
	rdfs:label "ownedComment" ;
	rdfs:comment "A Comment that belongs to this Element. Based on the UML property 'Element-ownedComment' which is described as: The Comments owned by this Element."@en ;
	rdfs:domain uml-class:Element ;
	rdfs:range uml-class:Comment ;
	mms-ontology:umlPropertySource uml-property:Element-ownedComment .

mms-property:isDestroyLinks a mms-ontology:UmlDatatypeProperty ;
	mms-ontology:key "isDestroyLinks" ;
	rdfs:label "isDestroyLinks" ;
	rdfs:comment "Specifies whether links in which the object participates are destroyed along with the object."@en ;
	rdfs:domain uml-class:DestroyObjectAction ;
	rdfs:range xsd:boolean ;
	mms-ontology:umlPropertySource uml-property:DestroyObjectAction-isDestroyLinks .

mms-property:isDestroyLinksDestroyObjectAction a mms-ontology:UmlDatatypeProperty ;
	owl:equivalentProperty mms-property:isDestroyLinks .

mms-property:subExpression a mms-ontology:UmlObjectProperty ;
	mms-ontology:cardinality "*"^^uml-model-dt:cardinalityRange ;
	mms-ontology:key "subExpressionIds" ;
	rdfs:label "subExpression" ;
	rdfs:comment "A StringExpression that is the subExpression of this StringExpression. Based on the UML property 'StringExpression-subExpression' which is described as: The StringExpressions that constitute this StringExpression."@en ;
	rdfs:domain uml-class:StringExpression ;
	rdfs:range uml-class:StringExpression ;
	mms-ontology:umlPropertySource uml-property:StringExpression-subExpression .

mms-property:isSynchronous a mms-ontology:UmlDatatypeProperty ;
	mms-ontology:key "isSynchronous" ;
	rdfs:label "isSynchronous" ;
	rdfs:comment "If true, the call is synchronous and the caller waits for completion of the invoked Behavior. If false, the call is asynchronous and the caller proceeds immediately and cannot receive return values."@en ;
	rdfs:domain uml-class:CallAction ;
	rdfs:range xsd:boolean ;
	mms-ontology:umlPropertySource uml-property:CallAction-isSynchronous .

mms-property:isSynchronousCallAction a mms-ontology:UmlDatatypeProperty ;
	owl:equivalentProperty mms-property:isSynchronous .

mms-property:templateTemplateableElement a mms-ontology:UmlObjectProperty ;
	mms-ontology:cardinality "1"^^uml-model-dt:cardinalityRange ;
	mms-ontology:key "templateId" ;
	rdfs:label "templateTemplateableElement" ;
	rdfs:comment "The TemplateableElement that is the template of this TemplateSignature. Based on the UML property 'TemplateSignature-template' which is described as: The TemplateableElement that owns this TemplateSignature."@en ;
	rdfs:domain uml-class:TemplateSignature ;
	rdfs:range uml-class:TemplateableElement ;
	mms-ontology:umlPropertySource uml-property:TemplateSignature-template .

mms-property:realizationRelationship a mms-ontology:UmlObjectProperty ;
	mms-ontology:cardinality "*"^^uml-model-dt:cardinalityRange ;
	mms-ontology:key "realizationIds" ;
	rdfs:label "realizationRelationship" ;
	rdfs:comment "A Relationship that is the realization of this InformationFlow. Based on the UML property 'InformationFlow-realization' which is described as: Determines which Relationship will realize the specified flow."@en ;
	rdfs:domain uml-class:InformationFlow ;
	rdfs:range uml-class:Relationship ;
	mms-ontology:umlPropertySource uml-property:InformationFlow-realization .

mms-property:realizationComponentRealization a mms-ontology:UmlObjectProperty ;
	mms-ontology:cardinality "*"^^uml-model-dt:cardinalityRange ;
	mms-ontology:key "realizationIds" ;
	rdfs:label "realizationComponentRealization" ;
	rdfs:comment "A ComponentRealization that is the realization of this Component. Based on the UML property 'Component-realization' which is described as: The set of Realizations owned by the Component. Realizations reference the Classifiers of which the Component is an abstraction; i.e., that realize its behavior."@en ;
	rdfs:domain uml-class:Component ;
	rdfs:range uml-class:ComponentRealization ;
	mms-ontology:umlPropertySource uml-property:Component-realization .

mms-property:extendedRegion a mms-ontology:UmlObjectProperty ;
	mms-ontology:cardinality "1"^^uml-model-dt:cardinalityRange ;
	mms-ontology:key "extendedRegionId" ;
	rdfs:label "extendedRegion" ;
	rdfs:comment "The Region that belongs to this Region. Based on the UML property 'Region-extendedRegion' which is described as: The region of which this region is an extension."@en ;
	rdfs:domain uml-class:Region ;
	rdfs:range uml-class:Region ;
	mms-ontology:umlPropertySource uml-property:Region-extendedRegion .

mms-property:slot a mms-ontology:UmlObjectProperty ;
	mms-ontology:cardinality "*"^^uml-model-dt:cardinalityRange ;
	mms-ontology:key "slotIds" ;
	rdfs:label "slot" ;
	rdfs:comment "A Slot that belongs to this InstanceSpecification. Based on the UML property 'InstanceSpecification-slot' which is described as: A Slot giving the value or values of a StructuralFeature of the instance. An InstanceSpecification can have one Slot per StructuralFeature of its Classifiers, including inherited features. It is not necessary to model a Slot for every StructuralFeature, in which case the InstanceSpecification is a partial description."@en ;
	rdfs:domain uml-class:InstanceSpecification ;
	rdfs:range uml-class:Slot ;
	mms-ontology:umlPropertySource uml-property:InstanceSpecification-slot .

mms-property:isSubmachineState a mms-ontology:UmlDatatypeProperty ;
	mms-ontology:key "isSubmachineState" ;
	rdfs:label "isSubmachineState" ;
	rdfs:comment "A State with isSubmachineState=true is said to be a submachine State Such a State refers to another StateMachine(submachine)."@en ;
	rdfs:domain uml-class:State ;
	rdfs:range xsd:boolean ;
	mms-ontology:umlPropertySource uml-property:State-isSubmachineState .

mms-property:isSubmachineStateState a mms-ontology:UmlDatatypeProperty ;
	owl:equivalentProperty mms-property:isSubmachineState .

mms-property:outgoingActivityEdge a mms-ontology:UmlObjectProperty ;
	mms-ontology:cardinality "*"^^uml-model-dt:cardinalityRange ;
	mms-ontology:key "outgoingIds" ;
	rdfs:label "outgoingActivityEdge" ;
	rdfs:comment "A ActivityEdge that is the outgoing of this ActivityNode. Based on the UML property 'ActivityNode-outgoing' which is described as: ActivityEdges that have the ActivityNode as their source."@en ;
	rdfs:domain uml-class:ActivityNode ;
	rdfs:range uml-class:ActivityEdge ;
	mms-ontology:umlPropertySource uml-property:ActivityNode-outgoing .

mms-property:outgoingTransition a mms-ontology:UmlObjectProperty ;
	mms-ontology:cardinality "*"^^uml-model-dt:cardinalityRange ;
	mms-ontology:key "outgoingIds" ;
	rdfs:label "outgoingTransition" ;
	rdfs:comment "A Transition that is the outgoing of this Vertex. Based on the UML property 'Vertex-outgoing' which is described as: Specifies the Transitions departing from this Vertex."@en ;
	rdfs:domain uml-class:Vertex ;
	rdfs:range uml-class:Transition ;
	mms-ontology:umlPropertySource uml-property:Vertex-outgoing .

mms-property:roleConnectableElementFromConnectorEnd a mms-ontology:UmlObjectProperty ;
	mms-ontology:cardinality "1"^^uml-model-dt:cardinalityRange ;
	mms-ontology:key "roleId" ;
	rdfs:label "roleConnectableElementFromConnectorEnd" ;
	rdfs:comment "The ConnectableElement that is the role of this ConnectorEnd. Based on the UML property 'ConnectorEnd-role' which is described as: The ConnectableElement attached at this ConnectorEnd. When an instance of the containing Classifier is created, a link may (depending on the multiplicities) be created to an instance of the Classifier that types this ConnectableElement."@en ;
	rdfs:domain uml-class:ConnectorEnd ;
	rdfs:range uml-class:ConnectableElement ;
	mms-ontology:umlPropertySource uml-property:ConnectorEnd-role .

mms-property:roleFromStructuredClassifier a mms-ontology:UmlObjectProperty ;
	mms-ontology:cardinality "*"^^uml-model-dt:cardinalityRange ;
	mms-ontology:key "roleIds" ;
	rdfs:label "roleFromStructuredClassifier" ;
	rdfs:comment "A ConnectableElement that is the role of this StructuredClassifier. Based on the UML property 'StructuredClassifier-role' which is described as: The roles that instances may play in this StructuredClassifier."@en ;
	rdfs:domain uml-class:StructuredClassifier ;
	rdfs:range uml-class:ConnectableElement ;
	mms-ontology:umlPropertySource uml-property:StructuredClassifier-role .

mms-property:settingBoolean a mms-ontology:UmlDatatypeProperty ;
	mms-ontology:cardinality "1"^^uml-model-dt:cardinalityRange ;
	mms-ontology:key "settingId" ;
	rdfs:label "settingBoolean" ;
	rdfs:comment "The Boolean that is the setting of this Continuation. Based on the UML property 'Continuation-setting' which is described as: True: when the Continuation is at the end of the enclosing InteractionFragment and False when it is in the beginning."@en ;
	rdfs:domain uml-class:Continuation ;
	rdfs:range xsd:boolean ;
	mms-ontology:umlPropertySource uml-property:Continuation-setting .

mms-property:constrainedElement a mms-ontology:UmlObjectProperty ;
	mms-ontology:cardinality "*"^^uml-model-dt:cardinalityRange ;
	mms-ontology:key "constrainedElementIds" ;
	rdfs:label "constrainedElement" ;
	rdfs:comment "A Element that belongs to this Constraint. Based on the UML property 'Constraint-constrainedElement' which is described as: The ordered set of Elements referenced by this Constraint."@en ;
	rdfs:domain uml-class:Constraint ;
	rdfs:range uml-class:Element ;
	mms-ontology:umlPropertySource uml-property:Constraint-constrainedElement .

mms-property:contentString a mms-ontology:UmlDatatypeProperty ;
	mms-ontology:cardinality "1"^^uml-model-dt:cardinalityRange ;
	mms-ontology:key "contentId" ;
	rdfs:label "contentString" ;
	rdfs:comment "The String that is the content of this Image. Based on the UML property 'Image-content' which is described as: This contains the serialization of the image according to the format. The value could represent a bitmap, image such as a GIF file, or drawing 'instructions' using a standard such as Scalable Vector Graphic (SVG) (which is XML based)."@en ;
	rdfs:domain uml-class:Image ;
	rdfs:range xsd:string ;
	mms-ontology:umlPropertySource uml-property:Image-content .

mms-property:nestingPackage a mms-ontology:UmlObjectProperty ;
	mms-ontology:cardinality "1"^^uml-model-dt:cardinalityRange ;
	mms-ontology:key "nestingPackageId" ;
	rdfs:label "nestingPackage" ;
	rdfs:comment "The Package that belongs to this Package. Based on the UML property 'Package-nestingPackage' which is described as: References the Package that owns this Package."@en ;
	rdfs:domain uml-class:Package ;
	rdfs:range uml-class:Package ;
	mms-ontology:umlPropertySource uml-property:Package-nestingPackage .

mms-property:generalFromClassifier a mms-ontology:UmlObjectProperty ;
	mms-ontology:cardinality "*"^^uml-model-dt:cardinalityRange ;
	mms-ontology:key "generalIds" ;
	rdfs:label "generalFromClassifier" ;
	rdfs:comment "A Classifier that is the general of this Classifier. Based on the UML property 'Classifier-general' which is described as: The generalizing Classifiers for this Classifier."@en ;
	rdfs:domain uml-class:Classifier ;
	rdfs:range uml-class:Classifier ;
	mms-ontology:umlPropertySource uml-property:Classifier-general .

mms-property:generalClassifierFromGeneralization a mms-ontology:UmlObjectProperty ;
	mms-ontology:cardinality "1"^^uml-model-dt:cardinalityRange ;
	mms-ontology:key "generalId" ;
	rdfs:label "generalClassifierFromGeneralization" ;
	rdfs:comment "The Classifier that is the general of this Generalization. Based on the UML property 'Generalization-general' which is described as: The general classifier in the Generalization relationship."@en ;
	rdfs:domain uml-class:Generalization ;
	rdfs:range uml-class:Classifier ;
	mms-ontology:umlPropertySource uml-property:Generalization-general .

mms-property:handler a mms-ontology:UmlObjectProperty ;
	mms-ontology:cardinality "*"^^uml-model-dt:cardinalityRange ;
	mms-ontology:key "handlerIds" ;
	rdfs:label "handler" ;
	rdfs:comment "A ExceptionHandler that is the handler of this ExecutableNode. Based on the UML property 'ExecutableNode-handler' which is described as: A set of ExceptionHandlers that are examined if an exception propagates out of the ExceptionNode."@en ;
	rdfs:domain uml-class:ExecutableNode ;
	rdfs:range uml-class:ExceptionHandler ;
	mms-ontology:umlPropertySource uml-property:ExecutableNode-handler .

mms-property:collaborationRole a mms-ontology:UmlObjectProperty ;
	mms-ontology:cardinality "*"^^uml-model-dt:cardinalityRange ;
	mms-ontology:key "collaborationRoleIds" ;
	rdfs:label "collaborationRole" ;
	rdfs:comment "A ConnectableElement that is the collaborationRole of this Collaboration. Based on the UML property 'Collaboration-collaborationRole' which is described as: Represents the participants in the Collaboration."@en ;
	rdfs:domain uml-class:Collaboration ;
	rdfs:range uml-class:ConnectableElement ;
	mms-ontology:umlPropertySource uml-property:Collaboration-collaborationRole .

mms-property:fileNameString a mms-ontology:UmlDatatypeProperty ;
	mms-ontology:cardinality "1"^^uml-model-dt:cardinalityRange ;
	mms-ontology:key "fileNameId" ;
	rdfs:label "fileNameString" ;
	rdfs:comment "The String that is the fileName of this Artifact. Based on the UML property 'Artifact-fileName' which is described as: A concrete name that is used to refer to the Artifact in a physical context. Example: file system name, universal resource locator."@en ;
	rdfs:domain uml-class:Artifact ;
	rdfs:range xsd:string ;
	mms-ontology:umlPropertySource uml-property:Artifact-fileName .

mms-property:redefinedPort a mms-ontology:UmlObjectProperty ;
	mms-ontology:cardinality "*"^^uml-model-dt:cardinalityRange ;
	mms-ontology:key "redefinedPortIds" ;
	rdfs:label "redefinedPort" ;
	rdfs:comment "A Port that belongs to this Port. Based on the UML property 'Port-redefinedPort' which is described as: A Port may be redefined when its containing EncapsulatedClassifier is specialized. The redefining Port may have additional Interfaces to those that are associated with the redefined Port or it may replace an Interface by one of its subtypes."@en ;
	rdfs:domain uml-class:Port ;
	rdfs:range uml-class:Port ;
	mms-ontology:umlPropertySource uml-property:Port-redefinedPort .

mms-property:client a mms-ontology:UmlObjectProperty ;
	mms-ontology:cardinality "*"^^uml-model-dt:cardinalityRange ;
	mms-ontology:key "clientIds" ;
	rdfs:label "client" ;
	rdfs:comment "A NamedElement that is the client of this Dependency. Based on the UML property 'Dependency-client' which is described as: The Element(s) dependent on the supplier Element(s). In some cases (such as a trace Abstraction) the assignment of direction (that is, the designation of the client Element) is at the discretion of the modeler and is a stipulation."@en ;
	rdfs:domain uml-class:Dependency ;
	rdfs:range uml-class:NamedElement ;
	mms-ontology:umlPropertySource uml-property:Dependency-client .

mms-property:conditionConstraintFromExtend a mms-ontology:UmlObjectProperty ;
	mms-ontology:cardinality "1"^^uml-model-dt:cardinalityRange ;
	mms-ontology:key "conditionId" ;
	rdfs:label "conditionConstraintFromExtend" ;
	rdfs:comment "The Constraint that is the condition of this Extend. Based on the UML property 'Extend-condition' which is described as: References the condition that must hold when the first ExtensionPoint is reached for the extension to take place. If no constraint is associated with the Extend relationship, the extension is unconditional."@en ;
	rdfs:domain uml-class:Extend ;
	rdfs:range uml-class:Constraint ;
	mms-ontology:umlPropertySource uml-property:Extend-condition .

mms-property:conditionFromParameterSet a mms-ontology:UmlObjectProperty ;
	mms-ontology:cardinality "*"^^uml-model-dt:cardinalityRange ;
	mms-ontology:key "conditionIds" ;
	rdfs:label "conditionFromParameterSet" ;
	rdfs:comment "A Constraint that is the condition of this ParameterSet. Based on the UML property 'ParameterSet-condition' which is described as: A constraint that should be satisfied for the owner of the Parameters in an input ParameterSet to start execution using the values provided for those Parameters, or the owner of the Parameters in an output ParameterSet to end execution providing the values for those Parameters, if all preconditions and conditions on input ParameterSets were satisfied."@en ;
	rdfs:domain uml-class:ParameterSet ;
	rdfs:range uml-class:Constraint ;
	mms-ontology:umlPropertySource uml-property:ParameterSet-condition .

mms-property:interfaceRealization a mms-ontology:UmlObjectProperty ;
	mms-ontology:cardinality "*"^^uml-model-dt:cardinalityRange ;
	mms-ontology:key "interfaceRealizationIds" ;
	rdfs:label "interfaceRealization" ;
	rdfs:comment "A InterfaceRealization that belongs to this BehavioredClassifier. Based on the UML property 'BehavioredClassifier-interfaceRealization' which is described as: The set of InterfaceRealizations owned by the BehavioredClassifier. Interface realizations reference the Interfaces of which the BehavioredClassifier is an implementation."@en ;
	rdfs:domain uml-class:BehavioredClassifier ;
	rdfs:range uml-class:InterfaceRealization ;
	mms-ontology:umlPropertySource uml-property:BehavioredClassifier-interfaceRealization .

mms-property:includingCaseUseCase a mms-ontology:UmlObjectProperty ;
	mms-ontology:cardinality "1"^^uml-model-dt:cardinalityRange ;
	mms-ontology:key "includingCaseId" ;
	rdfs:label "includingCaseUseCase" ;
	rdfs:comment "The UseCase that is the includingCase of this Include. Based on the UML property 'Include-includingCase' which is described as: The UseCase which includes the addition and owns the Include relationship."@en ;
	rdfs:domain uml-class:Include ;
	rdfs:range uml-class:UseCase ;
	mms-ontology:umlPropertySource uml-property:Include-includingCase .

mms-property:navigableOwnedEnd a mms-ontology:UmlObjectProperty ;
	mms-ontology:cardinality "*"^^uml-model-dt:cardinalityRange ;
	mms-ontology:key "navigableOwnedEndIds" ;
	rdfs:label "navigableOwnedEnd" ;
	rdfs:comment "A Property that is the navigableOwnedEnd of this Association. Based on the UML property 'Association-navigableOwnedEnd' which is described as: The navigable ends that are owned by the Association itself."@en ;
	rdfs:domain uml-class:Association ;
	rdfs:range uml-class:Property ;
	mms-ontology:umlPropertySource uml-property:Association-navigableOwnedEnd .

mms-property:destroyAtInputPin a mms-ontology:UmlObjectProperty ;
	mms-ontology:cardinality "1"^^uml-model-dt:cardinalityRange ;
	mms-ontology:key "destroyAtId" ;
	rdfs:label "destroyAtInputPin" ;
	rdfs:comment "The InputPin that is the destroyAt of this LinkEndDestructionData. Based on the UML property 'LinkEndDestructionData-destroyAt' which is described as: The InputPin that provides the position of an existing link to be destroyed in an ordered, nonunique Association end. The type of the destroyAt InputPin is UnlimitedNatural, but the value cannot be zero or unlimited."@en ;
	rdfs:domain uml-class:LinkEndDestructionData ;
	rdfs:range uml-class:InputPin ;
	mms-ontology:umlPropertySource uml-property:LinkEndDestructionData-destroyAt .

mms-property:relatedElement a mms-ontology:UmlObjectProperty ;
	mms-ontology:cardinality "*"^^uml-model-dt:cardinalityRange ;
	mms-ontology:key "relatedElementIds" ;
	rdfs:label "relatedElement" ;
	rdfs:comment "A Element that belongs to this Relationship. Based on the UML property 'Relationship-relatedElement' which is described as: Specifies the elements related by the Relationship."@en ;
	rdfs:domain uml-class:Relationship ;
	rdfs:range uml-class:Element ;
	mms-ontology:umlPropertySource uml-property:Relationship-relatedElement .

mms-property:containedNode a mms-ontology:UmlObjectProperty ;
	mms-ontology:cardinality "*"^^uml-model-dt:cardinalityRange ;
	mms-ontology:key "containedNodeIds" ;
	rdfs:label "containedNode" ;
	rdfs:comment "A ActivityNode that is the containedNode of this ActivityGroup. Based on the UML property 'ActivityGroup-containedNode' which is described as: ActivityNodes immediately contained in the ActivityGroup."@en ;
	rdfs:domain uml-class:ActivityGroup ;
	rdfs:range uml-class:ActivityNode ;
	mms-ontology:umlPropertySource uml-property:ActivityGroup-containedNode .

mms-property:exprValueSpecificationFromTimeExpression a mms-ontology:UmlObjectProperty ;
	mms-ontology:cardinality "1"^^uml-model-dt:cardinalityRange ;
	mms-ontology:key "exprId" ;
	rdfs:label "exprValueSpecificationFromTimeExpression" ;
	rdfs:comment "The ValueSpecification that is the expr of this TimeExpression. Based on the UML property 'TimeExpression-expr' which is described as: A ValueSpecification that evaluates to the value of the TimeExpression."@en ;
	rdfs:domain uml-class:TimeExpression ;
	rdfs:range uml-class:ValueSpecification ;
	mms-ontology:umlPropertySource uml-property:TimeExpression-expr .

mms-property:exprValueSpecificationFromDuration a mms-ontology:UmlObjectProperty ;
	mms-ontology:cardinality "1"^^uml-model-dt:cardinalityRange ;
	mms-ontology:key "exprId" ;
	rdfs:label "exprValueSpecificationFromDuration" ;
	rdfs:comment "The ValueSpecification that is the expr of this Duration. Based on the UML property 'Duration-expr' which is described as: A ValueSpecification that evaluates to the value of the Duration."@en ;
	rdfs:domain uml-class:Duration ;
	rdfs:range uml-class:ValueSpecification ;
	mms-ontology:umlPropertySource uml-property:Duration-expr .

mms-property:localPrecondition a mms-ontology:UmlObjectProperty ;
	mms-ontology:cardinality "*"^^uml-model-dt:cardinalityRange ;
	mms-ontology:key "localPreconditionIds" ;
	rdfs:label "localPrecondition" ;
	rdfs:comment "A Constraint that is the localPrecondition of this Action. Based on the UML property 'Action-localPrecondition' which is described as: A Constraint that must be satisfied when execution of the Action is started."@en ;
	rdfs:domain uml-class:Action ;
	rdfs:range uml-class:Constraint ;
	mms-ontology:umlPropertySource uml-property:Action-localPrecondition .

mms-property:subsettedProperty a mms-ontology:UmlObjectProperty ;
	mms-ontology:cardinality "*"^^uml-model-dt:cardinalityRange ;
	mms-ontology:key "subsettedPropertyIds" ;
	rdfs:label "subsettedProperty" ;
	rdfs:comment "A Property that belongs to this Property. Based on the UML property 'Property-subsettedProperty' which is described as: The properties of which this Property is constrained to be a subset, if any."@en ;
	rdfs:domain uml-class:Property ;
	rdfs:range uml-class:Property ;
	mms-ontology:umlPropertySource uml-property:Property-subsettedProperty .

mms-property:abstractionComponent a mms-ontology:UmlObjectProperty ;
	mms-ontology:cardinality "1"^^uml-model-dt:cardinalityRange ;
	mms-ontology:key "abstractionId" ;
	rdfs:label "abstractionComponent" ;
	rdfs:comment "The Component that is the abstraction of this ComponentRealization. Based on the UML property 'ComponentRealization-abstraction' which is described as: The Component that owns this ComponentRealization and which is implemented by its realizing Classifiers."@en ;
	rdfs:domain uml-class:ComponentRealization ;
	rdfs:range uml-class:Component ;
	mms-ontology:umlPropertySource uml-property:ComponentRealization-abstraction .

mms-property:enclosingInteraction a mms-ontology:UmlObjectProperty ;
	mms-ontology:cardinality "1"^^uml-model-dt:cardinalityRange ;
	mms-ontology:key "enclosingInteractionId" ;
	rdfs:label "enclosingInteraction" ;
	rdfs:comment "The Interaction that belongs to this InteractionFragment. Based on the UML property 'InteractionFragment-enclosingInteraction' which is described as: The Interaction enclosing this InteractionFragment."@en ;
	rdfs:domain uml-class:InteractionFragment ;
	rdfs:range uml-class:Interaction ;
	mms-ontology:umlPropertySource uml-property:InteractionFragment-enclosingInteraction .

mms-property:viewpointString a mms-ontology:UmlDatatypeProperty ;
	mms-ontology:cardinality "1"^^uml-model-dt:cardinalityRange ;
	mms-ontology:key "viewpointId" ;
	rdfs:label "viewpointString" ;
	rdfs:comment "The String that is the viewpoint of this Model. Based on the UML property 'Model-viewpoint' which is described as: The name of the viewpoint that is expressed by a model (this name may refer to a profile definition)."@en ;
	rdfs:domain uml-class:Model ;
	rdfs:range xsd:string ;
	mms-ontology:umlPropertySource uml-property:Model-viewpoint .

mms-property:redefinedBehavior a mms-ontology:UmlObjectProperty ;
	mms-ontology:cardinality "*"^^uml-model-dt:cardinalityRange ;
	mms-ontology:key "redefinedBehaviorIds" ;
	rdfs:label "redefinedBehavior" ;
	rdfs:comment "A Behavior that belongs to this Behavior. Based on the UML property 'Behavior-redefinedBehavior' which is described as: References the Behavior that this Behavior redefines. A subtype of Behavior may redefine any other subtype of Behavior. If the Behavior implements a BehavioralFeature, it replaces the redefined Behavior. If the Behavior is a classifierBehavior, it extends the redefined Behavior."@en ;
	rdfs:domain uml-class:Behavior ;
	rdfs:range uml-class:Behavior ;
	mms-ontology:umlPropertySource uml-property:Behavior-redefinedBehavior .

mms-property:finishOccurrenceSpecification a mms-ontology:UmlObjectProperty ;
	mms-ontology:cardinality "1"^^uml-model-dt:cardinalityRange ;
	mms-ontology:key "finishId" ;
	rdfs:label "finishOccurrenceSpecification" ;
	rdfs:comment "The OccurrenceSpecification that is the finish of this ExecutionSpecification. Based on the UML property 'ExecutionSpecification-finish' which is described as: References the OccurrenceSpecification that designates the finish of the Action or Behavior."@en ;
	rdfs:domain uml-class:ExecutionSpecification ;
	rdfs:range uml-class:OccurrenceSpecification ;
	mms-ontology:umlPropertySource uml-property:ExecutionSpecification-finish .

mms-property:redefinedConnector a mms-ontology:UmlObjectProperty ;
	mms-ontology:cardinality "*"^^uml-model-dt:cardinalityRange ;
	mms-ontology:key "redefinedConnectorIds" ;
	rdfs:label "redefinedConnector" ;
	rdfs:comment "A Connector that belongs to this Connector. Based on the UML property 'Connector-redefinedConnector' which is described as: A Connector may be redefined when its containing Classifier is specialized. The redefining Connector may have a type that specializes the type of the redefined Connector. The types of the ConnectorEnds of the redefining Connector may specialize the types of the ConnectorEnds of the redefined Connector. The properties of the ConnectorEnds of the redefining Connector may be replaced."@en ;
	rdfs:domain uml-class:Connector ;
	rdfs:range uml-class:Connector ;
	mms-ontology:umlPropertySource uml-property:Connector-redefinedConnector .

mms-property:protocolProtocolStateMachineFromInterface a mms-ontology:UmlObjectProperty ;
	mms-ontology:cardinality "1"^^uml-model-dt:cardinalityRange ;
	mms-ontology:key "protocolId" ;
	rdfs:label "protocolProtocolStateMachineFromInterface" ;
	rdfs:comment "The ProtocolStateMachine that is the protocol of this Interface. Based on the UML property 'Interface-protocol' which is described as: References a ProtocolStateMachine specifying the legal sequences of the invocation of the BehavioralFeatures described in the Interface."@en ;
	rdfs:domain uml-class:Interface ;
	rdfs:range uml-class:ProtocolStateMachine ;
	mms-ontology:umlPropertySource uml-property:Interface-protocol .

mms-property:protocolProtocolStateMachineFromPort a mms-ontology:UmlObjectProperty ;
	mms-ontology:cardinality "1"^^uml-model-dt:cardinalityRange ;
	mms-ontology:key "protocolId" ;
	rdfs:label "protocolProtocolStateMachineFromPort" ;
	rdfs:comment "The ProtocolStateMachine that is the protocol of this Port. Based on the UML property 'Port-protocol' which is described as: An optional ProtocolStateMachine which describes valid interactions at this interaction point."@en ;
	rdfs:domain uml-class:Port ;
	rdfs:range uml-class:ProtocolStateMachine ;
	mms-ontology:umlPropertySource uml-property:Port-protocol .

mms-property:ownedBehavior a mms-ontology:UmlObjectProperty ;
	mms-ontology:cardinality "*"^^uml-model-dt:cardinalityRange ;
	mms-ontology:key "ownedBehaviorIds" ;
	rdfs:label "ownedBehavior" ;
	rdfs:comment "A Behavior that belongs to this BehavioredClassifier. Based on the UML property 'BehavioredClassifier-ownedBehavior' which is described as: Behaviors owned by a BehavioredClassifier."@en ;
	rdfs:domain uml-class:BehavioredClassifier ;
	rdfs:range uml-class:Behavior ;
	mms-ontology:umlPropertySource uml-property:BehavioredClassifier-ownedBehavior .

mms-property:isAssured a mms-ontology:UmlDatatypeProperty ;
	mms-ontology:key "isAssured" ;
	rdfs:label "isAssured" ;
	rdfs:comment "If true, the modeler asserts that the test for at least one Clause of the ConditionalNode will succeed."@en ;
	rdfs:domain uml-class:ConditionalNode ;
	rdfs:range xsd:boolean ;
	mms-ontology:umlPropertySource uml-property:ConditionalNode-isAssured .

mms-property:isAssuredConditionalNode a mms-ontology:UmlDatatypeProperty ;
	owl:equivalentProperty mms-property:isAssured .

mms-property:transformationBehavior a mms-ontology:UmlObjectProperty ;
	mms-ontology:cardinality "1"^^uml-model-dt:cardinalityRange ;
	mms-ontology:key "transformationId" ;
	rdfs:label "transformationBehavior" ;
	rdfs:comment "The Behavior that is the transformation of this ObjectFlow. Based on the UML property 'ObjectFlow-transformation' which is described as: A Behavior used to change or replace object tokens flowing along the ObjectFlow."@en ;
	rdfs:domain uml-class:ObjectFlow ;
	rdfs:range uml-class:Behavior ;
	mms-ontology:umlPropertySource uml-property:ObjectFlow-transformation .

mms-property:realizingConnector a mms-ontology:UmlObjectProperty ;
	mms-ontology:cardinality "*"^^uml-model-dt:cardinalityRange ;
	mms-ontology:key "realizingConnectorIds" ;
	rdfs:label "realizingConnector" ;
	rdfs:comment "A Connector that belongs to this InformationFlow. Based on the UML property 'InformationFlow-realizingConnector' which is described as: Determines which Connectors will realize the specified flow."@en ;
	rdfs:domain uml-class:InformationFlow ;
	rdfs:range uml-class:Connector ;
	mms-ontology:umlPropertySource uml-property:InformationFlow-realizingConnector .

mms-property:importedPackage a mms-ontology:UmlObjectProperty ;
	mms-ontology:cardinality "1"^^uml-model-dt:cardinalityRange ;
	mms-ontology:key "importedPackageId" ;
	rdfs:label "importedPackage" ;
	rdfs:comment "The Package that belongs to this PackageImport. Based on the UML property 'PackageImport-importedPackage' which is described as: Specifies the Package whose members are imported into a Namespace."@en ;
	rdfs:domain uml-class:PackageImport ;
	rdfs:range uml-class:Package ;
	mms-ontology:umlPropertySource uml-property:PackageImport-importedPackage .

mms-property:stateInvariantConstraint a mms-ontology:UmlObjectProperty ;
	mms-ontology:cardinality "1"^^uml-model-dt:cardinalityRange ;
	mms-ontology:key "stateInvariantId" ;
	rdfs:label "stateInvariantConstraint" ;
	rdfs:comment "The Constraint that is the stateInvariant of this State. Based on the UML property 'State-stateInvariant' which is described as: Specifies conditions that are always true when this State is the current State. In ProtocolStateMachines state invariants are additional conditions to the preconditions of the outgoing Transitions, and to the postcondition of the incoming Transitions."@en ;
	rdfs:domain uml-class:State ;
	rdfs:range uml-class:Constraint ;
	mms-ontology:umlPropertySource uml-property:State-stateInvariant .

mms-property:inActivity a mms-ontology:UmlObjectProperty ;
	mms-ontology:cardinality "1"^^uml-model-dt:cardinalityRange ;
	mms-ontology:key "inActivityId" ;
	rdfs:label "inActivity" ;
	rdfs:comment "The Activity that belongs to this ActivityGroup. Based on the UML property 'ActivityGroup-inActivity' which is described as: The Activity containing the ActivityGroup, if it is directly owned by an Activity."@en ;
	rdfs:domain uml-class:ActivityGroup ;
	rdfs:range uml-class:Activity ;
	mms-ontology:umlPropertySource uml-property:ActivityGroup-inActivity .

mms-property:endType a mms-ontology:UmlObjectProperty ;
	mms-ontology:cardinality "*"^^uml-model-dt:cardinalityRange ;
	mms-ontology:key "endTypeIds" ;
	rdfs:label "endType" ;
	rdfs:comment "A Type that belongs to this Association. Based on the UML property 'Association-endType' which is described as: The Classifiers that are used as types of the ends of the Association."@en ;
	rdfs:domain uml-class:Association ;
	rdfs:range uml-class:Type ;
	mms-ontology:umlPropertySource uml-property:Association-endType .

mms-property:clientDependency a mms-ontology:UmlObjectProperty ;
	mms-ontology:cardinality "*"^^uml-model-dt:cardinalityRange ;
	mms-ontology:key "clientDependencyIds" ;
	rdfs:label "clientDependency" ;
	rdfs:comment "A Dependency that belongs to this NamedElement. Based on the UML property 'NamedElement-clientDependency' which is described as: Indicates the Dependencies that reference this NamedElement as a client."@en ;
	rdfs:domain uml-class:NamedElement ;
	rdfs:range uml-class:Dependency ;
	mms-ontology:umlPropertySource uml-property:NamedElement-clientDependency .

mms-property:nameExpressionStringExpression a mms-ontology:UmlObjectProperty ;
	mms-ontology:cardinality "1"^^uml-model-dt:cardinalityRange ;
	mms-ontology:key "nameExpressionId" ;
	rdfs:label "nameExpressionStringExpression" ;
	rdfs:comment "The StringExpression that is the nameExpression of this NamedElement. Based on the UML property 'NamedElement-nameExpression' which is described as: The StringExpression used to define the name of this NamedElement."@en ;
	rdfs:domain uml-class:NamedElement ;
	rdfs:range uml-class:StringExpression ;
	mms-ontology:umlPropertySource uml-property:NamedElement-nameExpression .

mms-property:containedEdge a mms-ontology:UmlObjectProperty ;
	mms-ontology:cardinality "*"^^uml-model-dt:cardinalityRange ;
	mms-ontology:key "containedEdgeIds" ;
	rdfs:label "containedEdge" ;
	rdfs:comment "A ActivityEdge that is the containedEdge of this ActivityGroup. Based on the UML property 'ActivityGroup-containedEdge' which is described as: ActivityEdges immediately contained in the ActivityGroup."@en ;
	rdfs:domain uml-class:ActivityGroup ;
	rdfs:range uml-class:ActivityEdge ;
	mms-ontology:umlPropertySource uml-property:ActivityGroup-containedEdge .

mms-property:specificMachineProtocolStateMachine a mms-ontology:UmlObjectProperty ;
	mms-ontology:cardinality "1"^^uml-model-dt:cardinalityRange ;
	mms-ontology:key "specificMachineId" ;
	rdfs:label "specificMachineProtocolStateMachine" ;
	rdfs:comment "The ProtocolStateMachine that is the specificMachine of this ProtocolConformance. Based on the UML property 'ProtocolConformance-specificMachine' which is described as: Specifies the ProtocolStateMachine which conforms to the general ProtocolStateMachine."@en ;
	rdfs:domain uml-class:ProtocolConformance ;
	rdfs:range uml-class:ProtocolStateMachine ;
	mms-ontology:umlPropertySource uml-property:ProtocolConformance-specificMachine .

mms-property:weightValueSpecification a mms-ontology:UmlObjectProperty ;
	mms-ontology:cardinality "1"^^uml-model-dt:cardinalityRange ;
	mms-ontology:key "weightId" ;
	rdfs:label "weightValueSpecification" ;
	rdfs:comment "The ValueSpecification that is the weight of this ActivityEdge. Based on the UML property 'ActivityEdge-weight' which is described as: The minimum number of tokens that must traverse the ActivityEdge at the same time. If no weight is specified, this is equivalent to specifying a constant value of 1."@en ;
	rdfs:domain uml-class:ActivityEdge ;
	rdfs:range uml-class:ValueSpecification ;
	mms-ontology:umlPropertySource uml-property:ActivityEdge-weight .

mms-property:isConjugated a mms-ontology:UmlDatatypeProperty ;
	mms-ontology:key "isConjugated" ;
	rdfs:label "isConjugated" ;
	rdfs:comment "Specifies the way that the provided and required Interfaces are derived from the Port’s Type."@en ;
	rdfs:domain uml-class:Port ;
	rdfs:range xsd:boolean ;
	mms-ontology:umlPropertySource uml-property:Port-isConjugated .

mms-property:isConjugatedPort a mms-ontology:UmlDatatypeProperty ;
	owl:equivalentProperty mms-property:isConjugated .

mms-property:conformance a mms-ontology:UmlObjectProperty ;
	mms-ontology:cardinality "*"^^uml-model-dt:cardinalityRange ;
	mms-ontology:key "conformanceIds" ;
	rdfs:label "conformance" ;
	rdfs:comment "A ProtocolConformance that is the conformance of this ProtocolStateMachine. Based on the UML property 'ProtocolStateMachine-conformance' which is described as: Conformance between ProtocolStateMachine "@en ;
	rdfs:domain uml-class:ProtocolStateMachine ;
	rdfs:range uml-class:ProtocolConformance ;
	mms-ontology:umlPropertySource uml-property:ProtocolStateMachine-conformance .

mms-property:regionAsInputExpansionRegion a mms-ontology:UmlObjectProperty ;
	mms-ontology:cardinality "1"^^uml-model-dt:cardinalityRange ;
	mms-ontology:key "regionAsInputId" ;
	rdfs:label "regionAsInputExpansionRegion" ;
	rdfs:comment "The ExpansionRegion that is the regionAsInput of this ExpansionNode. Based on the UML property 'ExpansionNode-regionAsInput' which is described as: The ExpansionRegion for which the ExpansionNode is an input."@en ;
	rdfs:domain uml-class:ExpansionNode ;
	rdfs:range uml-class:ExpansionRegion ;
	mms-ontology:umlPropertySource uml-property:ExpansionNode-regionAsInput .

mms-property:cfragmentGate a mms-ontology:UmlObjectProperty ;
	mms-ontology:cardinality "*"^^uml-model-dt:cardinalityRange ;
	mms-ontology:key "cfragmentGateIds" ;
	rdfs:label "cfragmentGate" ;
	rdfs:comment "A Gate that belongs to this CombinedFragment. Based on the UML property 'CombinedFragment-cfragmentGate' which is described as: Specifies the gates that form the interface between this CombinedFragment and its surroundings"@en ;
	rdfs:domain uml-class:CombinedFragment ;
	rdfs:range uml-class:Gate ;
	mms-ontology:umlPropertySource uml-property:CombinedFragment-cfragmentGate .

mms-property:isExternal a mms-ontology:UmlDatatypeProperty ;
	mms-ontology:key "isExternal" ;
	rdfs:label "isExternal" ;
	rdfs:comment "Indicates whether the ActivityPartition represents an entity to which the partitioning structure does not apply."@en ;
	rdfs:domain uml-class:ActivityPartition ;
	rdfs:range xsd:boolean ;
	mms-ontology:umlPropertySource uml-property:ActivityPartition-isExternal .

mms-property:isExternalActivityPartition a mms-ontology:UmlDatatypeProperty ;
	owl:equivalentProperty mms-property:isExternal .

mms-property:manifestation a mms-ontology:UmlObjectProperty ;
	mms-ontology:cardinality "*"^^uml-model-dt:cardinalityRange ;
	mms-ontology:key "manifestationIds" ;
	rdfs:label "manifestation" ;
	rdfs:comment "A Manifestation that belongs to this Artifact. Based on the UML property 'Artifact-manifestation' which is described as: The set of model elements that are manifested in the Artifact. That is, these model elements are utilized in the construction (or generation) of the artifact."@en ;
	rdfs:domain uml-class:Artifact ;
	rdfs:range uml-class:Manifestation ;
	mms-ontology:umlPropertySource uml-property:Artifact-manifestation .

mms-property:parameterSubstitution a mms-ontology:UmlObjectProperty ;
	mms-ontology:cardinality "*"^^uml-model-dt:cardinalityRange ;
	mms-ontology:key "parameterSubstitutionIds" ;
	rdfs:label "parameterSubstitution" ;
	rdfs:comment "A TemplateParameterSubstitution that is the parameterSubstitution of this TemplateBinding. Based on the UML property 'TemplateBinding-parameterSubstitution' which is described as: The TemplateParameterSubstitutions owned by this TemplateBinding."@en ;
	rdfs:domain uml-class:TemplateBinding ;
	rdfs:range uml-class:TemplateParameterSubstitution ;
	mms-ontology:umlPropertySource uml-property:TemplateBinding-parameterSubstitution .

mms-property:isID a mms-ontology:UmlDatatypeProperty ;
	mms-ontology:key "isID" ;
	rdfs:label "isID" ;
	rdfs:comment "True indicates this property can be used to uniquely identify an instance of the containing Class."@en ;
	rdfs:domain uml-class:Property ;
	rdfs:range xsd:boolean ;
	mms-ontology:umlPropertySource uml-property:Property-isID .

mms-property:isIDProperty a mms-ontology:UmlDatatypeProperty ;
	owl:equivalentProperty mms-property:isID .

mms-property:subject a mms-ontology:UmlObjectProperty ;
	mms-ontology:cardinality "*"^^uml-model-dt:cardinalityRange ;
	mms-ontology:key "subjectIds" ;
	rdfs:label "subject" ;
	rdfs:comment "A Classifier that is the subject of this UseCase. Based on the UML property 'UseCase-subject' which is described as: The subjects to which this UseCase applies. Each subject or its parts realize all the UseCases that apply to it."@en ;
	rdfs:domain uml-class:UseCase ;
	rdfs:range uml-class:Classifier ;
	mms-ontology:umlPropertySource uml-property:UseCase-subject .

mms-property:importedMember a mms-ontology:UmlObjectProperty ;
	mms-ontology:cardinality "*"^^uml-model-dt:cardinalityRange ;
	mms-ontology:key "importedMemberIds" ;
	rdfs:label "importedMember" ;
	rdfs:comment "A PackageableElement that is the importedMember of this Namespace. Based on the UML property 'Namespace-importedMember' which is described as: References the PackageableElements that are members of this Namespace as a result of either PackageImports or ElementImports."@en ;
	rdfs:domain uml-class:Namespace ;
	rdfs:range uml-class:PackageableElement ;
	mms-ontology:umlPropertySource uml-property:Namespace-importedMember .

mms-property:formatString a mms-ontology:UmlDatatypeProperty ;
	mms-ontology:cardinality "1"^^uml-model-dt:cardinalityRange ;
	mms-ontology:key "formatId" ;
	rdfs:label "formatString" ;
	rdfs:comment "The String that is the format of this Image. Based on the UML property 'Image-format' which is described as: This indicates the format of the content, which is how the string content should be interpreted. The following values are reserved: SVG, GIF, PNG, JPG, WMF, EMF, BMP. In addition the prefix 'MIME: ' is also reserved. This option can be used as an alternative to express the reserved values above, for example &#34;SVG&#34; could instead be expressed as &#34;MIME: image/svg+xml&#34;."@en ;
	rdfs:domain uml-class:Image ;
	rdfs:range xsd:string ;
	mms-ontology:umlPropertySource uml-property:Image-format .

mms-property:definingEndProperty a mms-ontology:UmlObjectProperty ;
	mms-ontology:cardinality "1"^^uml-model-dt:cardinalityRange ;
	mms-ontology:key "definingEndId" ;
	rdfs:label "definingEndProperty" ;
	rdfs:comment "The Property that is the definingEnd of this ConnectorEnd. Based on the UML property 'ConnectorEnd-definingEnd' which is described as: A derived property referencing the corresponding end on the Association which types the Connector owing this ConnectorEnd, if any. It is derived by selecting the end at the same place in the ordering of Association ends as this ConnectorEnd."@en ;
	rdfs:domain uml-class:ConnectorEnd ;
	rdfs:range uml-class:Property ;
	mms-ontology:umlPropertySource uml-property:ConnectorEnd-definingEnd .

mms-property:isBehavior a mms-ontology:UmlDatatypeProperty ;
	mms-ontology:key "isBehavior" ;
	rdfs:label "isBehavior" ;
	rdfs:comment "Specifies whether requests arriving at this Port are sent to the classifier behavior of this EncapsulatedClassifier. Such a Port is referred to as a behavior Port. Any invocation of a BehavioralFeature targeted at a behavior Port will be handled by the instance of the owning EncapsulatedClassifier itself, rather than by any instances that it may contain."@en ;
	rdfs:domain uml-class:Port ;
	rdfs:range xsd:boolean ;
	mms-ontology:umlPropertySource uml-property:Port-isBehavior .

mms-property:isBehaviorPort a mms-ontology:UmlDatatypeProperty ;
	owl:equivalentProperty mms-property:isBehavior .

mms-property:classifierBehavior a mms-ontology:UmlObjectProperty ;
	mms-ontology:cardinality "1"^^uml-model-dt:cardinalityRange ;
	mms-ontology:key "classifierBehaviorId" ;
	rdfs:label "classifierBehavior" ;
	rdfs:comment "The Behavior that belongs to this BehavioredClassifier. Based on the UML property 'BehavioredClassifier-classifierBehavior' which is described as: A Behavior that specifies the behavior of the BehavioredClassifier itself."@en ;
	rdfs:domain uml-class:BehavioredClassifier ;
	rdfs:range uml-class:Behavior ;
	mms-ontology:umlPropertySource uml-property:BehavioredClassifier-classifierBehavior .

mms-property:substitution a mms-ontology:UmlObjectProperty ;
	mms-ontology:cardinality "*"^^uml-model-dt:cardinalityRange ;
	mms-ontology:key "substitutionIds" ;
	rdfs:label "substitution" ;
	rdfs:comment "A Substitution that belongs to this Classifier. Based on the UML property 'Classifier-substitution' which is described as: The Substitutions owned by this Classifier."@en ;
	rdfs:domain uml-class:Classifier ;
	rdfs:range uml-class:Substitution ;
	mms-ontology:umlPropertySource uml-property:Classifier-substitution .

mms-property:redefinedClassifier a mms-ontology:UmlObjectProperty ;
	mms-ontology:cardinality "*"^^uml-model-dt:cardinalityRange ;
	mms-ontology:key "redefinedClassifierIds" ;
	rdfs:label "redefinedClassifier" ;
	rdfs:comment "A Classifier that belongs to this Classifier. Based on the UML property 'Classifier-redefinedClassifier' which is described as: The Classifiers redefined by this Classifier."@en ;
	rdfs:domain uml-class:Classifier ;
	rdfs:range uml-class:Classifier ;
	mms-ontology:umlPropertySource uml-property:Classifier-redefinedClassifier .

mms-property:formalTemplateParameter a mms-ontology:UmlObjectProperty ;
	mms-ontology:cardinality "1"^^uml-model-dt:cardinalityRange ;
	mms-ontology:key "formalId" ;
	rdfs:label "formalTemplateParameter" ;
	rdfs:comment "The TemplateParameter that is the formal of this TemplateParameterSubstitution. Based on the UML property 'TemplateParameterSubstitution-formal' which is described as: The formal TemplateParameter that is associated with this TemplateParameterSubstitution."@en ;
	rdfs:domain uml-class:TemplateParameterSubstitution ;
	rdfs:range uml-class:TemplateParameter ;
	mms-ontology:umlPropertySource uml-property:TemplateParameterSubstitution-formal .

mms-property:boundElementTemplateableElement a mms-ontology:UmlObjectProperty ;
	mms-ontology:cardinality "1"^^uml-model-dt:cardinalityRange ;
	mms-ontology:key "boundElementId" ;
	rdfs:label "boundElementTemplateableElement" ;
	rdfs:comment "The TemplateableElement that is the boundElement of this TemplateBinding. Based on the UML property 'TemplateBinding-boundElement' which is described as: The TemplateableElement that is bound by this TemplateBinding."@en ;
	rdfs:domain uml-class:TemplateBinding ;
	rdfs:range uml-class:TemplateableElement ;
	mms-ontology:umlPropertySource uml-property:TemplateBinding-boundElement .

mms-property:inInterruptibleRegion a mms-ontology:UmlObjectProperty ;
	mms-ontology:cardinality "*"^^uml-model-dt:cardinalityRange ;
	mms-ontology:key "inInterruptibleRegionIds" ;
	rdfs:label "inInterruptibleRegion" ;
	rdfs:comment "A InterruptibleActivityRegion that is the inInterruptibleRegion of this ActivityNode. Based on the UML property 'ActivityNode-inInterruptibleRegion' which is described as: InterruptibleActivityRegions containing the ActivityNode."@en ;
	rdfs:domain uml-class:ActivityNode ;
	rdfs:range uml-class:InterruptibleActivityRegion ;
	mms-ontology:umlPropertySource uml-property:ActivityNode-inInterruptibleRegion .

mms-property:loopVariableInput a mms-ontology:UmlObjectProperty ;
	mms-ontology:cardinality "*"^^uml-model-dt:cardinalityRange ;
	mms-ontology:key "loopVariableInputIds" ;
	rdfs:label "loopVariableInput" ;
	rdfs:comment "A InputPin that is the loopVariableInput of this LoopNode. Based on the UML property 'LoopNode-loopVariableInput' which is described as: A list of InputPins whose values are moved into the loopVariable Pins before the first iteration of the loop."@en ;
	rdfs:domain uml-class:LoopNode ;
	rdfs:range uml-class:InputPin ;
	mms-ontology:umlPropertySource uml-property:LoopNode-loopVariableInput .

mms-property:icon a mms-ontology:UmlObjectProperty ;
	mms-ontology:cardinality "*"^^uml-model-dt:cardinalityRange ;
	mms-ontology:key "iconIds" ;
	rdfs:label "icon" ;
	rdfs:comment "A Image that is the icon of this Stereotype. Based on the UML property 'Stereotype-icon' which is described as: Stereotype can change the graphical appearance of the extended model element by using attached icons. When this association is not null, it references the location of the icon content to be displayed within diagrams presenting the extended model elements."@en ;
	rdfs:domain uml-class:Stereotype ;
	rdfs:range uml-class:Image ;
	mms-ontology:umlPropertySource uml-property:Stereotype-icon .

mms-property:fromAction a mms-ontology:UmlObjectProperty ;
	mms-ontology:cardinality "1"^^uml-model-dt:cardinalityRange ;
	mms-ontology:key "fromActionId" ;
	rdfs:label "fromAction" ;
	rdfs:comment "The Action that belongs to this ActionInputPin. Based on the UML property 'ActionInputPin-fromAction' which is described as: The Action used to provide the values of the ActionInputPin."@en ;
	rdfs:domain uml-class:ActionInputPin ;
	rdfs:range uml-class:Action ;
	mms-ontology:umlPropertySource uml-property:ActionInputPin-fromAction .

mms-property:nameString a mms-ontology:UmlDatatypeProperty ;
	mms-ontology:cardinality "1"^^uml-model-dt:cardinalityRange ;
	mms-ontology:key "nameId" ;
	rdfs:label "nameString" ;
	rdfs:comment "The String that is the name of this NamedElement. Based on the UML property 'NamedElement-name' which is described as: The name of the NamedElement."@en ;
	rdfs:domain uml-class:NamedElement ;
	rdfs:range xsd:string ;
	mms-ontology:umlPropertySource uml-property:NamedElement-name .

mms-property:redefinedNode a mms-ontology:UmlObjectProperty ;
	mms-ontology:cardinality "*"^^uml-model-dt:cardinalityRange ;
	mms-ontology:key "redefinedNodeIds" ;
	rdfs:label "redefinedNode" ;
	rdfs:comment "A ActivityNode that is the redefinedNode of this ActivityNode. Based on the UML property 'ActivityNode-redefinedNode' which is described as: ActivityNodes from a generalization of the Activity containining this ActivityNode that are redefined by this ActivityNode."@en ;
	rdfs:domain uml-class:ActivityNode ;
	rdfs:range uml-class:ActivityNode ;
	mms-ontology:umlPropertySource uml-property:ActivityNode-redefinedNode .

mms-property:isDestroyOwnedObjects a mms-ontology:UmlDatatypeProperty ;
	mms-ontology:key "isDestroyOwnedObjects" ;
	rdfs:label "isDestroyOwnedObjects" ;
	rdfs:comment "Specifies whether objects owned by the object (via composition) are destroyed along with the object."@en ;
	rdfs:domain uml-class:DestroyObjectAction ;
	rdfs:range xsd:boolean ;
	mms-ontology:umlPropertySource uml-property:DestroyObjectAction-isDestroyOwnedObjects .

mms-property:isDestroyOwnedObjectsDestroyObjectAction a mms-ontology:UmlDatatypeProperty ;
	owl:equivalentProperty mms-property:isDestroyOwnedObjects .

mms-property:constrainingClassifier a mms-ontology:UmlObjectProperty ;
	mms-ontology:cardinality "*"^^uml-model-dt:cardinalityRange ;
	mms-ontology:key "constrainingClassifierIds" ;
	rdfs:label "constrainingClassifier" ;
	rdfs:comment "A Classifier that belongs to this ClassifierTemplateParameter. Based on the UML property 'ClassifierTemplateParameter-constrainingClassifier' which is described as: The classifiers that constrain the argument that can be used for the parameter. If the allowSubstitutable attribute is true, then any Classifier that is compatible with this constraining Classifier can be substituted; otherwise, it must be either this Classifier or one of its specializations. If this property is empty, there are no constraints on the Classifier that can be used as an argument."@en ;
	rdfs:domain uml-class:ClassifierTemplateParameter ;
	rdfs:range uml-class:Classifier ;
	mms-ontology:umlPropertySource uml-property:ClassifierTemplateParameter-constrainingClassifier .

mms-property:isService a mms-ontology:UmlDatatypeProperty ;
	mms-ontology:key "isService" ;
	rdfs:label "isService" ;
	rdfs:comment "If true, indicates that this Port is used to provide the published functionality of an EncapsulatedClassifier.  If false, this Port is used to implement the EncapsulatedClassifier but is not part of the essential externally-visible functionality of the EncapsulatedClassifier and can, therefore, be altered or deleted along with the internal implementation of the EncapsulatedClassifier and other properties that are considered part of its implementation."@en ;
	rdfs:domain uml-class:Port ;
	rdfs:range xsd:boolean ;
	mms-ontology:umlPropertySource uml-property:Port-isService .

mms-property:isServicePort a mms-ontology:UmlDatatypeProperty ;
	owl:equivalentProperty mms-property:isService .

mms-property:instanceInstanceSpecification a mms-ontology:UmlObjectProperty ;
	mms-ontology:cardinality "1"^^uml-model-dt:cardinalityRange ;
	mms-ontology:key "instanceId" ;
	rdfs:label "instanceInstanceSpecification" ;
	rdfs:comment "The InstanceSpecification that is the instance of this InstanceValue. Based on the UML property 'InstanceValue-instance' which is described as: The InstanceSpecification that represents the specified value."@en ;
	rdfs:domain uml-class:InstanceValue ;
	rdfs:range uml-class:InstanceSpecification ;
	mms-ontology:umlPropertySource uml-property:InstanceValue-instance .

mms-property:outputElement a mms-ontology:UmlObjectProperty ;
	mms-ontology:cardinality "*"^^uml-model-dt:cardinalityRange ;
	mms-ontology:key "outputElementIds" ;
	rdfs:label "outputElement" ;
	rdfs:comment "A ExpansionNode that is the outputElement of this ExpansionRegion. Based on the UML property 'ExpansionRegion-outputElement' which is described as: The ExpansionNodes that form the output collections of the ExpansionRegion."@en ;
	rdfs:domain uml-class:ExpansionRegion ;
	rdfs:range uml-class:ExpansionNode ;
	mms-ontology:umlPropertySource uml-property:ExpansionRegion-outputElement .

mms-property:part a mms-ontology:UmlObjectProperty ;
	mms-ontology:cardinality "*"^^uml-model-dt:cardinalityRange ;
	mms-ontology:key "partIds" ;
	rdfs:label "part" ;
	rdfs:comment "A Property that is the part of this StructuredClassifier. Based on the UML property 'StructuredClassifier-part' which is described as: The Properties specifying instances that the StructuredClassifier owns by composition. This collection is derived, selecting those owned Properties where isComposite is true."@en ;
	rdfs:domain uml-class:StructuredClassifier ;
	rdfs:range uml-class:Property ;
	mms-ontology:umlPropertySource uml-property:StructuredClassifier-part .

mms-property:changeExpressionValueSpecification a mms-ontology:UmlObjectProperty ;
	mms-ontology:cardinality "1"^^uml-model-dt:cardinalityRange ;
	mms-ontology:key "changeExpressionId" ;
	rdfs:label "changeExpressionValueSpecification" ;
	rdfs:comment "The ValueSpecification that is the changeExpression of this ChangeEvent. Based on the UML property 'ChangeEvent-changeExpression' which is described as: A Boolean-valued ValueSpecification that will result in a ChangeEvent whenever its value changes from false to true."@en ;
	rdfs:domain uml-class:ChangeEvent ;
	rdfs:range uml-class:ValueSpecification ;
	mms-ontology:umlPropertySource uml-property:ChangeEvent-changeExpression .

mms-property:symbolString a mms-ontology:UmlDatatypeProperty ;
	mms-ontology:cardinality "1"^^uml-model-dt:cardinalityRange ;
	mms-ontology:key "symbolId" ;
	rdfs:label "symbolString" ;
	rdfs:comment "The String that is the symbol of this Expression. Based on the UML property 'Expression-symbol' which is described as: The symbol associated with this node in the expression tree."@en ;
	rdfs:domain uml-class:Expression ;
	rdfs:range xsd:string ;
	mms-ontology:umlPropertySource uml-property:Expression-symbol .

mms-property:isException a mms-ontology:UmlDatatypeProperty ;
	mms-ontology:key "isException" ;
	rdfs:label "isException" ;
	rdfs:comment "Tells whether an output parameter may emit a value to the exclusion of the other outputs."@en ;
	rdfs:domain uml-class:Parameter ;
	rdfs:range xsd:boolean ;
	mms-ontology:umlPropertySource uml-property:Parameter-isException .

mms-property:isExceptionParameter a mms-ontology:UmlDatatypeProperty ;
	owl:equivalentProperty mms-property:isException .

mms-property:returnValueRecipientProperty a mms-ontology:UmlObjectProperty ;
	mms-ontology:cardinality "1"^^uml-model-dt:cardinalityRange ;
	mms-ontology:key "returnValueRecipientId" ;
	rdfs:label "returnValueRecipientProperty" ;
	rdfs:comment "The Property that is the returnValueRecipient of this InteractionUse. Based on the UML property 'InteractionUse-returnValueRecipient' which is described as: The recipient of the return value."@en ;
	rdfs:domain uml-class:InteractionUse ;
	rdfs:range uml-class:Property ;
	mms-ontology:umlPropertySource uml-property:InteractionUse-returnValueRecipient .

mms-property:isReentrant a mms-ontology:UmlDatatypeProperty ;
	mms-ontology:key "isReentrant" ;
	rdfs:label "isReentrant" ;
	rdfs:comment "Tells whether the Behavior can be invoked while it is still executing from a previous invocation."@en ;
	rdfs:domain uml-class:Behavior ;
	rdfs:range xsd:boolean ;
	mms-ontology:umlPropertySource uml-property:Behavior-isReentrant .

mms-property:isReentrantBehavior a mms-ontology:UmlDatatypeProperty ;
	owl:equivalentProperty mms-property:isReentrant .

mms-property:nestedNode a mms-ontology:UmlObjectProperty ;
	mms-ontology:cardinality "*"^^uml-model-dt:cardinalityRange ;
	mms-ontology:key "nestedNodeIds" ;
	rdfs:label "nestedNode" ;
	rdfs:comment "A Node that belongs to this Node. Based on the UML property 'Node-nestedNode' which is described as: The Nodes that are defined (nested) within the Node."@en ;
	rdfs:domain uml-class:Node ;
	rdfs:range uml-class:Node ;
	mms-ontology:umlPropertySource uml-property:Node-nestedNode .

mms-property:startOccurrenceSpecification a mms-ontology:UmlObjectProperty ;
	mms-ontology:cardinality "1"^^uml-model-dt:cardinalityRange ;
	mms-ontology:key "startId" ;
	rdfs:label "startOccurrenceSpecification" ;
	rdfs:comment "The OccurrenceSpecification that is the start of this ExecutionSpecification. Based on the UML property 'ExecutionSpecification-start' which is described as: References the OccurrenceSpecification that designates the start of the Action or Behavior."@en ;
	rdfs:domain uml-class:ExecutionSpecification ;
	rdfs:range uml-class:OccurrenceSpecification ;
	mms-ontology:umlPropertySource uml-property:ExecutionSpecification-start .

mms-property:extensionLocation a mms-ontology:UmlObjectProperty ;
	mms-ontology:cardinality "*"^^uml-model-dt:cardinalityRange ;
	mms-ontology:key "extensionLocationIds" ;
	rdfs:label "extensionLocation" ;
	rdfs:comment "A ExtensionPoint that is the extensionLocation of this Extend. Based on the UML property 'Extend-extensionLocation' which is described as: An ordered list of ExtensionPoints belonging to the extended UseCase, specifying where the respective behavioral fragments of the extending UseCase are to be inserted. The first fragment in the extending UseCase is associated with the first extension point in the list, the second fragment with the second point, and so on. Note that, in most practical cases, the extending UseCase has just a single behavior fragment, so that the list of ExtensionPoints is trivial."@en ;
	rdfs:domain uml-class:Extend ;
	rdfs:range uml-class:ExtensionPoint ;
	mms-ontology:umlPropertySource uml-property:Extend-extensionLocation .

mms-property:isStrict a mms-ontology:UmlDatatypeProperty ;
	mms-ontology:key "isStrict" ;
	rdfs:label "isStrict" ;
	rdfs:comment "Specifies that the Profile filtering rules for the metaclasses of the referenced metamodel shall be strictly applied."@en ;
	rdfs:domain uml-class:ProfileApplication ;
	rdfs:range xsd:boolean ;
	mms-ontology:umlPropertySource uml-property:ProfileApplication-isStrict .

mms-property:isStrictProfileApplication a mms-ontology:UmlDatatypeProperty ;
	owl:equivalentProperty mms-property:isStrict .

mms-property:ownedType a mms-ontology:UmlObjectProperty ;
	mms-ontology:cardinality "*"^^uml-model-dt:cardinalityRange ;
	mms-ontology:key "ownedTypeIds" ;
	rdfs:label "ownedType" ;
	rdfs:comment "A Type that belongs to this Package. Based on the UML property 'Package-ownedType' which is described as: References the packaged elements that are Types."@en ;
	rdfs:domain uml-class:Package ;
	rdfs:range uml-class:Type ;
	mms-ontology:umlPropertySource uml-property:Package-ownedType .

mms-property:superGroupActivityGroup a mms-ontology:UmlObjectProperty ;
	mms-ontology:cardinality "1"^^uml-model-dt:cardinalityRange ;
	mms-ontology:key "superGroupId" ;
	rdfs:label "superGroupActivityGroup" ;
	rdfs:comment "The ActivityGroup that is the superGroup of this ActivityGroup. Based on the UML property 'ActivityGroup-superGroup' which is described as: The ActivityGroup immediately containing this ActivityGroup, if it is directly owned by another ActivityGroup."@en ;
	rdfs:domain uml-class:ActivityGroup ;
	rdfs:range uml-class:ActivityGroup ;
	mms-ontology:umlPropertySource uml-property:ActivityGroup-superGroup .

mms-property:implementingClassifierBehavioredClassifier a mms-ontology:UmlObjectProperty ;
	mms-ontology:cardinality "1"^^uml-model-dt:cardinalityRange ;
	mms-ontology:key "implementingClassifierId" ;
	rdfs:label "implementingClassifierBehavioredClassifier" ;
	rdfs:comment "The BehavioredClassifier that is the implementingClassifier of this InterfaceRealization. Based on the UML property 'InterfaceRealization-implementingClassifier' which is described as: References the BehavioredClassifier that owns this InterfaceRealization, i.e., the BehavioredClassifier that realizes the Interface to which it refers."@en ;
	rdfs:domain uml-class:InterfaceRealization ;
	rdfs:range uml-class:BehavioredClassifier ;
	mms-ontology:umlPropertySource uml-property:InterfaceRealization-implementingClassifier .

mms-property:importedElementPackageableElement a mms-ontology:UmlObjectProperty ;
	mms-ontology:cardinality "1"^^uml-model-dt:cardinalityRange ;
	mms-ontology:key "importedElementId" ;
	rdfs:label "importedElementPackageableElement" ;
	rdfs:comment "The PackageableElement that is the importedElement of this ElementImport. Based on the UML property 'ElementImport-importedElement' which is described as: Specifies the PackageableElement whose name is to be added to a Namespace."@en ;
	rdfs:domain uml-class:ElementImport ;
	rdfs:range uml-class:PackageableElement ;
	mms-ontology:umlPropertySource uml-property:ElementImport-importedElement .

mms-property:interruptsInterruptibleActivityRegion a mms-ontology:UmlObjectProperty ;
	mms-ontology:cardinality "1"^^uml-model-dt:cardinalityRange ;
	mms-ontology:key "interruptsId" ;
	rdfs:label "interruptsInterruptibleActivityRegion" ;
	rdfs:comment "The InterruptibleActivityRegion that is the interrupts of this ActivityEdge. Based on the UML property 'ActivityEdge-interrupts' which is described as: The InterruptibleActivityRegion for which this ActivityEdge is an interruptingEdge."@en ;
	rdfs:domain uml-class:ActivityEdge ;
	rdfs:range uml-class:InterruptibleActivityRegion ;
	mms-ontology:umlPropertySource uml-property:ActivityEdge-interrupts .

mms-property:mergedPackage a mms-ontology:UmlObjectProperty ;
	mms-ontology:cardinality "1"^^uml-model-dt:cardinalityRange ;
	mms-ontology:key "mergedPackageId" ;
	rdfs:label "mergedPackage" ;
	rdfs:comment "The Package that belongs to this PackageMerge. Based on the UML property 'PackageMerge-mergedPackage' which is described as: References the Package that is to be merged with the receiving package of the PackageMerge."@en ;
	rdfs:domain uml-class:PackageMerge ;
	rdfs:range uml-class:Package ;
	mms-ontology:umlPropertySource uml-property:PackageMerge-mergedPackage .

mms-property:represented a mms-ontology:UmlObjectProperty ;
	mms-ontology:cardinality "*"^^uml-model-dt:cardinalityRange ;
	mms-ontology:key "representedIds" ;
	rdfs:label "represented" ;
	rdfs:comment "A Classifier that is the represented of this InformationItem. Based on the UML property 'InformationItem-represented' which is described as: Determines the classifiers that will specify the structure and nature of the information. An information item represents all its represented classifiers."@en ;
	rdfs:domain uml-class:InformationItem ;
	rdfs:range uml-class:Classifier ;
	mms-ontology:umlPropertySource uml-property:InformationItem-represented .

mms-property:isSingleExecution a mms-ontology:UmlDatatypeProperty ;
	mms-ontology:key "isSingleExecution" ;
	rdfs:label "isSingleExecution" ;
	rdfs:comment "If true, all invocations of the Activity are handled by the same execution."@en ;
	rdfs:domain uml-class:Activity ;
	rdfs:range xsd:boolean ;
	mms-ontology:umlPropertySource uml-property:Activity-isSingleExecution .

mms-property:isSingleExecutionActivity a mms-ontology:UmlDatatypeProperty ;
	owl:equivalentProperty mms-property:isSingleExecution .

mms-property:ownedPort a mms-ontology:UmlObjectProperty ;
	mms-ontology:cardinality "*"^^uml-model-dt:cardinalityRange ;
	mms-ontology:key "ownedPortIds" ;
	rdfs:label "ownedPort" ;
	rdfs:comment "A Port that belongs to this EncapsulatedClassifier. Based on the UML property 'EncapsulatedClassifier-ownedPort' which is described as: The Ports owned by the EncapsulatedClassifier."@en ;
	rdfs:domain uml-class:EncapsulatedClassifier ;
	rdfs:range uml-class:Port ;
	mms-ontology:umlPropertySource uml-property:EncapsulatedClassifier-ownedPort .

mms-property:referred a mms-ontology:UmlObjectProperty ;
	mms-ontology:cardinality "*"^^uml-model-dt:cardinalityRange ;
	mms-ontology:key "referredIds" ;
	rdfs:label "referred" ;
	rdfs:comment "A Operation that is the referred of this ProtocolTransition. Based on the UML property 'ProtocolTransition-referred' which is described as: This association refers to the associated Operation. It is derived from the Operation of the CallEvent Trigger when applicable."@en ;
	rdfs:domain uml-class:ProtocolTransition ;
	rdfs:range uml-class:Operation ;
	mms-ontology:umlPropertySource uml-property:ProtocolTransition-referred .

mms-property:ownedMember a mms-ontology:UmlObjectProperty ;
	mms-ontology:cardinality "*"^^uml-model-dt:cardinalityRange ;
	mms-ontology:key "ownedMemberIds" ;
	rdfs:label "ownedMember" ;
	rdfs:comment "A NamedElement that is the ownedMember of this Namespace. Based on the UML property 'Namespace-ownedMember' which is described as: A collection of NamedElements owned by the Namespace."@en ;
	rdfs:domain uml-class:Namespace ;
	rdfs:range uml-class:NamedElement ;
	mms-ontology:umlPropertySource uml-property:Namespace-ownedMember .

mms-property:utilizedElementPackageableElement a mms-ontology:UmlObjectProperty ;
	mms-ontology:cardinality "1"^^uml-model-dt:cardinalityRange ;
	mms-ontology:key "utilizedElementId" ;
	rdfs:label "utilizedElementPackageableElement" ;
	rdfs:comment "The PackageableElement that is the utilizedElement of this Manifestation. Based on the UML property 'Manifestation-utilizedElement' which is described as: The model element that is utilized in the manifestation in an Artifact."@en ;
	rdfs:domain uml-class:Manifestation ;
	rdfs:range uml-class:PackageableElement ;
	mms-ontology:umlPropertySource uml-property:Manifestation-utilizedElement .

mms-property:isStatic a mms-ontology:UmlDatatypeProperty ;
	mms-ontology:key "isStatic" ;
	rdfs:label "isStatic" ;
	rdfs:comment "Specifies whether this Feature characterizes individual instances classified by the Classifier (false) or the Classifier itself (true)."@en ;
	rdfs:domain uml-class:Feature ;
	rdfs:range xsd:boolean ;
	mms-ontology:umlPropertySource uml-property:Feature-isStatic .

mms-property:isStaticFeature a mms-ontology:UmlDatatypeProperty ;
	owl:equivalentProperty mms-property:isStatic .

